<?xml version="1.0"?>
<rdf:RDF xmlns="https://w3id.org/itsVocab/"
    xml:base="https://w3id.org/itsVocab/"
    xmlns:cc="http://creativecommons.org/ns#"
    xmlns:dcterms="http://purl.org/dc/terms/"
    xmlns:owl="http://www.w3.org/2002/07/owl#"
    xmlns:rdf="http://www.w3.org/1999/02/22-rdf-syntax-ns#"
    xmlns:rdfs="http://www.w3.org/2000/01/rdf-schema#"
    xmlns:skos="http://www.w3.org/2004/02/skos/core#"
    xmlns:vann="http://purl.org/vocab/vann/"
    xmlns:xml="http://www.w3.org/XML/1998/namespace"
    xmlns:xsd="http://www.w3.org/2001/XMLSchema#">
    <owl:Ontology rdf:about="https://w3id.org/itsVocab/">
        <dcterms:title>ITS Vocabulary</dcterms:title>
        <dcterms:description>
            A vocabulary defined for Intelligent Transport Systems and documented as a formal
            ontology. The contents of this vocabulary are periodically standardized in ISO 14812,
            whereas this file is maintained through a [GitHub
            project](https://github.com/ISO-TC204/iso14812).

            The original version of the vocabulary was published as [ISO/TS
            14812:2022](https://www.iso.org/standard/79779.html). [Edition
            2](https://www.iso.org/standard/85041.html) was released in 2025.

            With edition 3, the draft standard is now generated from this ontology file, originally
            developed in 2026.
        </dcterms:description>
        <vann:preferredNamespacePrefix>itsVocab</vann:preferredNamespacePrefix>
        <dcterms:license rdf:resource="http://creativecommons.org/licenses/by/4.0/" />
        <cc:attributionName>ISO 14812</cc:attributionName>

        <!-- Authors -->
        <dcterms:creator>Kenneth Vaughn</dcterms:creator>

        <!-- Dates -->
        <dcterms:issued rdf:datatype="xsd:date">2026-01-05</dcterms:issued>  <!-- latest date of prior
        versions -->
        <dcterms:modified rdf:datatype="xsd:date">2026-01-05</dcterms:modified>  <!-- latest edits -->

        <!-- Version history -->
        <owl:versionInfo>1.1.1</owl:versionInfo>
        <rdfs:comment>
            1.0.0 - 2022: Published as ISO/TS 14812:2022.
            1.1.0 - 2025: Updated to reflect ISO/TS 14812:2025 (Edition 2).
            1.1.1 - 2026: Converted to formal ontology.

            Note: Version numbers follow semantic versioning principles (major.minor.patch). This is
            different than ISO standard edition numbers, which are sequential.
        </rdfs:comment>
        <owl:versionIRI rdf:resource="https://w3id.org/itsVocab/1.1.1/" />
    </owl:Ontology>

    <skos:Collection rdf:about="terms">
      <skos:member rdf:resource="coreTerms"/>
      <skos:member rdf:resource="technologyTerms"/>
      <skos:member rdf:resource="infrastructureTerms"/>
      <skos:member rdf:resource="locationTerms"/>
      <skos:member rdf:resource="serviceTerms"/>
      <skos:member rdf:resource="userTerms"/>
      <skos:member rdf:resource="vehicleTerms"/>
      <skos:member rdf:resource="financialTerms"/>
    </skos:Collection>
    <skos:Collection rdf:about="coreTerms">
      <skos:member rdf:resource="entityTerms"/>
      <skos:member rdf:resource="generalSystemTerms"/>
      <skos:member rdf:resource="generalArchitectureTerms"/>
      <skos:member rdf:resource="architectureViewTerms"/>
      <skos:member rdf:resource="architectureCommunicationViewTerms"/>
      <skos:member rdf:resource="architectureEnterpriseViewTerms"/>
      <skos:member rdf:resource="architectureFunctionalViewTerms"/>
      <skos:member rdf:resource="architecturePhysicalViewTerms"/>
      <skos:member rdf:resource="architectureTypeTerms"/>
      <skos:member rdf:resource="dataConceptManagementTerms"/>
      <skos:member rdf:resource="dataConceptTypeTerms"/>
      <skos:member rdf:resource="systemEngineeringTerms"/>
      <skos:member rdf:resource="timeTerms"/>
      <skos:member rdf:resource="informationSecurityTerms"/>
      <skos:member rdf:resource="conceptRealizationTerms"/>
    </skos:Collection>
    <skos:Collection rdf:about="technologyTerms">
      <skos:member rdf:resource="top-levelPhysicalObjectTerms"/>
      <skos:member rdf:resource="centrePhysicalObjectTerms"/>
      <skos:member rdf:resource="fieldPhysicalObjectTerms"/>
      <skos:member rdf:resource="personalPhysicalObjectTerms"/>
      <skos:member rdf:resource="supportPhysicalObjectTerms"/>
      <skos:member rdf:resource="vehiclePhysicalObjectTerms"/>
      <skos:member rdf:resource="itsStationTerms"/>
      <skos:member rdf:resource="itsApplicationTerms"/>
      <skos:member rdf:resource="its-sApplicationProcessTerms"/>
      <skos:member rdf:resource="deviceComponentTerms"/>
    </skos:Collection>
    <skos:Collection rdf:about="infrastructureTerms">
      <skos:member rdf:resource="roadReservationComponentTerms"/>
      <skos:member rdf:resource="physicalTrafficSeparatorTerms"/>
      <skos:member rdf:resource="alternateModeInfrastructureComponentTerms"/>
      <skos:member rdf:resource="infrastructureOperatingModeTerms"/>
      <skos:member rdf:resource="roadNetworkTerms"/>
      <skos:member rdf:resource="junctionTerms"/>
      <skos:member rdf:resource="facilityTerms"/>
      <skos:member rdf:resource="kerbsideUsageTerms"/>
      <skos:member rdf:resource="roadEquipmentTerms"/>
    </skos:Collection>
    <skos:Collection rdf:about="locationTerms">
      <skos:member rdf:resource="locationTypeTerms"/>
      <skos:member rdf:resource="locationReferencingTerms"/>
      <skos:member rdf:resource="jurisdictionalTerms"/>
    </skos:Collection>
    <skos:Collection rdf:about="serviceTerms">
      <skos:member rdf:resource="genericServiceTerms"/>
      <skos:member rdf:resource="transportServiceTerms"/>
      <skos:member rdf:resource="itsServiceTerms"/>
      <skos:member rdf:resource="its-suServiceTerms"/>
      <skos:member rdf:resource="transportServiceApplicationTerms"/>
      <skos:member rdf:resource="transport-relatedSharingTerms"/>
      <skos:member rdf:resource="contractualModelTerms"/>
      <skos:member rdf:resource="financialModelTerms"/>
      <skos:member rdf:resource="operationalModelTerms"/>
      <skos:member rdf:resource="networkModelTerms"/>
      <skos:member rdf:resource="sharedTransportServiceTerms"/>
      <skos:member rdf:resource="sharedVehicleTerms"/>
    </skos:Collection>
    <skos:Collection rdf:about="userTerms">
      <skos:member rdf:resource="travellerTerms"/>
      <skos:member rdf:resource="vehicleOccupantTerms"/>
    </skos:Collection>
    <skos:Collection rdf:about="vehicleTerms">
      <skos:member rdf:resource="vehicleComponentTerms"/>
      <skos:member rdf:resource="vehicleAttributeTerms"/>
      <skos:member rdf:resource="vehicleAutomationTerms"/>
      <skos:member rdf:resource="vehicleConnectivityTerms"/>
      <skos:member rdf:resource="vehicleSpeedTerms"/>
      <skos:member rdf:resource="vehicleTypesEnvironmentTerms"/>
    </skos:Collection>
    <skos:Collection rdf:about="financialTerms">
      <skos:member rdf:resource="paymentTerms"/>
    </skos:Collection>
    <skos:Collection rdf:about="entityTerms">
      <skos:member rdf:resource="entity"/>
      <skos:member rdf:resource="immaterialEntity"/>
      <skos:member rdf:resource="materialEntity"/>
      <skos:member rdf:resource="non-biologicalEntity"/>
      <skos:member rdf:resource="biologicalEntity"/>
    </skos:Collection>
    <skos:Collection rdf:about="generalSystemTerms">
      <skos:member rdf:resource="system"/>
      <skos:member rdf:resource="transportSystem"/>
      <skos:member rdf:resource="surfaceTransportSystem"/>
      <skos:member rdf:resource="intelligentTransportSystem"/>
    </skos:Collection>
    <skos:Collection rdf:about="generalArchitectureTerms">
      <skos:member rdf:resource="architecture"/>
      <skos:member rdf:resource="architectureDescription"/>
      <skos:member rdf:resource="architectureFramework"/>
      <skos:member rdf:resource="stakeholder"/>
      <skos:member rdf:resource="concern"/>
      <skos:member rdf:resource="architectureViewpoint"/>
      <skos:member rdf:resource="architectureView"/>
      <skos:member rdf:resource="modelKind"/>
      <skos:member rdf:resource="architectureModel"/>
      <skos:member rdf:resource="element"/>
    </skos:Collection>
    <skos:Collection rdf:about="architectureViewTerms">
      <skos:member rdf:resource="communicationsView"/>
      <skos:member rdf:resource="communicationsViewpoint"/>
      <skos:member rdf:resource="enterpriseView"/>
      <skos:member rdf:resource="enterpriseViewpoint"/>
      <skos:member rdf:resource="functionalView"/>
      <skos:member rdf:resource="functionalViewpoint"/>
      <skos:member rdf:resource="physicalView"/>
    </skos:Collection>
    <skos:Collection rdf:about="architectureCommunicationViewTerms">
      <skos:member rdf:resource="applicationEntity"/>
      <skos:member rdf:resource="accessLayer"/>
      <skos:member rdf:resource="its-sAccessLayer"/>
      <skos:member rdf:resource="transnetLayer"/>
      <skos:member rdf:resource="facilitiesLayer"/>
      <skos:member rdf:resource="managementEntity"/>
    </skos:Collection>
    <skos:Collection rdf:about="architectureEnterpriseViewTerms">
      <skos:member rdf:resource="enterpriseObject"/>
      <skos:member rdf:resource="resource"/>
      <skos:member rdf:resource="document"/>
      <skos:member rdf:resource="interaction"/>
      <skos:member rdf:resource="formalCoordination"/>
      <skos:member rdf:resource="informalCoordination"/>
      <skos:member rdf:resource="role"/>
      <skos:member rdf:resource="relationship"/>
      <skos:member rdf:resource="include"/>
    </skos:Collection>
    <skos:Collection rdf:about="architectureFunctionalViewTerms">
      <skos:member rdf:resource="dataFlow"/>
      <skos:member rdf:resource="process"/>
      <skos:member rdf:resource="function"/>
    </skos:Collection>
    <skos:Collection rdf:about="architecturePhysicalViewTerms">
      <skos:member rdf:resource="physicalObject"/>
      <skos:member rdf:resource="itsComponent"/>
      <skos:member rdf:resource="terminator"/>
      <skos:member rdf:resource="informationFlow"/>
      <skos:member rdf:resource="informationTransfer"/>
      <skos:member rdf:resource="functionalObject"/>
    </skos:Collection>
    <skos:Collection rdf:about="architectureTypeTerms">
      <skos:member rdf:resource="referenceArchitecture"/>
      <skos:member rdf:resource="planningArchitecture"/>
      <skos:member rdf:resource="deploymentArchitecture"/>
      <skos:member rdf:resource="its-sReferenceArchitecture"/>
      <skos:member rdf:resource="itsReferenceArchitecture"/>
      <skos:member rdf:resource="itsPlanningArchitecture"/>
    </skos:Collection>
    <skos:Collection rdf:about="dataConceptManagementTerms">
      <skos:member rdf:resource="dataConcept"/>
      <skos:member rdf:resource="meta-attribute"/>
      <skos:member rdf:resource="dataDictionary"/>
    </skos:Collection>
    <skos:Collection rdf:about="dataConceptTypeTerms">
      <skos:member rdf:resource="dataElement"/>
      <skos:member rdf:resource="class"/>
      <skos:member rdf:resource="valueDomain"/>
      <skos:member rdf:resource="dataFrame"/>
      <skos:member rdf:resource="message"/>
    </skos:Collection>
    <skos:Collection rdf:about="systemEngineeringTerms">
      <skos:member rdf:resource="useCase"/>
      <skos:member rdf:resource="scenario"/>
    </skos:Collection>
    <skos:Collection rdf:about="timeTerms">
      <skos:member rdf:resource="instant"/>
      <skos:member rdf:resource="duration"/>
    </skos:Collection>
    <skos:Collection rdf:about="informationSecurityTerms">
      <skos:member rdf:resource="authentication"/>
      <skos:member rdf:resource="authenticator"/>
      <skos:member rdf:resource="control"/>
      <skos:member rdf:resource="cryptography"/>
      <skos:member rdf:resource="dataPrivacy"/>
      <skos:member rdf:resource="digitalSignature"/>
      <skos:member rdf:resource="informationSecurityEvent"/>
      <skos:member rdf:resource="informationSecurityIncident"/>
      <skos:member rdf:resource="nonRepudiation"/>
      <skos:member rdf:resource="objective"/>
      <skos:member rdf:resource="resilience"/>
      <skos:member rdf:resource="risk"/>
      <skos:member rdf:resource="threat"/>
      <skos:member rdf:resource="transparency"/>
      <skos:member rdf:resource="trustworthiness"/>
      <skos:member rdf:resource="vulnerability"/>
    </skos:Collection>
    <skos:Collection rdf:about="conceptRealizationTerms">
      <skos:member rdf:resource="design"/>
      <skos:member rdf:resource="implementation"/>
      <skos:member rdf:resource="instance"/>
      <skos:member rdf:resource="realization"/>
      <skos:member rdf:resource="requirement"/>
      <skos:member rdf:resource="requirementsSpecification"/>
    </skos:Collection>
    <skos:Collection rdf:about="top-levelPhysicalObjectTerms">
      <skos:member rdf:resource="centralSystem"/>
      <skos:member rdf:resource="fieldSystem"/>
      <skos:member rdf:resource="personalSystem"/>
      <skos:member rdf:resource="supportSystem"/>
    </skos:Collection>
    <skos:Collection rdf:about="centrePhysicalObjectTerms">
      <skos:member rdf:resource="emergencyManagementCentralSystem"/>
      <skos:member rdf:resource="fleetAndFreightManagementCentralSystem"/>
      <skos:member rdf:resource="maintenanceAndConstructionCentralManagementSystem"/>
      <skos:member rdf:resource="paymentAdministrationCentralSystem"/>
      <skos:member rdf:resource="publicTransportCentralManagementSystem"/>
      <skos:member rdf:resource="trafficManagementCentralSystem"/>
      <skos:member rdf:resource="trafficRegulationCentralSystem"/>
    </skos:Collection>
    <skos:Collection rdf:about="fieldPhysicalObjectTerms">
      <skos:member rdf:resource="fieldSupportEquipment"/>
      <skos:member rdf:resource="itsRoadsideEquipment"/>
      <skos:member rdf:resource="connectedVehicleRoadsideEquipment"/>
      <skos:member rdf:resource="roadsideUnit"/>
      <skos:member rdf:resource="connectedUnit"/>
      <skos:member rdf:resource="connected"/>
    </skos:Collection>
    <skos:Collection rdf:about="personalPhysicalObjectTerms">
      <skos:member rdf:resource="nomadicVehicleDevice"/>
      <skos:member rdf:resource="personalInformationDevice"/>
      <skos:member rdf:resource="nomadicDevice"/>
    </skos:Collection>
    <skos:Collection rdf:about="supportPhysicalObjectTerms">
      <skos:member rdf:resource="cooperativeItsCredentialsManagementSystem"/>
    </skos:Collection>
    <skos:Collection rdf:about="vehiclePhysicalObjectTerms">
      <skos:member rdf:resource="itsOn-boardEquipment"/>
    </skos:Collection>
    <skos:Collection rdf:about="itsStationTerms">
      <skos:member rdf:resource="boundedSecuredManagedDomain"/>
      <skos:member rdf:resource="itsTrustDomain"/>
      <skos:member rdf:resource="itsStation"/>
      <skos:member rdf:resource="its-sUnit"/>
      <skos:member rdf:resource="its-sCommunicationUnit"/>
      <skos:member rdf:resource="its-sHost"/>
      <skos:member rdf:resource="its-sRouter"/>
    </skos:Collection>
    <skos:Collection rdf:about="itsApplicationTerms">
      <skos:member rdf:resource="itsApplication"/>
      <skos:member rdf:resource="interoperabilityDesign"/>
      <skos:member rdf:resource="itsApplicationSpecification"/>
      <skos:member rdf:resource="applicationTemplate"/>
      <skos:member rdf:resource="itsImplementation"/>
    </skos:Collection>
    <skos:Collection rdf:about="its-sApplicationProcessTerms">
      <skos:member rdf:resource="itsApplicationRole"/>
      <skos:member rdf:resource="its-sApplicationProcess"/>
      <skos:member rdf:resource="its-sApplication"/>
      <skos:member rdf:resource="its-sApplicationImplementation"/>
      <skos:member rdf:resource="its-sApplicationProcessInstallation"/>
    </skos:Collection>
    <skos:Collection rdf:about="deviceComponentTerms">
      <skos:member rdf:resource="actuator"/>
      <skos:member rdf:resource="sensor"/>
    </skos:Collection>
    <skos:Collection rdf:about="roadReservationComponentTerms">
      <skos:member rdf:resource="cross-section"/>
      <skos:member rdf:resource="roadReservation"/>
      <skos:member rdf:resource="roadway"/>
      <skos:member rdf:resource="drivingSpace"/>
      <skos:member rdf:resource="carriageway"/>
      <skos:member rdf:resource="travelledWay"/>
      <skos:member rdf:resource="singleCarriageway"/>
      <skos:member rdf:resource="dualCarriageway"/>
      <skos:member rdf:resource="multipleCarriageway"/>
      <skos:member rdf:resource="roadside"/>
      <skos:member rdf:resource="verge"/>
      <skos:member rdf:resource="lane"/>
      <skos:member rdf:resource="trafficLane"/>
      <skos:member rdf:resource="reservedLane"/>
      <skos:member rdf:resource="usableWidth"/>
      <skos:member rdf:resource="lay-by"/>
      <skos:member rdf:resource="hardstanding"/>
      <skos:member rdf:resource="shoulder"/>
      <skos:member rdf:resource="hardShoulder"/>
      <skos:member rdf:resource="softShoulder"/>
    </skos:Collection>
    <skos:Collection rdf:about="physicalTrafficSeparatorTerms">
      <skos:member rdf:resource="physicalTrafficSeparator"/>
      <skos:member rdf:resource="centralReservation"/>
      <skos:member rdf:resource="jerseyBarrier"/>
    </skos:Collection>
    <skos:Collection rdf:about="alternateModeInfrastructureComponentTerms">
      <skos:member rdf:resource="cycleLane"/>
      <skos:member rdf:resource="cycleway"/>
      <skos:member rdf:resource="footpath"/>
      <skos:member rdf:resource="sidewalk"/>
      <skos:member rdf:resource="escalator"/>
      <skos:member rdf:resource="movingWalkway"/>
      <skos:member rdf:resource="pedestrianCrossing"/>
      <skos:member rdf:resource="sharedSpace"/>
      <skos:member rdf:resource="block-face"/>
    </skos:Collection>
    <skos:Collection rdf:about="infrastructureOperatingModeTerms">
      <skos:member rdf:resource="hardShoulderForEmergencyUse"/>
    </skos:Collection>
    <skos:Collection rdf:about="roadNetworkTerms">
      <skos:member rdf:resource="road"/>
      <skos:member rdf:resource="roadNetwork"/>
      <skos:member rdf:resource="roadModel"/>
      <skos:member rdf:resource="node"/>
      <skos:member rdf:resource="link"/>
      <skos:member rdf:resource="roadLink"/>
      <skos:member rdf:resource="roadSection"/>
      <skos:member rdf:resource="roadSegment"/>
      <skos:member rdf:resource="laneLink"/>
      <skos:member rdf:resource="laneSegment"/>
      <skos:member rdf:resource="alley"/>
      <skos:member rdf:resource="roadIdentifier"/>
      <skos:member rdf:resource="serviceRoad"/>
    </skos:Collection>
    <skos:Collection rdf:about="junctionTerms">
      <skos:member rdf:resource="intersection"/>
      <skos:member rdf:resource="junction"/>
      <skos:member rdf:resource="ingressLane"/>
      <skos:member rdf:resource="ingressLink"/>
      <skos:member rdf:resource="egressLane"/>
      <skos:member rdf:resource="egressLink"/>
      <skos:member rdf:resource="intersectionManoeuvre"/>
      <skos:member rdf:resource="junctionAtGrade"/>
      <skos:member rdf:resource="interchange"/>
    </skos:Collection>
    <skos:Collection rdf:about="facilityTerms">
      <skos:member rdf:resource="transportFacility"/>
      <skos:member rdf:resource="transportInfrastructure"/>
      <skos:member rdf:resource="bridge"/>
    </skos:Collection>
    <skos:Collection rdf:about="kerbsideUsageTerms">
      <skos:member rdf:resource="designatedParkingSpace"/>
      <skos:member rdf:resource="loadingArea"/>
      <skos:member rdf:resource="parkingSpace"/>
      <skos:member rdf:resource="parkingSpaceForPermitHolders"/>
      <skos:member rdf:resource="pick-upDrop-offArea"/>
    </skos:Collection>
    <skos:Collection rdf:about="roadEquipmentTerms">
      <skos:member rdf:resource="roadEquipment"/>
    </skos:Collection>
    <skos:Collection rdf:about="locationTypeTerms">
      <skos:member rdf:resource="location"/>
      <skos:member rdf:resource="spatialLocation"/>
      <skos:member rdf:resource="pointLocation"/>
      <skos:member rdf:resource="geographicPointLocation"/>
      <skos:member rdf:resource="linearLocation"/>
      <skos:member rdf:resource="areaLocation"/>
      <skos:member rdf:resource="geographicFeature"/>
      <skos:member rdf:resource="pointDestination"/>
      <skos:member rdf:resource="areaDestination"/>
      <skos:member rdf:resource="coordinateTuple"/>
    </skos:Collection>
    <skos:Collection rdf:about="locationReferencingTerms">
      <skos:member rdf:resource="locationReferencing"/>
      <skos:member rdf:resource="spatialReference"/>
      <skos:member rdf:resource="dynamicSpatialReference"/>
      <skos:member rdf:resource="pre-codedSpatialReference"/>
      <skos:member rdf:resource="linkLocation"/>
      <skos:member rdf:resource="geographicIdentifier"/>
      <skos:member rdf:resource="gazetteer"/>
      <skos:member rdf:resource="networkLocation"/>
      <skos:member rdf:resource="geographicDescriptor"/>
    </skos:Collection>
    <skos:Collection rdf:about="jurisdictionalTerms">
      <skos:member rdf:resource="campus"/>
      <skos:member rdf:resource="governmentalArea"/>
      <skos:member rdf:resource="isoNamedArea"/>
      <skos:member rdf:resource="jurisdiction"/>
      <skos:member rdf:resource="jurisdictionalArea"/>
      <skos:member rdf:resource="jurisdictionalBoundary"/>
      <skos:member rdf:resource="jurisdictionalEntity"/>
    </skos:Collection>
    <skos:Collection rdf:about="genericServiceTerms">
      <skos:member rdf:resource="service"/>
      <skos:member rdf:resource="serviceProvider"/>
      <skos:member rdf:resource="user"/>
    </skos:Collection>
    <skos:Collection rdf:about="transportServiceTerms">
      <skos:member rdf:resource="transportService"/>
      <skos:member rdf:resource="transportProvider"/>
      <skos:member rdf:resource="transportUser"/>
    </skos:Collection>
    <skos:Collection rdf:about="itsServiceTerms">
      <skos:member rdf:resource="itsService"/>
      <skos:member rdf:resource="itsServiceProvider"/>
      <skos:member rdf:resource="itsUser"/>
    </skos:Collection>
    <skos:Collection rdf:about="its-suServiceTerms">
      <skos:member rdf:resource="its-suService"/>
      <skos:member rdf:resource="its-suServiceProvider"/>
      <skos:member rdf:resource="its-suUser"/>
      <skos:member rdf:resource="its-suUserNeed"/>
    </skos:Collection>
    <skos:Collection rdf:about="transportServiceApplicationTerms">
      <skos:member rdf:resource="mobilityApp"/>
      <skos:member rdf:resource="b2cMobilitySharingApp"/>
      <skos:member rdf:resource="navigationApp"/>
      <skos:member rdf:resource="p2pMobilitySharingApp"/>
      <skos:member rdf:resource="ridesourcingApp"/>
      <skos:member rdf:resource="publicTransportApp"/>
      <skos:member rdf:resource="real-timeTravellerInformationApp"/>
      <skos:member rdf:resource="taxiHailingApp"/>
    </skos:Collection>
    <skos:Collection rdf:about="transport-relatedSharingTerms">
      <skos:member rdf:resource="publicTransport"/>
      <skos:member rdf:resource="sharedTransportService"/>
      <skos:member rdf:resource="sharedVehicleService"/>
      <skos:member rdf:resource="transportSharing"/>
    </skos:Collection>
    <skos:Collection rdf:about="contractualModelTerms">
      <skos:member rdf:resource="contractualModel"/>
      <skos:member rdf:resource="corporateCustomerModel"/>
      <skos:member rdf:resource="privateCustomerModel"/>
      <skos:member rdf:resource="governmentCustomerModel"/>
    </skos:Collection>
    <skos:Collection rdf:about="financialModelTerms">
      <skos:member rdf:resource="financialModel"/>
      <skos:member rdf:resource="commercial"/>
      <skos:member rdf:resource="public"/>
      <skos:member rdf:resource="cooperative"/>
      <skos:member rdf:resource="mutualBenefit"/>
      <skos:member rdf:resource="fractionalOwnership"/>
      <skos:member rdf:resource="private"/>
      <skos:member rdf:resource="membership-based"/>
    </skos:Collection>
    <skos:Collection rdf:about="operationalModelTerms">
      <skos:member rdf:resource="operationalModel"/>
      <skos:member rdf:resource="sequential"/>
      <skos:member rdf:resource="concurrent"/>
      <skos:member rdf:resource="fixedRoute"/>
      <skos:member rdf:resource="dynamicRoute"/>
    </skos:Collection>
    <skos:Collection rdf:about="networkModelTerms">
      <skos:member rdf:resource="networkModel"/>
      <skos:member rdf:resource="station-basedRoundtrip"/>
      <skos:member rdf:resource="station-basedOne-way"/>
    </skos:Collection>
    <skos:Collection rdf:about="sharedTransportServiceTerms">
      <skos:member rdf:resource="shuttleService"/>
      <skos:member rdf:resource="taxiService"/>
      <skos:member rdf:resource="taxi-shareService"/>
      <skos:member rdf:resource="rideshareService"/>
      <skos:member rdf:resource="ridesourcedService"/>
      <skos:member rdf:resource="ridesplitService"/>
    </skos:Collection>
    <skos:Collection rdf:about="sharedVehicleTerms">
      <skos:member rdf:resource="bikesharingService"/>
    </skos:Collection>
    <skos:Collection rdf:about="travellerTerms">
      <skos:member rdf:resource="traveller"/>
      <skos:member rdf:resource="roadUser"/>
      <skos:member rdf:resource="pedestrian"/>
      <skos:member rdf:resource="vulnerableRoadUser"/>
    </skos:Collection>
    <skos:Collection rdf:about="vehicleOccupantTerms">
      <skos:member rdf:resource="passenger"/>
      <skos:member rdf:resource="vehicleOccupant"/>
      <skos:member rdf:resource="driver"/>
      <skos:member rdf:resource="in-vehicleDriver"/>
    </skos:Collection>
    <skos:Collection rdf:about="vehicleComponentTerms">
      <skos:member rdf:resource="vehicle"/>
      <skos:member rdf:resource="motor"/>
      <skos:member rdf:resource="wheel"/>
      <skos:member rdf:resource="vehicleInputDevice"/>
      <skos:member rdf:resource="built-inVehicleInputDevice"/>
      <skos:member rdf:resource="nomadicVehicleInputDevice"/>
    </skos:Collection>
    <skos:Collection rdf:about="vehicleAttributeTerms">
      <skos:member rdf:resource="speed"/>
      <skos:member rdf:resource="designSpeed"/>
      <skos:member rdf:resource="anonymizedVehicleReference"/>
      <skos:member rdf:resource="vehicleEquipment"/>
      <skos:member rdf:resource="vehicleFuelType"/>
      <skos:member rdf:resource="vehicleIdentifier"/>
      <skos:member rdf:resource="vehicleLoadType"/>
      <skos:member rdf:resource="vehicleRegistrationPlateIdentifier"/>
      <skos:member rdf:resource="grossVehicleMass"/>
    </skos:Collection>
    <skos:Collection rdf:about="vehicleAutomationTerms">
      <skos:member rdf:resource="dynamicDrivingTask"/>
      <skos:member rdf:resource="operationalDesignDomain"/>
      <skos:member rdf:resource="fallback"/>
      <skos:member rdf:resource="fallback-readyUser"/>
      <skos:member rdf:resource="ddtPerformance-relevantSystemFailure"/>
      <skos:member rdf:resource="drivingAutomationSystem"/>
      <skos:member rdf:resource="driverSupportSystem"/>
      <skos:member rdf:resource="level1DrivingAutomation"/>
      <skos:member rdf:resource="level2DrivingAutomation"/>
      <skos:member rdf:resource="ads"/>
      <skos:member rdf:resource="level3Ads"/>
      <skos:member rdf:resource="level4Ads"/>
      <skos:member rdf:resource="level5Ads"/>
      <skos:member rdf:resource="conventionalVehicle"/>
      <skos:member rdf:resource="ads-equippedVehicle"/>
      <skos:member rdf:resource="dual-modeVehicle"/>
    </skos:Collection>
    <skos:Collection rdf:about="vehicleConnectivityTerms">
      <skos:member rdf:resource="off-grid"/>
      <skos:member rdf:resource="unconnected"/>
      <skos:member rdf:resource="disconnected"/>
    </skos:Collection>
    <skos:Collection rdf:about="vehicleSpeedTerms">
      <skos:member rdf:resource="ultra-low-speedVehicle"/>
      <skos:member rdf:resource="low-speedVehicle"/>
      <skos:member rdf:resource="moderatelyLow-speedVehicle"/>
      <skos:member rdf:resource="moderate-speedVehicle"/>
      <skos:member rdf:resource="moderatelyHigh-speedVehicle"/>
      <skos:member rdf:resource="high-speedVehicle"/>
      <skos:member rdf:resource="ultra-lowVehicleSpeed"/>
      <skos:member rdf:resource="lowVehicleSpeed"/>
      <skos:member rdf:resource="moderately-lowVehicleSpeed"/>
      <skos:member rdf:resource="moderateVehicleSpeed"/>
      <skos:member rdf:resource="moderately-highVehicleSpeed"/>
    </skos:Collection>
    <skos:Collection rdf:about="vehicleTypesEnvironmentTerms">
      <skos:member rdf:resource="roadVehicle"/>
      <skos:member rdf:resource="motorizedVehicle"/>
      <skos:member rdf:resource="motorVehicle"/>
      <skos:member rdf:resource="non-roadVehicle"/>
      <skos:member rdf:resource="roadCycle"/>
    </skos:Collection>
    <skos:Collection rdf:about="paymentTerms">
      <skos:member rdf:resource="paymentMeans"/>
      <skos:member rdf:resource="paymentMode"/>
    </skos:Collection>

    <owl:AnnotationProperty rdf:about="clause">
        <rdfs:label xml:lang="en">clause</rdfs:label>
        <rdfs:comment xml:lang="en">This property is used to identify the clause number of a concept within the document.</rdfs:comment>
        <rdfs:range rdf:resource="xsd:string"/>
    </owl:AnnotationProperty>
    
    <owl:AnnotationProperty rdf:about="altPrefLabel">
        <rdfs:label xml:lang="en">alternative preferred label</rdfs:label>
        <rdfs:comment xml:lang="en">This property is used to identify an alternative preferred label for a concept.</rdfs:comment>
        <rdfs:range rdf:resource="xsd:string"/>
    </owl:AnnotationProperty>
    
    

    <!-- 
    ///////////////////////////////////////////////////////////////////////////////////////
    //
    // Properties
    //
    ///////////////////////////////////////////////////////////////////////////////////////
     -->
    <owl:ObjectProperty rdf:about="acceptedBy">
        <rdfs:label xml:lang="en">accepted by</rdfs:label>
    </owl:ObjectProperty>

    <owl:ObjectProperty rdf:about="accessedBy">
        <rdfs:label xml:lang="en">accessed by</rdfs:label>
    </owl:ObjectProperty>

    <owl:ObjectProperty rdf:about="aggregates">
    </owl:ObjectProperty>

    <owl:ObjectProperty rdf:about="along">
    </owl:ObjectProperty>

    <owl:ObjectProperty rdf:about="annotatedOutlineFor">
        <rdfs:label xml:lang="en">annotated outline for</rdfs:label>
    </owl:ObjectProperty>

    <owl:ObjectProperty rdf:about="areaAbove">
        <rdfs:label xml:lang="en">area above</rdfs:label>
    </owl:ObjectProperty>

    <owl:ObjectProperty rdf:about="basedOn">
        <rdfs:label xml:lang="en">based on</rdfs:label>
    </owl:ObjectProperty>

    <owl:ObjectProperty rdf:about="canBe">
        <rdfs:label xml:lang="en">can be</rdfs:label>
    </owl:ObjectProperty>

    <owl:ObjectProperty rdf:about="canControl">
        <rdfs:label xml:lang="en">can control</rdfs:label>
    </owl:ObjectProperty>

    <owl:ObjectProperty rdf:about="changesPropertyOf">
        <rdfs:label xml:lang="en">changes property of</rdfs:label>
    </owl:ObjectProperty>

    <owl:ObjectProperty rdf:about="characteristicOf">
        <rdfs:label xml:lang="en">characteristic of</rdfs:label>
    </owl:ObjectProperty>

    <owl:ObjectProperty rdf:about="comprises">
    </owl:ObjectProperty>

    <owl:ObjectProperty rdf:about="connects">
    </owl:ObjectProperty>

    <owl:ObjectProperty rdf:about="constitutes">
    </owl:ObjectProperty>

    <owl:ObjectProperty rdf:about="containedIn">
        <rdfs:label xml:lang="en">contained in</rdfs:label>
    </owl:ObjectProperty>

    <owl:ObjectProperty rdf:about="contains">
    </owl:ObjectProperty>

    <owl:ObjectProperty rdf:about="contentsOf">
        <rdfs:label xml:lang="en">contents of</rdfs:label>
    </owl:ObjectProperty>

    <owl:ObjectProperty rdf:about="conventionsPrinciplesAndPracticesFor">
        <rdfs:label xml:lang="en">conventions, principles, and practices for</rdfs:label>
    </owl:ObjectProperty>

    <owl:ObjectProperty rdf:about="ddtControlledBy">
        <rdfs:label xml:lang="en">DDT controlled by</rdfs:label>
    </owl:ObjectProperty>

    <owl:ObjectProperty rdf:about="definesHowToProvide">
        <rdfs:label xml:lang="en">defines how to provide</rdfs:label>
    </owl:ObjectProperty>

    <owl:ObjectProperty rdf:about="delivers">
    </owl:ObjectProperty>

    <owl:ObjectProperty rdf:about="describedBy">
        <rdfs:label xml:lang="en">described by</rdfs:label>
    </owl:ObjectProperty>

    <owl:ObjectProperty rdf:about="describes">
    </owl:ObjectProperty>

    <owl:ObjectProperty rdf:about="designates">
    </owl:ObjectProperty>

    <owl:ObjectProperty rdf:about="designedFor">
        <rdfs:label xml:lang="en">designed for</rdfs:label>
    </owl:ObjectProperty>

    <owl:ObjectProperty rdf:about="designedToBenefit">
        <rdfs:label xml:lang="en">designed to benefit</rdfs:label>
    </owl:ObjectProperty>

    <owl:ObjectProperty rdf:about="designedWithExpectationOf">
        <rdfs:label xml:lang="en">designed with expectation of</rdfs:label>
    </owl:ObjectProperty>

    <owl:ObjectProperty rdf:about="desireToTransport">
        <rdfs:label xml:lang="en">desire to transport</rdfs:label>
    </owl:ObjectProperty>

    <owl:ObjectProperty rdf:about="desiredResultsOf">
        <rdfs:label xml:lang="en">desired results of</rdfs:label>
    </owl:ObjectProperty>

    <owl:ObjectProperty rdf:about="details">
    </owl:ObjectProperty>

    <owl:ObjectProperty rdf:about="elementIn">
        <rdfs:label xml:lang="en">element in</rdfs:label>
    </owl:ObjectProperty>

    <owl:ObjectProperty rdf:about="encodedReferenceFor">
        <rdfs:label xml:lang="en">encoded reference for</rdfs:label>
    </owl:ObjectProperty>

    <owl:ObjectProperty rdf:about="endsAt">
        <rdfs:label xml:lang="en">ends at</rdfs:label>
    </owl:ObjectProperty>

    <owl:ObjectProperty rdf:about="entryFor">
        <rdfs:label xml:lang="en">entry for</rdfs:label>
    </owl:ObjectProperty>

    <owl:ObjectProperty rdf:about="exhibits">
    </owl:ObjectProperty>

    <owl:ObjectProperty rdf:about="exitFor">
        <rdfs:label xml:lang="en">exit for</rdfs:label>
    </owl:ObjectProperty>

    <owl:ObjectProperty rdf:about="expresses">
    </owl:ObjectProperty>

    <owl:ObjectProperty rdf:about="extentOf">
        <rdfs:label xml:lang="en">extent of</rdfs:label>
    </owl:ObjectProperty>

    <owl:ObjectProperty rdf:about="for">
    </owl:ObjectProperty>

    <owl:ObjectProperty rdf:about="forAGiven">
        <rdfs:label xml:lang="en">for a given</rdfs:label>
    </owl:ObjectProperty>

    <owl:ObjectProperty rdf:about="forDesignated">
        <rdfs:label xml:lang="en">for designated</rdfs:label>
    </owl:ObjectProperty>

    <owl:ObjectProperty rdf:about="forMovementOf">
        <rdfs:label xml:lang="en">for movement of</rdfs:label>
    </owl:ObjectProperty>

    <owl:ObjectProperty rdf:about="frames">
    </owl:ObjectProperty>

    <owl:ObjectProperty rdf:about="from">
    </owl:ObjectProperty>

    <owl:ObjectProperty rdf:about="fuelUsedBy">
        <rdfs:label xml:lang="en">fuel used by</rdfs:label>
    </owl:ObjectProperty>

    <owl:ObjectProperty rdf:about="fulfils">
    </owl:ObjectProperty>

    <owl:ObjectProperty rdf:about="globallyUniqueIdentifierFor">
        <rdfs:label xml:lang="en">globally unique identifier for</rdfs:label>
    </owl:ObjectProperty>

    <owl:ObjectProperty rdf:about="governs">
    </owl:ObjectProperty>

    <owl:ObjectProperty rdf:about="groups">
    </owl:ObjectProperty>

    <owl:ObjectProperty rdf:about="has">
    </owl:ObjectProperty>

    <owl:ObjectProperty rdf:about="helpsIdentify">
        <rdfs:label xml:lang="en">helps identify</rdfs:label>
    </owl:ObjectProperty>

    <owl:ObjectProperty rdf:about="identifierUniqueWithinRegionFor">
        <rdfs:label xml:lang="en">identifier unique within region for</rdfs:label>
    </owl:ObjectProperty>

    <owl:ObjectProperty rdf:about="identifies">
    </owl:ObjectProperty>

    <owl:ObjectProperty rdf:about="implementationOf">
        <rdfs:label xml:lang="en">implementation of</rdfs:label>
    </owl:ObjectProperty>

    <owl:ObjectProperty rdf:about="implements">
    </owl:ObjectProperty>

    <owl:ObjectProperty rdf:about="inUseOrOnBoard">
        <rdfs:label xml:lang="en">in use or on board</rdfs:label>
    </owl:ObjectProperty>

    <owl:ObjectProperty rdf:about="installationOf">
        <rdfs:label xml:lang="en">installation of</rdfs:label>
    </owl:ObjectProperty>

    <owl:ObjectProperty rdf:about="instantiationOf">
        <rdfs:label xml:lang="en">instantiation of</rdfs:label>
    </owl:ObjectProperty>

    <owl:ObjectProperty rdf:about="involves">
    </owl:ObjectProperty>

    <owl:ObjectProperty rdf:about="is">
    </owl:ObjectProperty>

    <owl:ObjectProperty rdf:about="isA">
        <rdfs:label xml:lang="en">is a</rdfs:label>
    </owl:ObjectProperty>

    <owl:ObjectProperty rdf:about="isIn">
        <rdfs:label xml:lang="en">is in</rdfs:label>
    </owl:ObjectProperty>

    <owl:ObjectProperty rdf:about="isRequiredToOperate">
        <rdfs:label xml:lang="en">is required to operate</rdfs:label>
    </owl:ObjectProperty>

    <owl:ObjectProperty rdf:about="limitOf">
        <rdfs:label xml:lang="en">limit of</rdfs:label>
    </owl:ObjectProperty>

    <owl:ObjectProperty rdf:about="loadCarriedBy">
        <rdfs:label xml:lang="en">load carried by</rdfs:label>
    </owl:ObjectProperty>

    <owl:ObjectProperty rdf:about="locatedWithin">
        <rdfs:label xml:lang="en">located within</rdfs:label>
    </owl:ObjectProperty>

    <owl:ObjectProperty rdf:about="maxOperatingWeightFor">
        <rdfs:label xml:lang="en">max operating weight for</rdfs:label>
    </owl:ObjectProperty>

    <owl:ObjectProperty rdf:about="maximumSustainedSpeedOf">
        <rdfs:label xml:lang="en">maximum sustained speed of</rdfs:label>
    </owl:ObjectProperty>

    <owl:ObjectProperty rdf:about="mayBeCausedBy">
        <rdfs:label xml:lang="en">may be caused by</rdfs:label>
    </owl:ObjectProperty>

    <owl:ObjectProperty rdf:about="mayBeCausedByAViolationOf">
        <rdfs:label xml:lang="en">may be caused by a violation of</rdfs:label>
    </owl:ObjectProperty>

    <owl:ObjectProperty rdf:about="meetingOrCrossing">
        <rdfs:label xml:lang="en">meeting or crossing</rdfs:label>
    </owl:ObjectProperty>

    <owl:ObjectProperty rdf:about="meetsRequirementsOf">
        <rdfs:label xml:lang="en">meets requirements of</rdfs:label>
    </owl:ObjectProperty>

    <owl:ObjectProperty rdf:about="observesPropertyOf">
        <rdfs:label xml:lang="en">observes property of</rdfs:label>
    </owl:ObjectProperty>

    <owl:ObjectProperty rdf:about="operatesWithinA">
        <rdfs:label xml:lang="en">operates within a</rdfs:label>
    </owl:ObjectProperty>

    <owl:ObjectProperty rdf:about="operatingMassOf">
        <rdfs:label xml:lang="en">operating mass of</rdfs:label>
    </owl:ObjectProperty>

    <owl:ObjectProperty rdf:about="operatingModeOf">
        <rdfs:label xml:lang="en">operating mode of</rdfs:label>
    </owl:ObjectProperty>

    <owl:ObjectProperty rdf:about="performsAllOf">
        <rdfs:label xml:lang="en">performs all of</rdfs:label>
    </owl:ObjectProperty>

    <owl:ObjectProperty rdf:about="performsInformationProcessingFor">
        <rdfs:label xml:lang="en">performs information processing for</rdfs:label>
    </owl:ObjectProperty>

    <owl:ObjectProperty rdf:about="performsPartOf">
        <rdfs:label xml:lang="en">performs part of</rdfs:label>
    </owl:ObjectProperty>

    <owl:ObjectProperty rdf:about="performsPartOrAllOf">
        <rdfs:label xml:lang="en">performs part or all of</rdfs:label>
    </owl:ObjectProperty>

    <owl:ObjectProperty rdf:about="processToDevelop">
        <rdfs:label xml:lang="en">process to develop</rdfs:label>
    </owl:ObjectProperty>

    <owl:ObjectProperty rdf:about="providesItsOwn">
        <rdfs:label xml:lang="en">provides its own</rdfs:label>
    </owl:ObjectProperty>

    <owl:ObjectProperty rdf:about="rateOfChangeOfPositionOf">
        <rdfs:label xml:lang="en">rate of change of position of</rdfs:label>
    </owl:ObjectProperty>

    <owl:ObjectProperty rdf:about="readyToPerform">
        <rdfs:label xml:lang="en">ready to perform</rdfs:label>
    </owl:ObjectProperty>

    <owl:ObjectProperty rdf:about="realizationOf">
        <rdfs:label xml:lang="en">realization of</rdfs:label>
    </owl:ObjectProperty>

    <owl:ObjectProperty rdf:about="referenceUsedBy">
        <rdfs:label xml:lang="en">reference used by</rdfs:label>
    </owl:ObjectProperty>

    <owl:ObjectProperty rdf:about="representedBy">
        <rdfs:label xml:lang="en">represented by</rdfs:label>
    </owl:ObjectProperty>

    <owl:ObjectProperty rdf:about="represents">
    </owl:ObjectProperty>

    <owl:ObjectProperty rdf:about="requiresProcessingWithin">
        <rdfs:label xml:lang="en">requires processing within</rdfs:label>
    </owl:ObjectProperty>

    <owl:ObjectProperty rdf:about="residesIn">
        <rdfs:label xml:lang="en">resides in</rdfs:label>
    </owl:ObjectProperty>

    <owl:ObjectProperty rdf:about="rulesDefinedBy">
        <rdfs:label xml:lang="en">rules defined by</rdfs:label>
    </owl:ObjectProperty>

    <owl:ObjectProperty rdf:about="sentFrom">
        <rdfs:label xml:lang="en">sent from</rdfs:label>
    </owl:ObjectProperty>

    <owl:ObjectProperty rdf:about="sentTo">
        <rdfs:label xml:lang="en">sent to</rdfs:label>
    </owl:ObjectProperty>

    <owl:ObjectProperty rdf:about="situatedIn">
        <rdfs:label xml:lang="en">situated in</rdfs:label>
    </owl:ObjectProperty>

    <owl:ObjectProperty rdf:about="specificationOf">
        <rdfs:label xml:lang="en">specification of</rdfs:label>
    </owl:ObjectProperty>

    <owl:ObjectProperty rdf:about="startsAt">
        <rdfs:label xml:lang="en">starts at</rdfs:label>
    </owl:ObjectProperty>

    <owl:ObjectProperty rdf:about="store">
    </owl:ObjectProperty>

    <owl:ObjectProperty rdf:about="storedIn">
        <rdfs:label xml:lang="en">stored in</rdfs:label>
    </owl:ObjectProperty>

    <owl:ObjectProperty rdf:about="systemOf">
        <rdfs:label xml:lang="en">system of</rdfs:label>
    </owl:ObjectProperty>

    <owl:ObjectProperty rdf:about="timingAndLocationOfRemunerationTo">
        <rdfs:label xml:lang="en">timing and location of remuneration to</rdfs:label>
    </owl:ObjectProperty>

    <owl:ObjectProperty rdf:about="to">
    </owl:ObjectProperty>

    <owl:ObjectProperty rdf:about="toBoardOrAlightFrom">
        <rdfs:label xml:lang="en">to board or alight from</rdfs:label>
    </owl:ObjectProperty>

    <owl:ObjectProperty rdf:about="transports">
    </owl:ObjectProperty>

    <owl:ObjectProperty rdf:about="travellingIn">
        <rdfs:label xml:lang="en">travelling in</rdfs:label>
    </owl:ObjectProperty>

    <owl:ObjectProperty rdf:about="uses">
    </owl:ObjectProperty>

    <owl:ObjectProperty rdf:about="using">
    </owl:ObjectProperty>





    <!-- 
    ///////////////////////////////////////////////////////////////////////////////////////
    //
    // Classes
    //
    ///////////////////////////////////////////////////////////////////////////////////////
     -->

    <owl:Class rdf:about="entity">
        <clause>3.1.1.1</clause>
        <skos:prefLabel xml:lang="en">entity</skos:prefLabel>
        <skos:definition>concrete or abstract thing that exists, did exist, or can possibly exist,
            including associations among these things</skos:definition>
        <skos:example>Person (3.1.1.6), object, event, idea, process, etc.</skos:example>
        <skos:historyNote>Introduced in ISO/TS 14812:2022</skos:historyNote>
    </owl:Class>
    <owl:Class rdf:about="immaterialEntity">
        <clause>3.1.1.2</clause>
        <skos:prefLabel xml:lang="en">immaterial entity</skos:prefLabel>
        <skos:definition>entity (3.1.1.1) that does not occupy three-dimensional space</skos:definition>
        <skos:example>Idea, process, organization, etc.</skos:example>
        <rdfs:subClassOf rdf:resource="entity"/>
        <skos:historyNote>Introduced in ISO/TS 14812:2022</skos:historyNote>
    </owl:Class>
    <owl:Class rdf:about="materialEntity">
        <clause>3.1.1.3</clause>
        <skos:prefLabel xml:lang="en">material entity</skos:prefLabel>
        <skos:definition>entity (3.1.1.1) that occupies three-dimensional space</skos:definition>
        <skos:note>All material entities have certain characteristics that can be
            described and therefore this concept is important for ontology purposes.</skos:note>
        <rdfs:subClassOf rdf:resource="entity"/>
        <skos:historyNote>Introduced in ISO/TS 14812:2022</skos:historyNote>
    </owl:Class>
    <owl:Class rdf:about="non-biologicalEntity">
        <clause>3.1.1.4</clause>
        <skos:prefLabel xml:lang="en">non-biological entity</skos:prefLabel>
        <skos:definition>material entity (3.1.1.3) that is not and has never been a living organism</skos:definition>
        <rdfs:subClassOf rdf:resource="materialEntity"/>
        <skos:historyNote>Introduced in ISO/TS 14812:2022</skos:historyNote>
    </owl:Class>
    <owl:Class rdf:about="biologicalEntity">
        <clause>3.1.1.5</clause>
        <skos:prefLabel xml:lang="en">biological entity</skos:prefLabel>
        <skos:definition>material entity (3.1.1.3) that was or is a living organism</skos:definition>
        <rdfs:subClassOf rdf:resource="materialEntity"/>
        <skos:historyNote>Introduced in ISO/TS 14812:2022</skos:historyNote>
    </owl:Class>
    <owl:Class rdf:about="person">
        <clause>3.1.1.6</clause>
        <skos:prefLabel xml:lang="en">person</skos:prefLabel>
        <skos:definition>biological entity (3.1.1.5) that is a human being</skos:definition>
        <rdfs:subClassOf rdf:resource="biologicalEntity"/>
        <skos:historyNote>Introduced in ISO/TS 14812:2022</skos:historyNote>
    </owl:Class>
    <owl:Class rdf:about="system">
        <clause>3.1.2.1</clause>
        <skos:prefLabel xml:lang="en">system</skos:prefLabel>
        <skos:definition>combination of interacting elements (3.1.3.10) organized to achieve one or
            more stated purposes</skos:definition>
        <dcterms:source>ISO/IEC/IEEE 15288:2015, 4.1.46, modified - Notes to entry
            removed.</dcterms:source>
        <rdfs:subClassOf>
            <owl:Restriction>
                <owl:onProperty rdf:resource="situatedIn"/>
                <owl:someValuesFrom rdf:resource="environment"/>
            </owl:Restriction>
        </rdfs:subClassOf>
        <rdfs:subClassOf>
            <owl:Restriction>
                <owl:onProperty rdf:resource="exhibits"/>
                <owl:someValuesFrom rdf:resource="architecture"/>
            </owl:Restriction>
        </rdfs:subClassOf>
        <rdfs:subClassOf>
            <owl:Restriction>
                <owl:onProperty rdf:resource="designedFor"/>
                <owl:someValuesFrom rdf:resource="user"/>
            </owl:Restriction>
        </rdfs:subClassOf>
        <skos:historyNote>Introduced in ISO/TS 14812:2022</skos:historyNote>
    </owl:Class>
    <owl:Class rdf:about="transportSystem">
        <clause>3.1.2.2</clause>
        <skos:prefLabel xml:lang="en">transport system</skos:prefLabel>
        <skos:definition>system (3.1.2.1) of infrastructure elements (3.1.3.10) and optionally
            vehicles (3.7.1.1) that are jointly designed to move material entities (3.1.1.3) from an
            origin to a destination</skos:definition>
        <skos:note>Transport systems can also include any supporting system, such
            as information and control systems.</skos:note>
        <rdfs:subClassOf rdf:resource="system"/>
        <skos:historyNote>Introduced in ISO/TS 14812:2022</skos:historyNote>
    </owl:Class>
    <owl:Class rdf:about="surfaceTransportSystem">
        <clause>3.1.2.3</clause>
        <skos:prefLabel xml:lang="en">surface transport system</skos:prefLabel>
        <skos:altLabel xml:lang="en">transport system</skos:altLabel>
        <skos:definition>transport system (3.1.2.2) designed to move material entities (3.1.1.3)
            across the surface or near-surface of the Earth</skos:definition>
        <skos:note>A surface transport system can include tunnels, bridges and
            similar elements (3.1.3.10).</skos:note>
        <skos:note>There is not complete agreement on the precise limitations of a
            "surface transport system" within the ITS community. Currently, the term is almost
            exclusively applied to ground-based travel of goods and people over significant
            distances. The term is viewed as including ferry systems, which often form an integral
            part of a local surface transport system; it is less clear if it includes long-distance
            sea-fairing ships. The term "surface transport systems" is also generally limited to
            transport systems that cover a considerable distance (e.g. factory conveyance
            technologies are not often referred to as "surface transport systems"). It has been
            suggested that air travel, which is arguably a transport system designed to move
            physical entities between points on the surface of the earth, ought to be included in
            the scope of the term, but this perspective is not universally accepted. It is expected
            that the exact limitations of the term will be further refined as ITS matures.</skos:note>
        <skos:note>Due to the defined scope of ITS, the term "transport system" is
            intended to be interpreted as being synonymous with the term "surface transport system"
            unless explicitly specified otherwise.</skos:note>
        <rdfs:subClassOf rdf:resource="transportSystem"/>
        <skos:historyNote>Introduced in ISO/TS 14812:2022</skos:historyNote>
    </owl:Class>
    <owl:Class rdf:about="intelligentTransportSystem">
        <clause>3.1.2.4</clause>
        <skos:prefLabel xml:lang="en">intelligent transport system</skos:prefLabel>
        <altPrefLabel xml:lang="en">ITS</altPrefLabel>
        <skos:altLabel xml:lang="en">intelligent transportation system</skos:altLabel>
        <skos:definition>system (3.1.2.1) comprised of information, communication, sensor and
            control technologies and that is designed to benefit a surface transport system
            (3.1.2.3)</skos:definition>
        <skos:note>"Intelligent transportation system" is the American English
            equivalent.</skos:note>
        <skos:note>Benefits potentially include, but are not limited to, increased
            safety, sustainability, efficiency and comfort.</skos:note>
        <skos:note>The full term (i.e. "intelligent transport system") is often
            used when the noun is used as a subject, whereas the abbreviation (i.e. "ITS") is often
            used to modify another noun (e.g. "Intelligent transport systems provide ITS
            services.").</skos:note>
        <rdfs:subClassOf rdf:resource="system"/>
        <rdfs:subClassOf>
            <owl:Restriction>
                <owl:onProperty rdf:resource="designedToBenefit"/>
                <owl:someValuesFrom rdf:resource="surfaceTransportSystem"/>
            </owl:Restriction>
        </rdfs:subClassOf>
        <skos:historyNote>Introduced in ISO/TS 14812:2022</skos:historyNote>
    </owl:Class>
    <owl:Class rdf:about="cooperativeIts">
        <clause>3.1.2.5</clause>
        <skos:prefLabel xml:lang="en">cooperative ITS</skos:prefLabel>
        <altPrefLabel xml:lang="en">C-ITS</altPrefLabel>
        <skos:definition>subset of ITS (3.1.2.4) where information is shared among ITS stations
            (3.2.7.3) in a manner that enables its use by multiple ITS services (3.5.3.1)</skos:definition>
        <rdfs:subClassOf rdf:resource="intelligentTransportSystem"/>
        <skos:historyNote>Introduced in ISO/TS 14812:2022</skos:historyNote>
    </owl:Class>
    <owl:Class rdf:about="architecture">
        <clause>3.1.3.1</clause>
        <skos:prefLabel xml:lang="en">architecture</skos:prefLabel>
        <altPrefLabel xml:lang="en">system architecture</altPrefLabel>
        <skos:definition>&lt;system&gt; fundamental concepts or properties of a system (3.1.2.1) in
            its environment (3.1.3.11) embodied in its elements (3.1.3.10), relationships (3.1.6.8)
            and in the principles of its design and evolution</skos:definition>
        <dcterms:source>ISO/IEC/IEEE 42010:2011, 3.2</dcterms:source>
        <rdfs:subClassOf>
            <owl:Restriction>
                <owl:onProperty rdf:resource="aggregates"/>
                <owl:someValuesFrom rdf:resource="element"/>
            </owl:Restriction>
        </rdfs:subClassOf>
        <skos:historyNote>Introduced in ISO/TS 14812:2022</skos:historyNote>
    </owl:Class>
    <owl:Class rdf:about="architectureDescription">
        <clause>3.1.3.2</clause>
        <skos:prefLabel xml:lang="en">architecture description</skos:prefLabel>
        <skos:definition>work product used to express an architecture (3.1.3.1)</skos:definition>
        <dcterms:source>ISO/IEC/IEEE 42010:2011, 3.3</dcterms:source>
        <rdfs:subClassOf>
            <owl:Restriction>
                <owl:onProperty rdf:resource="expresses"/>
                <owl:someValuesFrom rdf:resource="architecture"/>
            </owl:Restriction>
        </rdfs:subClassOf>
        <rdfs:subClassOf>
            <owl:Restriction>
                <owl:onProperty rdf:resource="identifies"/>
                <owl:someValuesFrom rdf:resource="system"/>
            </owl:Restriction>
        </rdfs:subClassOf>
        <rdfs:subClassOf>
            <owl:Restriction>
                <owl:onProperty rdf:resource="identifies"/>
                <owl:someValuesFrom rdf:resource="stakeholder"/>
            </owl:Restriction>
        </rdfs:subClassOf>
        <rdfs:subClassOf>
            <owl:Restriction>
                <owl:onProperty rdf:resource="identifies"/>
                <owl:someValuesFrom rdf:resource="concern"/>
            </owl:Restriction>
        </rdfs:subClassOf>
        <rdfs:subClassOf>
            <owl:Restriction>
                <owl:onProperty rdf:resource="aggregates"/>
                <owl:someValuesFrom rdf:resource="architectureView"/>
            </owl:Restriction>
        </rdfs:subClassOf>
        <rdfs:subClassOf>
            <owl:Restriction>
                <owl:onProperty rdf:resource="aggregates"/>
                <owl:someValuesFrom rdf:resource="architectureViewpoint"/>
            </owl:Restriction>
        </rdfs:subClassOf>
        <skos:historyNote>Introduced in ISO/TS 14812:2022</skos:historyNote>
    </owl:Class>
    <owl:Class rdf:about="architectureFramework">
        <clause>3.1.3.3</clause>
        <skos:prefLabel xml:lang="en">architecture framework</skos:prefLabel>
        <skos:definition>conventions, principles and practices for the description of architectures
            (3.1.3.1) established within a specific domain of application and/or community of
            stakeholders (3.1.3.4)</skos:definition>
        <skos:example>Generalised Enterprise Reference Architecture and Methodologies
            (GERAM) [ISO 15704] is an architecture framework.</skos:example>
        <skos:example>Reference Model of Open Distributed Processing (RM-ODP) [ISO/IEC
            10746] is an architecture framework.</skos:example>
        <dcterms:source>ISO/IEC/IEEE 42010:2011, 3.4</dcterms:source>
        <rdfs:subClassOf>
            <owl:Restriction>
                <owl:onProperty rdf:resource="conventionsPrinciplesAndPracticesFor"/>
                <owl:someValuesFrom rdf:resource="architectureDescription"/>
            </owl:Restriction>
        </rdfs:subClassOf>
        <skos:historyNote>Introduced in ISO/TS 14812:2022</skos:historyNote>
    </owl:Class>
    <owl:Class rdf:about="stakeholder">
        <clause>3.1.3.4</clause>
        <skos:prefLabel xml:lang="en">stakeholder</skos:prefLabel>
        <altPrefLabel xml:lang="en">system stakeholder</altPrefLabel>
        <skos:definition>&lt;system&gt; individual, team, organization, or classes (3.1.12.2)
            thereof, having an interest in a system (3.1.2.1)</skos:definition>
        <dcterms:source>ISO/IEC/IEEE 42010:2011, 3.10</dcterms:source>
        <rdfs:subClassOf>
            <owl:Restriction>
                <owl:onProperty rdf:resource="has"/>
                <owl:someValuesFrom rdf:resource="concern"/>
            </owl:Restriction>
        </rdfs:subClassOf>
        <skos:historyNote>Introduced in ISO/TS 14812:2022</skos:historyNote>
    </owl:Class>
    <owl:Class rdf:about="concern">
        <clause>3.1.3.5</clause>
        <skos:prefLabel xml:lang="en">concern</skos:prefLabel>
        <altPrefLabel xml:lang="en">system concern</altPrefLabel>
        <skos:definition>&lt;system&gt; interest in a system (3.1.2.1) relevant to one or more of
            its stakeholders (3.1.3.4)</skos:definition>
        <skos:note>A concern pertains to any influence on a system in its
            environment (3.1.3.11), including developmental, technological, business, operational,
            organizational, political, economic, legal, regulatory, ecological and social
            influences.</skos:note>
        <dcterms:source>ISO/IEC/IEEE 42010:2011, 3.7</dcterms:source>
        <skos:historyNote>Introduced in ISO/TS 14812:2022</skos:historyNote>
    </owl:Class>
    <owl:Class rdf:about="architectureViewpoint">
        <clause>3.1.3.6</clause>
        <skos:prefLabel xml:lang="en">architecture viewpoint</skos:prefLabel>
        <skos:definition>work product establishing the conventions for the construction,
            interpretation and use of architecture views (3.1.3.7) to frame specific system concerns
            (3.1.3.5)</skos:definition>
        <dcterms:source>ISO/IEC/IEEE 42010:2011, 3.6</dcterms:source>
        <rdfs:subClassOf>
            <owl:Restriction>
                <owl:onProperty rdf:resource="aggregates"/>
                <owl:someValuesFrom rdf:resource="modelKind"/>
            </owl:Restriction>
        </rdfs:subClassOf>
        <rdfs:subClassOf>
            <owl:Restriction>
                <owl:onProperty rdf:resource="frames"/>
                <owl:someValuesFrom rdf:resource="concern"/>
            </owl:Restriction>
        </rdfs:subClassOf>
        <rdfs:subClassOf>
            <owl:Restriction>
                <owl:onProperty rdf:resource="governs"/>
                <owl:someValuesFrom rdf:resource="architectureView"/>
            </owl:Restriction>
        </rdfs:subClassOf>
        <skos:historyNote>Introduced in ISO/TS 14812:2022</skos:historyNote>
    </owl:Class>
    <owl:Class rdf:about="architectureView">
        <clause>3.1.3.7</clause>
        <skos:prefLabel xml:lang="en">architecture view</skos:prefLabel>
        <skos:definition>work product expressing the architecture (3.1.3.1) of a system (3.1.2.1)
            from the perspective of specific system concerns (3.1.3.5)</skos:definition>
        <dcterms:source>ISO/IEC/IEEE 42010:2011, 3.5</dcterms:source>
        <rdfs:subClassOf>
            <owl:Restriction>
                <owl:onProperty rdf:resource="aggregates"/>
                <owl:someValuesFrom rdf:resource="architectureModel"/>
            </owl:Restriction>
        </rdfs:subClassOf>
        <skos:historyNote>Introduced in ISO/TS 14812:2022</skos:historyNote>
    </owl:Class>
    <owl:Class rdf:about="modelKind">
        <clause>3.1.3.8</clause>
        <skos:prefLabel xml:lang="en">model kind</skos:prefLabel>
        <skos:definition>conventions for a type of modelling</skos:definition>
        <skos:note>Examples of model kinds include data flow (3.1.7.1) diagrams,
            class (3.1.11.2) diagrams, Petri nets, balance sheets, organization charts and state
            transition models.</skos:note>
        <dcterms:source>ISO/IEC/IEEE 42010:2011, 3.9</dcterms:source>
        <rdfs:subClassOf>
            <owl:Restriction>
                <owl:onProperty rdf:resource="governs"/>
                <owl:someValuesFrom rdf:resource="architectureModel"/>
            </owl:Restriction>
        </rdfs:subClassOf>
        <skos:historyNote>Introduced in ISO/TS 14812:2022</skos:historyNote>
    </owl:Class>
    <owl:Class rdf:about="architectureModel">
        <clause>3.1.3.9</clause>
        <skos:prefLabel xml:lang="en">architecture model</skos:prefLabel>
        <skos:definition>work product representing one or more architecture views (3.1.3.7) and
            expressed in a format governed by a model kind (3.1.3.8)</skos:definition>
        <skos:historyNote>Introduced in ISO/TS 14812:2022</skos:historyNote>
    </owl:Class>
    <owl:Class rdf:about="element">
        <clause>3.1.3.10</clause>
        <skos:prefLabel xml:lang="en">element</skos:prefLabel>
        <altPrefLabel xml:lang="en">architecture element</altPrefLabel>
        <skos:definition>&lt;architecture&gt; component member of an architecture model (3.1.3.9)
            included in an architecture view (3.1.3.7)</skos:definition>
        <skos:historyNote>Introduced in ISO/TS 14812:2022</skos:historyNote>
    </owl:Class>
    <owl:Class rdf:about="environment">
        <clause>3.1.3.11</clause>
        <skos:prefLabel xml:lang="en">environment</skos:prefLabel>
        <altPrefLabel xml:lang="en">system environment</altPrefLabel>
        <skos:definition>&lt;system&gt; context determining the setting and circumstances of all
            influences upon a system (3.1.2.1)</skos:definition>
        <skos:note>The environment of a system includes developmental,
            technological, business, operational, organizational, political, economic, legal,
            regulatory, ecological and social influences.</skos:note>
        <dcterms:source>ISO/IEC/IEEE 42010:2011, 3.8</dcterms:source>
        <skos:historyNote>Introduced in ISO/TS 14812:2022</skos:historyNote>
    </owl:Class>
    <owl:Class rdf:about="communicationsView">
        <clause>3.1.4.1</clause>
        <skos:prefLabel xml:lang="en">communications view</skos:prefLabel>
        <skos:definition>architecture view (3.1.3.7) from the communications viewpoint (3.1.4.2)</skos:definition>
        <skos:note>Within ITS, the preferred model for describing the
            communications view is based on the ITS-S reference architecture (3.1.9.4).</skos:note>
        <rdfs:subClassOf rdf:resource="architectureView"/>
        <rdfs:subClassOf>
            <owl:Restriction>
                <owl:onProperty rdf:resource="basedOn"/>
                <owl:someValuesFrom rdf:resource="its-sReferenceArchitecture"/>
            </owl:Restriction>
        </rdfs:subClassOf>
        <skos:historyNote>Introduced in ISO/TS 14812:2022</skos:historyNote>
    </owl:Class>
    <owl:Class rdf:about="communicationsViewpoint">
        <clause>3.1.4.2</clause>
        <skos:prefLabel xml:lang="en">communications viewpoint</skos:prefLabel>
        <skos:definition>architecture viewpoint (3.1.3.6) used to frame concerns (3.1.3.5) related
            to all layers of the Open Systems Interconnection (OSI) stack and related management and
            security issues</skos:definition>
        <rdfs:subClassOf rdf:resource="architectureViewpoint"/>
        <rdfs:subClassOf>
            <owl:Restriction>
                <owl:onProperty rdf:resource="governs"/>
                <owl:someValuesFrom rdf:resource="communicationsView"/>
            </owl:Restriction>
        </rdfs:subClassOf>
        <skos:historyNote>Introduced in ISO/TS 14812:2022</skos:historyNote>
    </owl:Class>
    <owl:Class rdf:about="enterpriseView">
        <clause>3.1.4.3</clause>
        <skos:prefLabel xml:lang="en">enterprise view</skos:prefLabel>
        <skos:definition>architecture view (3.1.3.7) from the enterprise viewpoint (3.1.4.4)</skos:definition>
        <rdfs:subClassOf rdf:resource="architectureView"/>
        <rdfs:subClassOf>
            <owl:Restriction>
                <owl:onProperty rdf:resource="aggregates"/>
                <owl:someValuesFrom rdf:resource="enterpriseObject"/>
            </owl:Restriction>
        </rdfs:subClassOf>
        <rdfs:subClassOf>
            <owl:Restriction>
                <owl:onProperty rdf:resource="aggregates"/>
                <owl:someValuesFrom rdf:resource="resource"/>
            </owl:Restriction>
        </rdfs:subClassOf>
        <rdfs:subClassOf>
            <owl:Restriction>
                <owl:onProperty rdf:resource="aggregates"/>
                <owl:someValuesFrom rdf:resource="informationFlow"/>
            </owl:Restriction>
        </rdfs:subClassOf>
        <rdfs:subClassOf>
            <owl:Restriction>
                <owl:onProperty rdf:resource="aggregates"/>
                <owl:someValuesFrom rdf:resource="interaction"/>
            </owl:Restriction>
        </rdfs:subClassOf>
        <rdfs:subClassOf>
            <owl:Restriction>
                <owl:onProperty rdf:resource="aggregates"/>
                <owl:someValuesFrom rdf:resource="role"/>
            </owl:Restriction>
        </rdfs:subClassOf>
        <rdfs:subClassOf>
            <owl:Restriction>
                <owl:onProperty rdf:resource="aggregates"/>
                <owl:someValuesFrom rdf:resource="relationship"/>
            </owl:Restriction>
        </rdfs:subClassOf>
        <skos:historyNote>Introduced in ISO/TS 14812:2022</skos:historyNote>
    </owl:Class>
    <owl:Class rdf:about="enterpriseViewpoint">
        <clause>3.1.4.4</clause>
        <skos:prefLabel xml:lang="en">enterprise viewpoint</skos:prefLabel>
        <skos:definition>architecture viewpoint (3.1.3.6) used to frame the policies, funding
            incentives, working arrangements and jurisdictional structure that support the technical
            layers of the architecture (3.1.3.1)</skos:definition>
        <rdfs:subClassOf rdf:resource="architectureViewpoint"/>
        <rdfs:subClassOf>
            <owl:Restriction>
                <owl:onProperty rdf:resource="governs"/>
                <owl:someValuesFrom rdf:resource="enterpriseView"/>
            </owl:Restriction>
        </rdfs:subClassOf>
        <skos:historyNote>Introduced in ISO/TS 14812:2022</skos:historyNote>
    </owl:Class>
    <owl:Class rdf:about="functionalView">
        <clause>3.1.4.5</clause>
        <skos:prefLabel xml:lang="en">functional view</skos:prefLabel>
        <skos:definition>architecture view (3.1.3.7) from the functional viewpoint (3.1.4.6)</skos:definition>
        <rdfs:subClassOf rdf:resource="architectureView"/>
        <rdfs:subClassOf>
            <owl:Restriction>
                <owl:onProperty rdf:resource="aggregates"/>
                <owl:someValuesFrom rdf:resource="process"/>
            </owl:Restriction>
        </rdfs:subClassOf>
        <rdfs:subClassOf>
            <owl:Restriction>
                <owl:onProperty rdf:resource="aggregates"/>
                <owl:someValuesFrom rdf:resource="dataFlow"/>
            </owl:Restriction>
        </rdfs:subClassOf>
        <rdfs:subClassOf>
            <owl:Restriction>
                <owl:onProperty rdf:resource="aggregates"/>
                <owl:someValuesFrom rdf:resource="processSpecification"/>
            </owl:Restriction>
        </rdfs:subClassOf>
        <rdfs:subClassOf>
            <owl:Restriction>
                <owl:onProperty rdf:resource="aggregates"/>
                <owl:someValuesFrom rdf:resource="terminator"/>
            </owl:Restriction>
        </rdfs:subClassOf>
        <skos:historyNote>Introduced in ISO/TS 14812:2022</skos:historyNote>
    </owl:Class>
    <owl:Class rdf:about="functionalViewpoint">
        <clause>3.1.4.6</clause>
        <skos:prefLabel xml:lang="en">functional viewpoint</skos:prefLabel>
        <skos:definition>architecture viewpoint (3.1.3.6) used to frame concerns (3.1.3.5) related
            to the definition of processes (3.1.7.2) that perform surface transport functions and
            data flows (3.1.7.1) shared between these processes</skos:definition>
        <rdfs:subClassOf rdf:resource="architectureViewpoint"/>
        <rdfs:subClassOf>
            <owl:Restriction>
                <owl:onProperty rdf:resource="governs"/>
                <owl:someValuesFrom rdf:resource="functionalView"/>
            </owl:Restriction>
        </rdfs:subClassOf>
        <skos:historyNote>Introduced in ISO/TS 14812:2022</skos:historyNote>
    </owl:Class>
    <owl:Class rdf:about="physicalView">
        <clause>3.1.4.7</clause>
        <skos:prefLabel xml:lang="en">physical view</skos:prefLabel>
        <skos:definition>architecture view (3.1.3.7) from the physical viewpoint (3.1.4.8)</skos:definition>
        <skos:note>The term "deployment view" is sometimes used within the broader
            ICT community, but the term "physical view" is preferred to prevent confusion between
            the physical view of a reference architecture and any part of a deployment architecture
            (3.1.9.3).</skos:note>
        <rdfs:subClassOf rdf:resource="architectureView"/>
        <rdfs:subClassOf>
            <owl:Restriction>
                <owl:onProperty rdf:resource="aggregates"/>
                <owl:someValuesFrom rdf:resource="physicalObject"/>
            </owl:Restriction>
        </rdfs:subClassOf>
        <rdfs:subClassOf>
            <owl:Restriction>
                <owl:onProperty rdf:resource="aggregates"/>
                <owl:someValuesFrom rdf:resource="informationTransfer"/>
            </owl:Restriction>
        </rdfs:subClassOf>
        <rdfs:subClassOf>
            <owl:Restriction>
                <owl:onProperty rdf:resource="aggregates"/>
                <owl:someValuesFrom rdf:resource="functionalObject"/>
            </owl:Restriction>
        </rdfs:subClassOf>
        <skos:historyNote>Introduced in ISO/TS 14812:2022</skos:historyNote>
    </owl:Class>
    <owl:Class rdf:about="physicalViewpoint">
        <clause>3.1.4.8</clause>
        <skos:prefLabel xml:lang="en">physical viewpoint</skos:prefLabel>
        <skos:definition>architecture viewpoint (3.1.3.6) used to frame concerns (3.1.3.5) related
            to the assignment of functionality to physical objects (3.1.8.1) and the interfaces
            among these physical objects</skos:definition>
        <rdfs:subClassOf rdf:resource="architectureViewpoint"/>
        <rdfs:subClassOf>
            <owl:Restriction>
                <owl:onProperty rdf:resource="governs"/>
                <owl:someValuesFrom rdf:resource="physicalView"/>
            </owl:Restriction>
        </rdfs:subClassOf>
        <skos:historyNote>Introduced in ISO/TS 14812:2022</skos:historyNote>
    </owl:Class>
    <owl:Class rdf:about="applicationEntity">
        <clause>3.1.5.1</clause>
        <skos:prefLabel xml:lang="en">application entity</skos:prefLabel>
        <altPrefLabel xml:lang="en">ITS-S application entity</altPrefLabel>
        <skos:hiddenLabel xml:lang="en">information layer</skos:hiddenLabel>
        <skos:definition>part of the ITS station reference architecture (3.1.9.4) that is
            responsible for providing ITS-related functionality</skos:definition>
        <skos:note>Within the US, the National Transportation Communications for
            ITS Protocol (NTCIP) standards identify an "information layer" on top of the traditional
            OSI stack. However, the purpose of this layer includes both information configuration
            and functionality. The ITS-S reference architecture separates these two roles between
            the management entity (3.1.5.6) and the application entity.</skos:note>
        <skos:historyNote>Introduced in ISO/TS 14812:2022</skos:historyNote>
    </owl:Class>
    <owl:Class rdf:about="accessLayer">
        <clause>3.1.5.2</clause>
        <skos:prefLabel xml:lang="en">access layer</skos:prefLabel>
        <skos:altLabel xml:lang="en">link layer</skos:altLabel>
        <skos:altLabel xml:lang="en">subnet layer</skos:altLabel>
        <skos:definition>communications layer that corresponds to the physical and data link layers
            of the OSI model</skos:definition>
        <skos:note>Within the Internet Engineering Task Force (IETF), the term
            "link layer" is used to describe the same functionality as the access layer.</skos:note>
        <skos:note>Within the US, the NTCIP standards use the term "subnet layer"
            to describe the same functionality as the access layer.</skos:note>
        <skos:historyNote>Introduced in ISO/TS 14812:2022. Revised in 2025 based on input from WG 16
            and to align more closely with the other definitions within ISO 14812.</skos:historyNote>
    </owl:Class>
    <owl:Class rdf:about="its-sAccessLayer">
        <clause>3.1.5.3</clause>
        <skos:prefLabel xml:lang="en">ITS-S access layer</skos:prefLabel>
        <skos:definition>communications layer in the ITS station reference architecture (3.1.9.4)
            corresponding to the physical and data link layers of the OSI model for ITS
            communications</skos:definition>
        <rdfs:subClassOf rdf:resource="accessLayer"/>
        <skos:historyNote>Introduced in ISO/TS 14812:2022. Revised in 2025 based on input from WG 16
            and to align more closely with the other definitions within ISO 14812.</skos:historyNote>
    </owl:Class>
    <owl:Class rdf:about="transnetLayer">
        <clause>3.1.5.4</clause>
        <skos:prefLabel xml:lang="en">transnet layer</skos:prefLabel>
        <altPrefLabel xml:lang="en">ITS-S networking and transport layer</altPrefLabel>
        <altPrefLabel xml:lang="en">networking and transport layer</altPrefLabel>
        <skos:definition>communications layer in the ITS station reference architecture (3.1.9.4)
            corresponding to the network and transport layers of the OSI model</skos:definition>
        <skos:note>The full name of this layer is the networking and transport
            layer, but the term transnet layer provides a more concise name.</skos:note>
        <skos:historyNote>Introduced in ISO/TS 14812:2022. Revised in 2025 based on input from WG 16
            and to align more closely with the other definitions within ISO 14812.</skos:historyNote>
    </owl:Class>
    <owl:Class rdf:about="facilitiesLayer">
        <clause>3.1.5.5</clause>
        <skos:prefLabel xml:lang="en">facilities layer</skos:prefLabel>
        <altPrefLabel xml:lang="en">ITS-S facilities layer</altPrefLabel>
        <skos:hiddenLabel xml:lang="en">application layer</skos:hiddenLabel>
        <skos:definition>communications layer in the ITS station reference architecture (3.1.9.4)
            corresponding to the session, presentation and application layers of the OSI model</skos:definition>
        <skos:note>Within the US, the NTCIP standards call the facilities layer the
            "application layer". However, as this term is easily confused with both the OSI
            application layer and the application entity (3.1.5.1), the term should be avoided and
            qualified when used (e.g. OSI application layer).</skos:note>
        <skos:historyNote>Introduced in ISO/TS 14812:2022. Revised in 2025 based on input from WG 16
            and to align more closely with the other definitions within ISO 14812.</skos:historyNote>
    </owl:Class>
    <owl:Class rdf:about="managementEntity">
        <clause>3.1.5.6</clause>
        <skos:prefLabel xml:lang="en">management entity</skos:prefLabel>
        <altPrefLabel xml:lang="en">ITS-S management entity</altPrefLabel>
        <skos:definition>part of the ITS station reference architecture (3.1.9.4) that is
            responsible for management and configuration of all layers and entities within the ITS-S</skos:definition>
        <skos:historyNote>Introduced in ISO/TS 14812:2022. Revised in 2025 based on input from WG 16
            and to align more closely with the other definitions within ISO 14812.</skos:historyNote>
    </owl:Class>
    <owl:Class rdf:about="securityEntity">
        <clause>3.1.5.7</clause>
        <skos:prefLabel xml:lang="en">security entity</skos:prefLabel>
        <altPrefLabel xml:lang="en">ITS-S security entity</altPrefLabel>
        <skos:definition>part of the ITS station reference architecture (3.1.9.4) that is
            responsible for providing communication security and system (3.1.2.1) security</skos:definition>
        <skos:historyNote>Introduced in ISO/TS 14812:2022. Revised in 2025 based on input from WG 16
            and to align more closely with the other definitions within ISO 14812.</skos:historyNote>
    </owl:Class>
    <owl:Class rdf:about="enterpriseObject">
        <clause>3.1.6.1</clause>
        <skos:prefLabel xml:lang="en">enterprise object</skos:prefLabel>
        <skos:definition>element (3.1.3.10) within an enterprise view (3.1.4.3) that represents an
            organization or individual</skos:definition>
        <skos:historyNote>Introduced in ISO/TS 14812:2022</skos:historyNote>
    </owl:Class>
    <owl:Class rdf:about="resource">
        <clause>3.1.6.2</clause>
        <skos:prefLabel xml:lang="en">resource</skos:prefLabel>
        <altPrefLabel xml:lang="en">enterprise view resource</altPrefLabel>
        <skos:definition>&lt;enterprise view&gt; element (3.1.3.10) that represents an entity
            (3.1.1.1) that is managed, operated, referenced and/or used to develop and provide ITS
            (3.1.2.4)</skos:definition>
        <skos:historyNote>Introduced in ISO/TS 14812:2022</skos:historyNote>
    </owl:Class>
    <owl:Class rdf:about="document">
        <clause>3.1.6.3</clause>
        <skos:prefLabel xml:lang="en">document</skos:prefLabel>
        <skos:definition>uniquely identified unit of information for human use</skos:definition>
        <skos:example>A report, specification, manual or book, in printed or electronic
            form.</skos:example>
        <skos:note>A document can be a single information item, or part of a larger
            information item.</skos:note>
        <dcterms:source>ISO/IEC/IEEE 15289:2019, 3.1.10</dcterms:source>
        <rdfs:subClassOf rdf:resource="resource"/>
        <skos:historyNote>Introduced in ISO/TS 14812:2022</skos:historyNote>
    </owl:Class>
    <owl:Class rdf:about="interaction">
        <clause>3.1.6.4</clause>
        <skos:prefLabel xml:lang="en">interaction</skos:prefLabel>
        <altPrefLabel xml:lang="en">enterprise view interaction</altPrefLabel>
        <skos:definition>&lt;enterprise view&gt; element (3.1.3.10) that represents coordination
            between two enterprise objects (3.1.6.1)</skos:definition>
        <skos:historyNote>Introduced in ISO/TS 14812:2022</skos:historyNote>
    </owl:Class>
    <owl:Class rdf:about="formalCoordination">
        <clause>3.1.6.5</clause>
        <skos:prefLabel xml:lang="en">formal coordination</skos:prefLabel>
        <altPrefLabel xml:lang="en">enterprise view formal coordination</altPrefLabel>
        <skos:definition>&lt;enterprise view&gt; interaction (3.1.6.4) between two enterprise
            objects (3.1.6.1) governed by a documented agreement</skos:definition>
        <skos:example>A road operator can enter into formal agreement(s) with the owner of a
            road (3.3.5.1) and the owner(s) of the associated roadside (3.3.1.10) equipment.</skos:example>
        <rdfs:subClassOf rdf:resource="interaction"/>
        <skos:historyNote>Introduced in ISO/TS 14812:2022</skos:historyNote>
    </owl:Class>
    <owl:Class rdf:about="informalCoordination">
        <clause>3.1.6.6</clause>
        <skos:prefLabel xml:lang="en">informal coordination</skos:prefLabel>
        <altPrefLabel xml:lang="en">enterprise view informal coordination</altPrefLabel>
        <skos:definition>&lt;enterprise view&gt; interaction (3.1.6.4) between two enterprise
            objects (3.1.6.1) governed by an understanding that is not documented in a formal
            agreement between the two parties</skos:definition>
        <rdfs:subClassOf rdf:resource="interaction"/>
        <skos:historyNote>Introduced in ISO/TS 14812:2022</skos:historyNote>
    </owl:Class>
    <owl:Class rdf:about="role">
        <clause>3.1.6.7</clause>
        <skos:prefLabel xml:lang="en">role</skos:prefLabel>
        <altPrefLabel xml:lang="en">enterprise view role</altPrefLabel>
        <skos:definition>&lt;enterprise view&gt; element (3.1.3.10) that represents the specified
            responsibilities between an enterprise object (3.1.6.1) and another enterprise view
            (3.1.4.3) element</skos:definition>
        <skos:historyNote>Introduced in ISO/TS 14812:2022</skos:historyNote>
    </owl:Class>
    <owl:Class rdf:about="relationship">
        <clause>3.1.6.8</clause>
        <skos:prefLabel xml:lang="en">relationship</skos:prefLabel>
        <altPrefLabel xml:lang="en">enterprise view relationship</altPrefLabel>
        <skos:definition>&lt;enterprise view&gt; element (3.1.3.10) that represents an association
            between two resources (3.1.6.2)</skos:definition>
        <skos:historyNote>Introduced in ISO/TS 14812:2022</skos:historyNote>
    </owl:Class>
    <owl:Class rdf:about="include">
        <clause>3.1.6.9</clause>
        <skos:prefLabel xml:lang="en">include</skos:prefLabel>
        <altPrefLabel xml:lang="en">enterprise view include</altPrefLabel>
        <skos:definition>&lt;enterprise view&gt; relationship (3.1.6.8) where one resource (3.1.6.2)
            contains another resource</skos:definition>
        <skos:example>Every ITS component includes one or more modules (3.1.8.7).</skos:example>
        <rdfs:subClassOf rdf:resource="relationship"/>
        <skos:historyNote>Introduced in ISO/TS 14812:2022</skos:historyNote>
    </owl:Class>
    <owl:Class rdf:about="extend">
        <clause>3.1.6.10</clause>
        <skos:prefLabel xml:lang="en">extend</skos:prefLabel>
        <altPrefLabel xml:lang="en">enterprise view extend</altPrefLabel>
        <skos:definition>&lt;enterprise view&gt; relationship (3.1.6.8) where one resource (3.1.6.2)
            supplements another resource</skos:definition>
        <skos:example>A module (3.1.8.7) can extend the functionality of another module.</skos:example>
        <rdfs:subClassOf rdf:resource="relationship"/>
        <skos:historyNote>Introduced in ISO/TS 14812:2022</skos:historyNote>
    </owl:Class>
    <owl:Class rdf:about="dataFlow">
        <clause>3.1.7.1</clause>
        <skos:prefLabel xml:lang="en">data flow</skos:prefLabel>
        <skos:definition>representation of data flowing between two processes (3.1.7.2) or between a
            process and a terminator (3.1.8.3)</skos:definition>
        <skos:historyNote>Introduced in ISO/TS 14812:2022</skos:historyNote>
    </owl:Class>
    <owl:Class rdf:about="process">
        <clause>3.1.7.2</clause>
        <skos:prefLabel xml:lang="en">process</skos:prefLabel>
        <altPrefLabel xml:lang="en">functional view process</altPrefLabel>
        <skos:definition>&lt;functional view&gt; series of one or more functions (3.1.7.3) in
            support of an ITS service (3.5.3.1)</skos:definition>
        <rdfs:subClassOf>
            <owl:Restriction>
                <owl:onProperty rdf:resource="aggregates"/>
                <owl:someValuesFrom rdf:resource="function"/>
            </owl:Restriction>
        </rdfs:subClassOf>
        <skos:historyNote>Introduced in ISO/TS 14812:2022</skos:historyNote>
    </owl:Class>
    <owl:Class rdf:about="function">
        <clause>3.1.7.3</clause>
        <skos:prefLabel xml:lang="en">function</skos:prefLabel>
        <altPrefLabel xml:lang="en">functional view function</altPrefLabel>
        <skos:definition>&lt;functional view&gt; series of actions or activities performed by a
            given object to achieve a goal</skos:definition>
        <skos:note>A function transforms inputs into outputs that may include the
            creation, modification, monitoring or destruction of elements (3.1.3.10).</skos:note>
        <skos:historyNote>Introduced in ISO/TS 14812:2022</skos:historyNote>
    </owl:Class>
    <owl:Class rdf:about="processSpecification">
        <clause>3.1.7.4</clause>
        <skos:prefLabel xml:lang="en">process specification</skos:prefLabel>
        <skos:definition>document (3.1.6.3) that defines a lowest-level process (3.1.7.2)</skos:definition>
        <skos:historyNote>Introduced in ISO/TS 14812:2022</skos:historyNote>
    </owl:Class>
    <owl:Class rdf:about="physicalObject">
        <clause>3.1.8.1</clause>
        <skos:prefLabel xml:lang="en">physical object</skos:prefLabel>
        <altPrefLabel xml:lang="en">ITS physical object</altPrefLabel>
        <skos:definition>&lt;physical view&gt; abstraction of a material entity (3.1.1.3) that
            interacts with other abstract material entities in the provision of ITS services
            (3.5.3.1)</skos:definition>
        <skos:note>Physical objects are represented as elements (3.1.3.10) within
            the physical view (3.1.4.7) and perform a role. Physical objects can be implemented as
            cloud-based systems (3.1.2.1).</skos:note>
        <skos:note>Within many ITS reference architectures (3.1.9.5), physical
            objects are placed into one of five categories: centre, support, field, vehicle or
            traveller (3.6.1.1).</skos:note>
        <rdfs:subClassOf rdf:resource="resource"/>
        <rdfs:subClassOf rdf:resource="system"/>
        <skos:historyNote>Introduced in ISO/TS 14812:2022</skos:historyNote>
    </owl:Class>
    <owl:Class rdf:about="itsComponent">
        <clause>3.1.8.2</clause>
        <skos:prefLabel xml:lang="en">ITS component</skos:prefLabel>
        <skos:definition>physical object (3.1.8.1) that has been assigned one or more functional
            objects (3.1.8.6) in the provision of one or more ITS services (3.5.3.1)</skos:definition>
        <skos:note>Physical objects are ITS components if they are an integral part
            of the system (3.1.2.1); otherwise they are terminators (3.1.8.3).</skos:note>
        <rdfs:subClassOf rdf:resource="physicalObject"/>
        <rdfs:subClassOf>
            <owl:Restriction>
                <owl:onProperty rdf:resource="aggregates"/>
                <owl:someValuesFrom rdf:resource="functionalObject"/>
            </owl:Restriction>
        </rdfs:subClassOf>
        <skos:historyNote>Introduced in ISO/TS 14812:2022</skos:historyNote>
    </owl:Class>
    <owl:Class rdf:about="terminator">
        <clause>3.1.8.3</clause>
        <skos:prefLabel xml:lang="en">terminator</skos:prefLabel>
        <altPrefLabel xml:lang="en">ITS terminator</altPrefLabel>
        <skos:definition>entity (3.1.1.1) that is external to the ITS service (3.5.3.1)
            implementation but with which the implementation communicates either to obtain inputs or
            to which it can send outputs</skos:definition>
        <skos:note>A terminator can exist within functional (3.1.4.5) and physical
            views (3.1.4.7).</skos:note>
        <rdfs:subClassOf rdf:resource="physicalObject"/>
        <skos:historyNote>Introduced in ISO/TS 14812:2022</skos:historyNote>
    </owl:Class>
    <owl:Class rdf:about="informationFlow">
        <clause>3.1.8.4</clause>
        <skos:prefLabel xml:lang="en">information flow</skos:prefLabel>
        <skos:definition>information that is exchanged between physical objects (3.1.8.1)</skos:definition>
        <skos:historyNote>Introduced in ISO/TS 14812:2022</skos:historyNote>
    </owl:Class>
    <owl:Class rdf:about="informationTransfer">
        <clause>3.1.8.5</clause>
        <skos:prefLabel xml:lang="en">information transfer</skos:prefLabel>
        <skos:altLabel xml:lang="en">information flow triple</skos:altLabel>
        <skos:definition>information flow (3.1.8.4) from a physical object (3.1.8.1) acting as an
            information provider and sent to another physical object acting as an information
            consumer</skos:definition>
        <skos:note>The term "information flow triple" is used extensively in the
            Architecture Reference for Cooperative and Intelligent Transportation (ARC-IT; see
            Reference [25]).</skos:note>
        <rdfs:subClassOf>
            <owl:Restriction>
                <owl:onProperty rdf:resource="sentFrom"/>
                <owl:someValuesFrom rdf:resource="physicalObject"/>
            </owl:Restriction>
        </rdfs:subClassOf>
        <rdfs:subClassOf>
            <owl:Restriction>
                <owl:onProperty rdf:resource="sentTo"/>
                <owl:someValuesFrom rdf:resource="physicalObject"/>
            </owl:Restriction>
        </rdfs:subClassOf>
        <rdfs:subClassOf>
            <owl:Restriction>
                <owl:onProperty rdf:resource="contentsOf"/>
                <owl:someValuesFrom rdf:resource="informationFlow"/>
            </owl:Restriction>
        </rdfs:subClassOf>
        <skos:historyNote>Introduced in ISO/TS 14812:2022</skos:historyNote>
    </owl:Class>
    <owl:Class rdf:about="functionalObject">
        <clause>3.1.8.6</clause>
        <skos:prefLabel xml:lang="en">functional object</skos:prefLabel>
        <altPrefLabel xml:lang="en">ITS functional object</altPrefLabel>
        <skos:definition>set of related processes (3.1.7.2) that are performed by a physical object
            (3.1.8.1) to fulfil aspects of an ITS service (3.5.3.1)</skos:definition>
        <skos:example>A vehicle OBE can include a "vehicle basic safety" functional object.</skos:example>
        <skos:note>The term "module" is used by the European FRAME architecture
            while the Architecture Reference for Cooperative and Intelligent Transportation (ARC-IT)
            uses the term "functional object".</skos:note>
        <rdfs:subClassOf rdf:resource="resource"/>
        <rdfs:subClassOf>
            <owl:Restriction>
                <owl:onProperty rdf:resource="groups"/>
                <owl:someValuesFrom rdf:resource="process"/>
            </owl:Restriction>
        </rdfs:subClassOf>
        <skos:historyNote>Introduced in ISO/TS 14812:2022</skos:historyNote>
    </owl:Class>
    <owl:Class rdf:about="module">
        <clause>3.1.8.7</clause>
        <skos:prefLabel xml:lang="en">module</skos:prefLabel>
        <altPrefLabel xml:lang="en">ITS module</altPrefLabel>
        <skos:definition>functional object (3.1.8.6) that can be replaced and has defined interfaces</skos:definition>
        <rdfs:subClassOf rdf:resource="functionalObject"/>
        <skos:historyNote>Introduced in ISO/TS 14812:2022</skos:historyNote>
    </owl:Class>
    <owl:Class rdf:about="referenceArchitecture">
        <clause>3.1.9.1</clause>
        <skos:prefLabel xml:lang="en">reference architecture</skos:prefLabel>
        <skos:definition>architecture (3.1.3.1) that provides a template solution for planning
            (3.1.9.2) and deployment architectures (3.1.9.3)</skos:definition>
        <skos:note>Interface standards are based on a reference architecture, which
            should be explicitly described.</skos:note>
        <rdfs:subClassOf rdf:resource="architecture"/>
        <skos:historyNote>Introduced in ISO/TS 14812:2022</skos:historyNote>
    </owl:Class>
    <owl:Class rdf:about="planningArchitecture">
        <clause>3.1.9.2</clause>
        <skos:prefLabel xml:lang="en">planning architecture</skos:prefLabel>
        <skos:altLabel xml:lang="en">regional architecture</skos:altLabel>
        <skos:definition>architecture (3.1.3.1) that provides a long-term vision of system elements
            (3.1.3.10) that may be deployed and managed by different projects and/or entities
            (3.1.1.1) within a geographic area</skos:definition>
        <skos:note>Some countries use the term "regional architecture", but in
            International Standards, the term "regional" is avoided due to its multiple meanings.</skos:note>
        <rdfs:subClassOf rdf:resource="architecture"/>
        <skos:historyNote>Introduced in ISO/TS 14812:2022</skos:historyNote>
    </owl:Class>
    <owl:Class rdf:about="deploymentArchitecture">
        <clause>3.1.9.3</clause>
        <skos:prefLabel xml:lang="en">deployment architecture</skos:prefLabel>
        <skos:definition>architecture (3.1.3.1) that provides a vision of a specific deployment of a
            system (3.1.2.1) within a geographic area</skos:definition>
        <rdfs:subClassOf rdf:resource="architecture"/>
        <skos:historyNote>Introduced in ISO/TS 14812:2022</skos:historyNote>
    </owl:Class>
    <owl:Class rdf:about="its-sReferenceArchitecture">
        <clause>3.1.9.4</clause>
        <skos:prefLabel xml:lang="en">ITS-S reference architecture</skos:prefLabel>
        <skos:definition>reference architecture (3.1.9.1) for handling communications within a
            physical object (3.1.8.1) as defined in ISO 21217</skos:definition>
        <skos:note>The ITS-S reference architecture provides a model for describing
            communication.</skos:note>
        <rdfs:subClassOf rdf:resource="referenceArchitecture"/>
        <rdfs:subClassOf>
            <owl:Restriction>
                <owl:onProperty rdf:resource="aggregates"/>
                <owl:someValuesFrom rdf:resource="applicationEntity"/>
            </owl:Restriction>
        </rdfs:subClassOf>
        <rdfs:subClassOf>
            <owl:Restriction>
                <owl:onProperty rdf:resource="aggregates"/>
                <owl:someValuesFrom rdf:resource="its-sAccessLayer"/>
            </owl:Restriction>
        </rdfs:subClassOf>
        <rdfs:subClassOf>
            <owl:Restriction>
                <owl:onProperty rdf:resource="aggregates"/>
                <owl:someValuesFrom rdf:resource="transnetLayer"/>
            </owl:Restriction>
        </rdfs:subClassOf>
        <rdfs:subClassOf>
            <owl:Restriction>
                <owl:onProperty rdf:resource="aggregates"/>
                <owl:someValuesFrom rdf:resource="facilitiesLayer"/>
            </owl:Restriction>
        </rdfs:subClassOf>
        <rdfs:subClassOf>
            <owl:Restriction>
                <owl:onProperty rdf:resource="aggregates"/>
                <owl:someValuesFrom rdf:resource="managementEntity"/>
            </owl:Restriction>
        </rdfs:subClassOf>
        <rdfs:subClassOf>
            <owl:Restriction>
                <owl:onProperty rdf:resource="aggregates"/>
                <owl:someValuesFrom rdf:resource="securityEntity"/>
            </owl:Restriction>
        </rdfs:subClassOf>
        <skos:historyNote>Introduced in ISO/TS 14812:2022</skos:historyNote>
    </owl:Class>
    <owl:Class rdf:about="itsReferenceArchitecture">
        <clause>3.1.9.5</clause>
        <skos:prefLabel xml:lang="en">ITS reference architecture</skos:prefLabel>
        <skos:definition>reference architecture (3.1.9.1) for one or more ITS services (3.5.3.1)</skos:definition>
        <skos:note>An ITS architecture can be a reference, planning or deployment
            architecture (3.1.9.3).</skos:note>
        <skos:note>The Architecture Reference for Cooperative and Intelligent
            Transportation (ARC-IT; see Reference [25]) is an example of an ITS reference
            architecture.</skos:note>
        <rdfs:subClassOf rdf:resource="referenceArchitecture"/>
        <skos:historyNote>Introduced in ISO/TS 14812:2022. Updated Note 2 to entry in 2025 to reference a more modern architecture reference model.</skos:historyNote>
    </owl:Class>
    <owl:Class rdf:about="itsPlanningArchitecture">
        <clause>3.1.9.6</clause>
        <skos:prefLabel xml:lang="en">ITS planning architecture</skos:prefLabel>
        <skos:definition>planning architecture (3.1.9.2) for one or more ITS services (3.5.3.1)</skos:definition>
        <rdfs:subClassOf rdf:resource="planningArchitecture"/>
    </owl:Class>
    <owl:Class rdf:about="itsDeploymentArchitecture">
        <clause>3.1.9.7</clause>
        <skos:prefLabel xml:lang="en">ITS deployment architecture</skos:prefLabel>
        <skos:definition>deployment architecture (3.1.9.3) for one or more ITS services (3.5.3.1)</skos:definition>
        <rdfs:subClassOf rdf:resource="deploymentArchitecture"/>
        <skos:historyNote>Introduced in ISO/TS 14812:2022</skos:historyNote>
    </owl:Class>
    <owl:Class rdf:about="dataConcept">
        <clause>3.1.10.1</clause>
        <skos:prefLabel xml:lang="en">data concept</skos:prefLabel>
        <skos:definition>data element (3.1.11.1), class (3.1.11.2), value domain (3.1.11.3), data
            frame (3.1.11.4), message (3.1.11.5) or interface dialogue (3.1.11.6) defined, at a
            minimum, with an unambiguous identifier and a definition</skos:definition>
        <skos:note>In order to exchange a value corresponding to a data concept,
            more information than an identifier, a name and a definition can be needed. For a
            property, a data type is needed. Depending on the kind of property, other data elements
            such as unit of measure, and language, can be needed as well. The additional information
            can be given in the data dictionary (3.1.10.3), in a data specification that references
            the data concept or associated with the data themselves.</skos:note>
        <rdfs:subClassOf>
            <owl:Restriction>
                <owl:onProperty rdf:resource="describes"/>
                <owl:someValuesFrom rdf:resource="entity"/>
            </owl:Restriction>
        </rdfs:subClassOf>
        <rdfs:subClassOf>
            <owl:Restriction>
                <owl:onProperty rdf:resource="storedIn"/>
                <owl:someValuesFrom rdf:resource="dataDictionary"/>
            </owl:Restriction>
        </rdfs:subClassOf>
        <skos:historyNote>Introduced in ISO/TS 14812:2022</skos:historyNote>
    </owl:Class>
    <owl:Class rdf:about="meta-attribute">
        <clause>3.1.10.2</clause>
        <skos:prefLabel xml:lang="en">meta-attribute</skos:prefLabel>
        <skos:definition>documenting characteristic of a data concept (3.1.10.1) that is stored in a
            data dictionary (3.1.10.3)</skos:definition>
        <rdfs:subClassOf>
            <owl:Restriction>
                <owl:onProperty rdf:resource="characteristicOf"/>
                <owl:someValuesFrom rdf:resource="dataConcept"/>
            </owl:Restriction>
        </rdfs:subClassOf>
        <skos:historyNote>Introduced in ISO/TS 14812:2022</skos:historyNote>
    </owl:Class>
    <owl:Class rdf:about="dataDictionary">
        <clause>3.1.10.3</clause>
        <skos:prefLabel xml:lang="en">data dictionary</skos:prefLabel>
        <skos:definition>collection of data concepts (3.1.10.1) that allows lookup by entity
            (3.1.1.1) identifier</skos:definition>
        <dcterms:source>ISO 22745-2:2010, B.2.16, modified - "collection of data dictionary
            entries..." replaced with "collection of data concepts...".</dcterms:source>
        <skos:historyNote>Introduced in ISO/TS 14812:2022</skos:historyNote>
    </owl:Class>
    <owl:Class rdf:about="dataConceptRegistry">
        <clause>3.1.10.4</clause>
        <skos:prefLabel xml:lang="en">data concept registry</skos:prefLabel>
        <skos:definition>electronic data dictionary (3.1.10.3) that follows precise documented rules
            for the registration and management of stored data concepts (3.1.10.1)</skos:definition>
        <skos:note>The data concept registry contains meta-attributes (3.1.10.2)
            about data concepts in terms of their names and representational forms as well as the
            semantics associated with the data concepts. A data concept registry may contain
            metadata that assists information interchange and re-use, both from the perspective of
            human users and for machine-interpretation of data concepts.</skos:note>
        <skos:note>A data concept registry typically includes advanced features for
            adding retrieving, and working with its contents.</skos:note>
        <rdfs:subClassOf rdf:resource="dataDictionary"/>
        <skos:historyNote>Introduced in ISO/TS 14812:2022</skos:historyNote>
    </owl:Class>
    <owl:Class rdf:about="dataElement">
        <clause>3.1.11.1</clause>
        <skos:prefLabel xml:lang="en">data element</skos:prefLabel>
        <skos:definition>unit of data that is considered in a given context to be indivisible and
            which includes an unambiguous representational form</skos:definition>
        <skos:note>This definition states that a data element is "indivisible" in a
            given context. This means it is possible for a data element considered indivisible in
            one context [e.g. location (3.4.1.1)] to be divisible in another context (e.g. latitude,
            longitude, and elevation).</skos:note>
        <rdfs:subClassOf rdf:resource="dataConcept"/>
        <rdfs:subClassOf>
            <owl:Restriction>
                <owl:onProperty rdf:resource="describes"/>
                <owl:qualifiedCardinality rdf:datatype="xsd:nonNegativeInteger">1</owl:qualifiedCardinality>
                <owl:onClass rdf:resource="class"/>
            </owl:Restriction>
        </rdfs:subClassOf>
        <rdfs:subClassOf>
            <owl:Restriction>
                <owl:onProperty rdf:resource="representedBy"/>
                <owl:qualifiedCardinality rdf:datatype="xsd:nonNegativeInteger">1</owl:qualifiedCardinality>
                <owl:onClass rdf:resource="valueDomain"/>
            </owl:Restriction>
        </rdfs:subClassOf>
        <skos:historyNote>Introduced in ISO/TS 14812:2022</skos:historyNote>
    </owl:Class>
    <owl:Class rdf:about="class">
        <clause>3.1.11.2</clause>
        <skos:prefLabel xml:lang="en">class</skos:prefLabel>
        <skos:altLabel xml:lang="en">object class</skos:altLabel>
        <skos:definition>set of ideas, abstractions or things in the real world that are identified
            with explicit boundaries and meaning and whose properties and behaviour follow the same
            rules</skos:definition>
        <skos:note>Some ISO/TC 204 documents use the term "object class" for
            consistency with ISO 11179-1, but within ITS, the term "class" is more generally
            understood.</skos:note>
        <skos:note>This is semantically equivalent to a "class" as used within UML
            (ISO19505-2:2012).</skos:note>
        <dcterms:source>ISO/IEC 11179-1:2015, 3.3.18, modified - term changed to from
            "object class" to "class" and Notes to entry added.</dcterms:source>
        <rdfs:subClassOf rdf:resource="dataConcept"/>
        <skos:historyNote>Introduced in ISO/TS 14812:2022</skos:historyNote>
    </owl:Class>
    <owl:Class rdf:about="valueDomain">
        <clause>3.1.11.3</clause>
        <skos:prefLabel xml:lang="en">value domain</skos:prefLabel>
        <skos:definition>a set of permissible values</skos:definition>
        <rdfs:subClassOf rdf:resource="dataConcept"/>
        <skos:historyNote>Introduced in ISO/TS 14812:2022</skos:historyNote>
    </owl:Class>
    <owl:Class rdf:about="dataFrame">
        <clause>3.1.11.4</clause>
        <skos:prefLabel xml:lang="en">data frame</skos:prefLabel>
        <skos:definition>specific grouping of data elements (3.1.11.1) that describes information of
            interest through a useful grouping of more atomic properties about one or more classes
            (3.1.11.2)</skos:definition>
        <skos:note>The grouping can be a set, sequence or a choice.</skos:note>
        <skos:note>Note 2 entry: A data frame can contain other data frames.</skos:note>
        <rdfs:subClassOf rdf:resource="dataConcept"/>
        <skos:historyNote>Introduced in ISO/TS 14812:2022</skos:historyNote>
    </owl:Class>
    <owl:Class rdf:about="message">
        <clause>3.1.11.5</clause>
        <skos:prefLabel xml:lang="en">message</skos:prefLabel>
        <skos:definition>grouping of data elements (3.1.11.1), data frames (3.1.11.4), or data
            elements and data frames that is used to convey information</skos:definition>
        <rdfs:subClassOf rdf:resource="dataConcept"/>
        <rdfs:subClassOf>
            <owl:Restriction>
                <owl:onProperty rdf:resource="contains"/>
                <owl:minQualifiedCardinality rdf:datatype="xsd:nonNegativeInteger">0</owl:minQualifiedCardinality>
                <owl:onClass rdf:resource="dataFrame"/>
            </owl:Restriction>
        </rdfs:subClassOf>
        <rdfs:subClassOf>
            <owl:Restriction>
                <owl:onProperty rdf:resource="contains"/>
                <owl:minQualifiedCardinality rdf:datatype="xsd:nonNegativeInteger">0</owl:minQualifiedCardinality>
                <owl:onClass rdf:resource="dataElement"/>
            </owl:Restriction>
        </rdfs:subClassOf>
        <skos:historyNote>Introduced in ISO/TS 14812:2022</skos:historyNote>
    </owl:Class>
    <owl:Class rdf:about="interfaceDialogue">
        <clause>3.1.11.6</clause>
        <skos:prefLabel xml:lang="en">interface dialogue</skos:prefLabel>
        <skos:altLabel xml:lang="en">dialog</skos:altLabel>
        <skos:altLabel xml:lang="en">dialogue</skos:altLabel>
        <skos:definition>bi-directional communication sequence between two parties in accordance
            with predetermined protocols</skos:definition>
        <skos:note>The term "dialog" represents the American English spelling.</skos:note>
        <skos:note>The term "dialogue" can be used when the interface context is
            known.</skos:note>
        <rdfs:subClassOf rdf:resource="dataConcept"/>
        <rdfs:subClassOf>
            <owl:Restriction>
                <owl:onProperty rdf:resource="uses"/>
                <owl:someValuesFrom rdf:resource="message"/>
            </owl:Restriction>
        </rdfs:subClassOf>
        <skos:historyNote>Introduced in ISO/TS 14812:2022</skos:historyNote>
    </owl:Class>
    <owl:Class rdf:about="useCase">
        <clause>3.1.12.1</clause>
        <skos:prefLabel xml:lang="en">use case</skos:prefLabel>
        <skos:definition>description of the behavioural requirements of a system (3.1.2.1) and its
            interaction (3.1.6.4) with a user (3.5.1.3)</skos:definition>
        <dcterms:source>ISO/IEC/IEEE 26515:2018, 3.15, modified - Note 1 to entry removed.</dcterms:source>
        <rdfs:subClassOf>
            <owl:Restriction>
                <owl:onProperty rdf:resource="aggregates"/>
                <owl:someValuesFrom rdf:resource="scenario"/>
            </owl:Restriction>
        </rdfs:subClassOf>
        <skos:historyNote>Introduced in ISO/TS 14812:2022</skos:historyNote>
    </owl:Class>
    <owl:Class rdf:about="scenario">
        <clause>3.1.12.2</clause>
        <skos:prefLabel xml:lang="en">scenario</skos:prefLabel>
        <altPrefLabel xml:lang="en">use case scenario</altPrefLabel>
        <skos:definition>&lt;use case&gt; description of the sequence of events from the user's
            (3.5.1.3) perspective to perform a task in a specified context</skos:definition>
        <dcterms:source>ISO/IEC 25062:2006, A.17</dcterms:source>
        <skos:historyNote>Introduced in ISO/TS 14812:2022</skos:historyNote>
    </owl:Class>
    <owl:Class rdf:about="role">
        <clause>3.1.12.3</clause>
        <skos:prefLabel xml:lang="en">role</skos:prefLabel>
        <skos:definition>specified responsibilities</skos:definition>
        <dcterms:source>ISO/IEC 11179-3:2013, 3.2.121</dcterms:source>
        <skos:historyNote>Introduced in ISO/TS 14812:2022</skos:historyNote>
    </owl:Class>
    <owl:Class rdf:about="instant">
        <clause>3.1.13.1</clause>
        <skos:prefLabel xml:lang="en">instant</skos:prefLabel>
        <skos:definition>0-dimensional geometric primitive representing position in time</skos:definition>
        <dcterms:source>ISO 19108:2002, 4.1.17, modified - Note 1 to entry removed.</dcterms:source>
        <skos:historyNote>Introduced in ISO/TS 14812:2022</skos:historyNote>
    </owl:Class>
    <owl:Class rdf:about="duration">
        <clause>3.1.13.2</clause>
        <skos:prefLabel xml:lang="en">duration</skos:prefLabel>
        <skos:definition>time between two instants (3.1.13.1)</skos:definition>
        <rdfs:subClassOf>
            <owl:Restriction>
                <owl:onProperty rdf:resource="startsAt"/>
                <owl:qualifiedCardinality rdf:datatype="xsd:nonNegativeInteger">1</owl:qualifiedCardinality>
                <owl:onClass rdf:resource="instant"/>
            </owl:Restriction>
        </rdfs:subClassOf>
        <rdfs:subClassOf>
            <owl:Restriction>
                <owl:onProperty rdf:resource="endsAt"/>
                <owl:qualifiedCardinality rdf:datatype="xsd:nonNegativeInteger">1</owl:qualifiedCardinality>
                <owl:onClass rdf:resource="instant"/>
            </owl:Restriction>
        </rdfs:subClassOf>
        <skos:historyNote>Introduced in ISO/TS 14812:2022</skos:historyNote>
    </owl:Class>
    <owl:Class rdf:about="authentication">
        <clause>3.1.14.1</clause>
        <skos:prefLabel xml:lang="en">authentication</skos:prefLabel>
        <skos:definition>verification that a message (3.1.11.5) was sent by the purported originator
            to the intended recipient and that the message was not changed in transit</skos:definition>
        <dcterms:source>ISO/IEC 2382:2015</dcterms:source>
        <skos:historyNote>Introduced in ISO/TS 14812:2025</skos:historyNote>
    </owl:Class>
    <owl:Class rdf:about="authenticator">
        <clause>3.1.14.2</clause>
        <skos:prefLabel xml:lang="en">authenticator</skos:prefLabel>
        <skos:definition>a network entity that executes an authentication (3.1.14.1) process on a
            message (3.1.11.5)</skos:definition>
        <dcterms:source>ISO/IEC/IEEE 8802-21, adapted from</dcterms:source>
        <skos:historyNote>Introduced in ISO/TS 14812:2025</skos:historyNote>
    </owl:Class>
    <owl:Class rdf:about="control">
        <clause>3.1.14.3</clause>
        <skos:prefLabel xml:lang="en">control</skos:prefLabel>
        <skos:definition>measure that is modifying risk (3.1.14.12)</skos:definition>
        <dcterms:source>ISO/IEC 27000:2018, 3.14</dcterms:source>
        <skos:historyNote>Introduced in ISO/TS 14812:2025</skos:historyNote>
    </owl:Class>
    <owl:Class rdf:about="cryptography">
        <clause>3.1.14.4</clause>
        <skos:prefLabel xml:lang="en">cryptography</skos:prefLabel>
        <skos:definition>discipline that embodies the principles, means, and methods for the
            transformation of data in order to hide their semantic content, prevent their
            unauthorized use, or prevent their undetected modification</skos:definition>
        <dcterms:source>ISO/IEC 22739:2018</dcterms:source>
        <skos:historyNote>Introduced in ISO/TS 14812:2025</skos:historyNote>
    </owl:Class>
    <owl:Class rdf:about="dataPrivacy">
        <clause>3.1.14.5</clause>
        <skos:prefLabel xml:lang="en">data privacy</skos:prefLabel>
        <skos:definition>rights and obligations of individuals and organizations with respect to the
            collection, use, retention, disclosure and disposal of personal information</skos:definition>
        <dcterms:source>ISO/IEC 17573-2:2018</dcterms:source>
        <skos:historyNote>Introduced in ISO/TS 14812:2025</skos:historyNote>
    </owl:Class>
    <owl:Class rdf:about="digitalSignature">
        <clause>3.1.14.6</clause>
        <skos:prefLabel xml:lang="en">digital signature</skos:prefLabel>
        <skos:definition>data appended to a message, that allow the recipient of the message
            (3.1.11.5) to verify the source of the message</skos:definition>
        <dcterms:source>ISO/IEC 2382:2015</dcterms:source>
        <skos:historyNote>Introduced in ISO/TS 14812:2025</skos:historyNote>
    </owl:Class>
    <owl:Class rdf:about="informationSecurityEvent">
        <clause>3.1.14.7</clause>
        <skos:prefLabel xml:lang="en">information security event</skos:prefLabel>
        <skos:definition>occurrence indicating a possible breach of information security or failure
            of controls (3.1.14.3)</skos:definition>
        <dcterms:source>ISO/IEC 27035-1</dcterms:source>
        <skos:historyNote>Introduced in ISO/TS 14812:2025</skos:historyNote>
    </owl:Class>
    <owl:Class rdf:about="informationSecurityIncident">
        <clause>3.1.14.8</clause>
        <skos:prefLabel xml:lang="en">information security incident</skos:prefLabel>
        <clause>3.1.14.8</clause>
        <skos:prefLabel xml:lang="en"></skos:prefLabel>
        <skos:definition>related and identified information security event(s) (3.1.14.7) that can
            harm an organization's assets or compromise its operations</skos:definition>
        <dcterms:source>ISO/IEC 27035-1</dcterms:source>
        <skos:historyNote>Introduced in ISO/TS 14812:2025</skos:historyNote>
    </owl:Class>
    <owl:Class rdf:about="non-repudiation">
        <clause>3.1.14.9</clause>
        <skos:prefLabel xml:lang="en">non-repudiation</skos:prefLabel>
        <skos:definition>ability to prove the occurrence of a claimed event or action and its
            originating entities</skos:definition>
        <dcterms:source>ISO/IEC 27000:2018, 3.48</dcterms:source>
        <skos:historyNote>Introduced in ISO/TS 14812:2025</skos:historyNote>
    </owl:Class>
    <owl:Class rdf:about="objective">
        <clause>3.1.14.10</clause>
        <skos:prefLabel xml:lang="en">objective</skos:prefLabel>
        <skos:definition>result to be achieved</skos:definition>
        <dcterms:source>ISO/IEC 27000:2018, 3.49</dcterms:source>
        <skos:historyNote>Introduced in ISO/TS 14812:2025</skos:historyNote>
    </owl:Class>
    <owl:Class rdf:about="resilience">
        <clause>3.1.14.11</clause>
        <skos:prefLabel xml:lang="en">resilience</skos:prefLabel>
        <skos:definition>capability of a system to maintain its functions and structure in the face
            of internal and external change, and to degrade gracefully when this is necessary</skos:definition>
        <dcterms:source>ISO/IEC 23257:2019</dcterms:source>
        <skos:historyNote>Introduced in ISO/TS 14812:2025</skos:historyNote>
    </owl:Class>
    <owl:Class rdf:about="risk">
        <clause>3.1.14.12</clause>
        <skos:prefLabel xml:lang="en">risk</skos:prefLabel>
        <skos:definition>effect of uncertainty on objectives (3.1.14.10)</skos:definition>
        <dcterms:source>ISO/IEC 27000:2018, 3.61</dcterms:source>
        <skos:historyNote>Introduced in ISO/TS 14812:2025</skos:historyNote>
    </owl:Class>
    <owl:Class rdf:about="threat">
        <clause>3.1.14.13</clause>
        <skos:prefLabel xml:lang="en">threat</skos:prefLabel>
        <skos:definition>potential cause of an unwanted incident, which can result in harm to a
            system or organization</skos:definition>
        <dcterms:source>ISO/IEC 27000:2018, 3.75</dcterms:source>
        <skos:historyNote>Introduced in ISO/TS 14812:2025</skos:historyNote>
    </owl:Class>
    <owl:Class rdf:about="transparency">
        <clause>3.1.14.14</clause>
        <skos:prefLabel xml:lang="en">transparency</skos:prefLabel>
        <skos:definition>open, comprehensive and understandable presentation of information</skos:definition>
        <dcterms:source>ISO/IEC 19944-1</dcterms:source>
        <skos:historyNote>Introduced in ISO/TS 14812:2025</skos:historyNote>
    </owl:Class>
    <owl:Class rdf:about="trustworthiness">
        <clause>3.1.14.15</clause>
        <skos:prefLabel xml:lang="en">trustworthiness</skos:prefLabel>
        <skos:definition>ability to meet stakeholders expectations in a verifiable way</skos:definition>
        <dcterms:source>ISO/IEC 5723</dcterms:source>
        <skos:historyNote>Introduced in ISO/TS 14812:2025</skos:historyNote>
    </owl:Class>
    <owl:Class rdf:about="vulnerability">
        <clause>3.1.14.16</clause>
        <skos:prefLabel xml:lang="en">vulnerability</skos:prefLabel>
        <skos:definition>weakness of an asset or control (3.1.14.3) that can be exploited by one or
            more threats (3.1.14.13)</skos:definition>
        <dcterms:source>ISO/IEC 27000:2018, 3.77</dcterms:source>
        <skos:historyNote>Introduced in ISO/TS 14812:2025</skos:historyNote>
    </owl:Class>
    <owl:Class rdf:about="design">
        <clause>3.1.15.1</clause>
        <skos:prefLabel xml:lang="en">design</skos:prefLabel>
        <skos:definition>the process or the result of the process to define the architecture, system
            elements, interfaces, and other characteristics of a system or system element</skos:definition>
        <skos:example>Example: Complete documentation for building a specific model of a smartphone</skos:example>
        <skos:note>Design provides the detailed implementation-level physical
            structure, behaviour, temporal relationships, and other attributes of system elements.
            It is information including specification of system elements and their relationships,
            that is sufficiently complete to support a compliant implementation of the architecture,</skos:note>
        <dcterms:source>ISO/IEC/IEEE 24765:2017, definitions 1 and 2 merged, example added</dcterms:source>
        <skos:historyNote>Introduced in ISO/TS 14812:2025</skos:historyNote>
    </owl:Class>
    <owl:Class rdf:about="implementation">
        <clause>3.1.15.2</clause>
        <skos:prefLabel xml:lang="en">implementation</skos:prefLabel>
        <skos:definition>the process or the result of the process of translating a design into
            hardware components, software components, or both</skos:definition>
        <skos:example>Example: The process of building a specific model of a smartphone or the
            resultant model of smartphone</skos:example>
        <skos:note>An implementation is the conceptual set of all instances of a
            product resulting from the translation. The set of all instances can consist of a single
            instance.</skos:note>
        <dcterms:source>ISO/IEC/IEEE 24765:2017, definitions 1 and 2 merged with example and note added</dcterms:source>
        <skos:historyNote>Introduced in ISO/TS 14812:2025</skos:historyNote>
    </owl:Class>
    <owl:Class rdf:about="instance">
        <clause>3.1.15.3</clause>
        <skos:prefLabel xml:lang="en">instance</skos:prefLabel>
        <skos:definition>discrete, bounded object with an intrinsic, immutable, and unique identity</skos:definition>
        <skos:example>Example: A specific smartphone (e.g., having a unique serial number)</skos:example>
        <skos:note>An instance of an implementation can also be called a physical
            instantiation, in the case of a hardware component.</skos:note>
        <dcterms:source>ISO/IEC/IEEE 24765:2017, definition 1, example and note added</dcterms:source>
        <skos:historyNote>Introduced in ISO/TS 14812:2025</skos:historyNote>
    </owl:Class>
    <owl:Class rdf:about="realization">
        <clause>3.1.15.4</clause>
        <skos:prefLabel xml:lang="en">realization</skos:prefLabel>
        <skos:definition>implementation of a system concept</skos:definition>
        <skos:note>A realization requires the development of a design and the
            translation of this design into hardware components, software components, or both.</skos:note>
        <dcterms:source>ISO/IEC/IEEE 24765:2017, example added</dcterms:source>
        <skos:historyNote>Introduced in ISO/TS 14812:2025</skos:historyNote>
    </owl:Class>
    <owl:Class rdf:about="requirement">
        <clause>3.1.15.5</clause>
        <skos:prefLabel xml:lang="en">requirement</skos:prefLabel>
        <skos:definition>provision that contains criteria to be fulfilled</skos:definition>
        <skos:example>Example: A measurable characteristic of a smartphone</skos:example>
        <dcterms:source>ISO/IEC/IEEE 24765:2017, example added</dcterms:source>
        <skos:historyNote>Introduced in ISO/TS 14812:2025</skos:historyNote>
    </owl:Class>
    <owl:Class rdf:about="requirementsSpecification">
        <clause>3.1.15.6</clause>
        <skos:prefLabel xml:lang="en">requirements specification</skos:prefLabel>
        <skos:definition>document that specifies the requirements for a system or component</skos:definition>
        <skos:example>Example: Wi-Fi 7, 5G, Bluetooth 5.3</skos:example>
        <skos:note>A device can conform to multiple requirements specifications,
            each with a different focus.</skos:note>
        <dcterms:source>ISO/IEC/IEEE 24765:2017, example and note added</dcterms:source>
        <skos:historyNote>Introduced in ISO/TS 14812:2025</skos:historyNote>
    </owl:Class>
    <owl:Class rdf:about="centralSystem">
        <clause>3.2.1.1</clause>
        <skos:prefLabel xml:lang="en">central system</skos:prefLabel>
        <altPrefLabel xml:lang="en">ITS central system</altPrefLabel>
        <skos:definition>ITS component (3.1.8.2) that provides application, management, and/or
            administrative functions from a centralized location (3.4.1.1) [i.e. not at the roadside
            (3.3.1.10)]</skos:definition>
        <rdfs:subClassOf rdf:resource="itsComponent"/>
        <skos:historyNote>Introduced in ISO/TS 14812:2022</skos:historyNote>
    </owl:Class>
    <owl:Class rdf:about="fieldSystem">
        <clause>3.2.1.2</clause>
        <skos:prefLabel xml:lang="en">field system</skos:prefLabel>
        <altPrefLabel xml:lang="en">ITS field system</altPrefLabel>
        <altPrefLabel xml:lang="en">roadside system</altPrefLabel>
        <skos:definition>infrastructure-based ITS component (3.1.8.2) located outside of a data
            centre that is designed to provide local processing or routing services while stationary</skos:definition>
        <skos:example>Traffic detector, camera, signal controller, message sign, tolling
            station.</skos:example>
        <skos:note>Typically, field systems are located along the roadside
            (3.3.1.10).</skos:note>
        <skos:note>Typically, the operation of a field system is governed by
            management functions running in a centre system.</skos:note>
        <skos:note>Field systems can be permanently installed or transportable.</skos:note>
        <skos:note>The term "roadside system" is typically used to describe field
            systems along a roadside but can also be used to refer to kiosks.</skos:note>
        <rdfs:subClassOf rdf:resource="itsComponent"/>
        <skos:historyNote>Introduced in ISO/TS 14812:2022</skos:historyNote>
    </owl:Class>
    <owl:Class rdf:about="personalSystem">
        <clause>3.2.1.3</clause>
        <skos:prefLabel xml:lang="en">personal system</skos:prefLabel>
        <altPrefLabel xml:lang="en">ITS personal system</altPrefLabel>
        <altPrefLabel xml:lang="en">traveller system</altPrefLabel>
        <skos:definition>ITS component (3.1.8.2), other than a vehicle system (3.2.1.5), that is
            used by a person (3.1.1.6) in relation to a past, current or upcoming journey</skos:definition>
        <rdfs:subClassOf rdf:resource="itsComponent"/>
        <skos:historyNote>Introduced in ISO/TS 14812:2022</skos:historyNote>
    </owl:Class>
    <owl:Class rdf:about="supportSystem">
        <clause>3.2.1.4</clause>
        <skos:prefLabel xml:lang="en">support system</skos:prefLabel>
        <altPrefLabel xml:lang="en">ITS support system</altPrefLabel>
        <skos:definition>ITS component (3.1.8.2) that provides services in support of one or more
            other ITS components</skos:definition>
        <skos:example>Data distribution system (3.1.2.1), network time source, cooperative
            ITS (3.1.2.5) credentials management system.</skos:example>
        <rdfs:subClassOf rdf:resource="itsComponent"/>
        <skos:historyNote>Introduced in ISO/TS 14812:2022</skos:historyNote>
    </owl:Class>
    <owl:Class rdf:about="vehicleSystem">
        <clause>3.2.1.5</clause>
        <skos:prefLabel xml:lang="en">vehicle system</skos:prefLabel>
        <altPrefLabel xml:lang="en">ITS vehicle system</altPrefLabel>
        <skos:definition>ITS component (3.1.8.2) that is installed as a component of a vehicle
            (3.7.1.1)</skos:definition>
        <rdfs:subClassOf rdf:resource="itsComponent"/>
        <skos:historyNote>Introduced in ISO/TS 14812:2022</skos:historyNote>
    </owl:Class>
    <owl:Class rdf:about="emergencyManagementCentralSystem">
        <clause>3.2.2.1</clause>
        <skos:prefLabel xml:lang="en">emergency management central system</skos:prefLabel>
        <skos:definition>centre system (3.2.1.1) that allows an entity (3.1.1.1) to manage and
            respond to crashes, events, disasters, evacuation orders and other incidents</skos:definition>
        <rdfs:subClassOf rdf:resource="centralSystem"/>
        <skos:historyNote>Introduced in ISO/TS 14812:2022</skos:historyNote>
    </owl:Class>
    <owl:Class rdf:about="fleetAndFreightManagementCentralSystem">
        <clause>3.2.2.2</clause>
        <skos:prefLabel xml:lang="en">fleet and freight management central system</skos:prefLabel>
        <skos:definition>centre system (3.2.1.1) that allows a fleet or freight operator to manage
            and control its personnel, equipment and/or freight</skos:definition>
        <rdfs:subClassOf rdf:resource="centralSystem"/>
        <skos:historyNote>Introduced in ISO/TS 14812:2022</skos:historyNote>
    </owl:Class>
    <owl:Class rdf:about="maintenanceAndConstructionCentralManagementSystem">
        <clause>3.2.2.3</clause>
        <skos:prefLabel xml:lang="en">maintenance and construction central management system</skos:prefLabel>
        <skos:definition>centre system (3.2.1.1) that allows an entity (3.1.1.1) to monitor and
            manage the construction and maintenance of road (3.3.5.1) infrastructure</skos:definition>
        <rdfs:subClassOf rdf:resource="centralSystem"/>
        <skos:historyNote>Introduced in ISO/TS 14812:2022</skos:historyNote>
    </owl:Class>
    <owl:Class rdf:about="paymentAdministrationCentralSystem">
        <clause>3.2.2.4</clause>
        <skos:prefLabel xml:lang="en">payment administration central system</skos:prefLabel>
        <skos:definition>centre system (3.2.1.1) that allows an entity (3.1.1.1) to manage financial
            transactions related to transportation, especially the electronic transfer of funds</skos:definition>
        <rdfs:subClassOf rdf:resource="centralSystem"/>
        <skos:historyNote>Introduced in ISO/TS 14812:2022</skos:historyNote>
    </owl:Class>
    <owl:Class rdf:about="publicTransportCentralManagementSystem">
        <clause>3.2.2.5</clause>
        <skos:prefLabel xml:lang="en">public transport central management system</skos:prefLabel>
        <skos:definition>centre system (3.2.1.1) that allows an entity (3.1.1.1) to manage the
            activities of a public transport (3.5.6.1) agency</skos:definition>
        <rdfs:subClassOf rdf:resource="centralSystem"/>
        <skos:historyNote>Introduced in ISO/TS 14812:2022</skos:historyNote>
    </owl:Class>
    <owl:Class rdf:about="trafficManagementCentralSystem">
        <clause>3.2.2.6</clause>
        <skos:prefLabel xml:lang="en">traffic management central system</skos:prefLabel>
        <skos:definition>centre system (3.2.1.1) that monitors and controls traffic and the road
            network (3.3.5.2)</skos:definition>
        <rdfs:subClassOf rdf:resource="centralSystem"/>
        <skos:historyNote>Introduced in ISO/TS 14812:2022</skos:historyNote>
    </owl:Class>
    <owl:Class rdf:about="trafficRegulationCentralSystem">
        <clause>3.2.2.7</clause>
        <skos:prefLabel xml:lang="en">traffic regulation central system</skos:prefLabel>
        <skos:definition>centre system (3.2.1.1) that officially records traffic regulations in
            electronic form so that they can be distributed to other systems</skos:definition>
        <rdfs:subClassOf rdf:resource="centralSystem"/>
        <skos:historyNote>Introduced in ISO/TS 14812:2022</skos:historyNote>
    </owl:Class>
    <owl:Class rdf:about="transportInformationCentralSystem">
        <clause>3.2.2.8</clause>
        <skos:prefLabel xml:lang="en">transport information central system</skos:prefLabel>
        <skos:definition>centre system (3.2.1.1) that provides information of interest to the
            travelling public</skos:definition>
        <rdfs:subClassOf rdf:resource="centralSystem"/>
        <skos:historyNote>Introduced in ISO/TS 14812:2022</skos:historyNote>
    </owl:Class>
    <owl:Class rdf:about="fieldSupportEquipment">
        <clause>3.2.3.1</clause>
        <skos:prefLabel xml:lang="en">field support equipment</skos:prefLabel>
        <altPrefLabel xml:lang="en">ITS field support equipment</altPrefLabel>
        <skos:definition>portable field system (3.2.1.2) used by field personnel to locally
            troubleshoot, initialize, reprogram and test infrastructure equipment</skos:definition>
        <rdfs:subClassOf rdf:resource="fieldSystem"/>
        <skos:historyNote>Introduced in ISO/TS 14812:2022</skos:historyNote>
    </owl:Class>
    <owl:Class rdf:about="itsRoadsideEquipment">
        <clause>3.2.3.2</clause>
        <skos:prefLabel xml:lang="en">ITS roadside equipment</skos:prefLabel>
        <altPrefLabel xml:lang="en">ITS roadway equipment</altPrefLabel>
        <skos:definition>field system (3.2.1.2) that performs localized ITS services (3.5.3.1)</skos:definition>
        <skos:example>traffic signal controller, variable message sign, vehicle detection</skos:example>
        <skos:note>ITS services that can be performed by ITS roadside equipment
            include surveillance, traffic control, information provision, payment transaction
            services, and/or enforcement</skos:note>
        <skos:note>"ITS roadway equipment" is used within the current version of
            the Architecture Reference for Cooperative and Intelligent Transportation (ARC-IT; see
            Reference [25]). The term roadway (3.3.1.3) has been revised to reflect that the
            equipment is typically along the roadway rather than a part of the roadway.</skos:note>
        <skos:note>While the term "roadside" indicates the typical location of the
            equipment, ITS roadside equipment (or portions thereof) can be embedded in the roadway
            itself.</skos:note>
        <rdfs:subClassOf rdf:resource="fieldSystem"/>
        <skos:historyNote>Introduced in ISO/TS 14812:2022. Added Note 3 to entry in 2025.</skos:historyNote>
    </owl:Class>
    <owl:Class rdf:about="connectedVehicleRoadsideEquipment">
        <clause>3.2.3.3</clause>
        <skos:prefLabel xml:lang="en">connected vehicle roadside equipment</skos:prefLabel>
        <altPrefLabel xml:lang="en">CV-RSE</altPrefLabel>
        <skos:definition>ITS roadside equipment (3.2.3.2) that perform ITS services (3.5.3.1) by
            exchanging electronic messages (3.1.11.5) with nearby connected vehicles (3.2.3.7) and/or
            personal systems (3.2.1.3) via short-range wireless technologies</skos:definition>
        <skos:note>Connected roadside equipment typically provides ITS-related
            functionality but the term includes roadside equipment that only provide the ITS service
            of routing for short-range wireless technologies.</skos:note>
        <skos:note>The term "connected vehicle roadside equipment" is used within
            the current version of the Architecture Reference for Cooperative and Intelligent
            Transportation (ARC-IT; see Reference [25]).</skos:note>
        <rdfs:subClassOf rdf:resource="itsRoadsideEquipment"/>
        <rdfs:subClassOf>
            <owl:Restriction>
                <owl:onProperty rdf:resource="aggregates"/>
                <owl:minQualifiedCardinality rdf:datatype="xsd:nonNegativeInteger">0</owl:minQualifiedCardinality>
                <owl:onClass rdf:resource="roadsideUnit"/>
            </owl:Restriction>
        </rdfs:subClassOf>
        <skos:historyNote>Introduced in ISO/TS 14812:2022. Revised in 2025 to 1. add "vehicle" to term 
            (i.e., from connected roadside equipment to connected vehicle roadside equipment), 2.  
            Replace "ITS connected roadside equipment" and "RSE" with "CV-RSE", and 3. change 
            reference to "vehicle systems" to "connected vehicles". </skos:historyNote>
    </owl:Class>
    <owl:Class rdf:about="roadsideUnit">
        <clause>3.2.3.4</clause>
        <skos:prefLabel xml:lang="en">roadside unit</skos:prefLabel>
        <altPrefLabel xml:lang="en">ITS roadside unit</altPrefLabel>
        <altPrefLabel xml:lang="en">RSU</altPrefLabel>
        <skos:definition>part of connected roadside equipment (3.2.3.3) that provides wireless
            connectivity to vehicle systems (3.2.1.5) and/or personal systems (3.2.1.3)</skos:definition>
        <rdfs:subClassOf rdf:resource="connectedUnit"/>
        <skos:historyNote>Introduced in ISO/TS 14812:2022</skos:historyNote>
    </owl:Class>
    <owl:Class rdf:about="connectedUnit">
        <clause>3.2.3.5</clause>
        <skos:prefLabel xml:lang="en">connected unit</skos:prefLabel>
        <altPrefLabel xml:lang="en">ITS connected unit</altPrefLabel>
        <skos:definition>electronic device that is connected (3.2.3.6) using one or more
            communication media</skos:definition>
        <rdfs:subClassOf>
            <owl:Restriction>
                <owl:onProperty rdf:resource="is"/>
                <owl:someValuesFrom rdf:resource="connected"/>
            </owl:Restriction>
        </rdfs:subClassOf>
        <skos:historyNote>Introduced in ISO/TS 14812:2022</skos:historyNote>
    </owl:Class>
    <owl:Class rdf:about="connected">
        <clause>3.2.3.6</clause>
        <skos:prefLabel xml:lang="en">connected</skos:prefLabel>
        <altPrefLabel xml:lang="en">ITS connected</altPrefLabel>
        <skos:definition>characteristic of a material entity (3.1.1.3) that is equipped with enabled
            (i.e. on) and operational electronic communication technologies to support ITS services
            (3.5.3.1), including the means to send and receive data to and from other connected
            entities</skos:definition>
        <skos:note>The term "connected" does not imply support for any specific
            communications interface or ITS-S application process (3.2.9.2).</skos:note>
        <rdfs:subClassOf>
            <owl:Restriction>
                <owl:onProperty rdf:resource="characteristicOf"/>
                <owl:someValuesFrom rdf:resource="materialEntity"/>
            </owl:Restriction>
        </rdfs:subClassOf>
        <skos:historyNote>Introduced in ISO/TS 14812:2022</skos:historyNote>
    </owl:Class>
    <owl:Class rdf:about="connectedVehicle">
        <clause>3.2.3.7</clause>
        <skos:prefLabel xml:lang="en">connected vehicle</skos:prefLabel>
        <skos:definition>vehicle (3.7.1.1) that is connected (3.2.3.6) using one or more
            communication media</skos:definition>
        <rdfs:subClassOf rdf:resource="vehicle"/>
        <rdfs:subClassOf>
            <owl:Restriction>
                <owl:onProperty rdf:resource="is"/>
                <owl:someValuesFrom rdf:resource="connected"/>
            </owl:Restriction>
        </rdfs:subClassOf>
        <skos:historyNote>Introduced in ISO/TS 14812:2025</skos:historyNote>
    </owl:Class>
    <owl:Class rdf:about="nomadicVehicleDevice">
        <clause>3.2.4.1</clause>
        <skos:prefLabel xml:lang="en">nomadic vehicle device</skos:prefLabel>
        <altPrefLabel xml:lang="en">carry-in vehicle device</altPrefLabel>
        <skos:altLabel xml:lang="en">external in-vehicle device</skos:altLabel>
        <skos:definition>personal system (3.2.1.3) consisting of global navigation satellite system
            (GNSS) and/or wireless modules (3.1.8.7) that are connected (3.2.3.6) to a vehicle
            (3.7.1.1) during a trip</skos:definition>
        <rdfs:subClassOf rdf:resource="personalSystem"/>
        <skos:historyNote>Introduced in ISO/TS 14812:2022</skos:historyNote>
    </owl:Class>
    <owl:Class rdf:about="personalInformationDevice">
        <clause>3.2.4.2</clause>
        <skos:prefLabel xml:lang="en">personal information device</skos:prefLabel>
        <altPrefLabel xml:lang="en">ITS personal information device</altPrefLabel>
        <skos:definition>personal system (3.2.1.3) that enables personal access to traveller
            (3.6.1.1) information</skos:definition>
        <skos:example>Personal computer.</skos:example>
        <rdfs:subClassOf rdf:resource="personalSystem"/>
        <skos:historyNote>Introduced in ISO/TS 14812:2022</skos:historyNote>
    </owl:Class>
    <owl:Class rdf:about="nomadicDevice">
        <clause>3.2.4.3</clause>
        <skos:prefLabel xml:lang="en">nomadic device</skos:prefLabel>
        <altPrefLabel xml:lang="en">ITS nomadic device</altPrefLabel>
        <skos:definition>personal information device (3.2.4.2) that is taken with and can be
            accessed by the traveller (3.6.1.1) during a journey</skos:definition>
        <skos:example>Smartphone.</skos:example>
        <rdfs:subClassOf rdf:resource="personalInformationDevice"/>
        <rdfs:subClassOf>
            <owl:Restriction>
                <owl:onProperty rdf:resource="accessedBy"/>
                <owl:minQualifiedCardinality rdf:datatype="xsd:nonNegativeInteger">0</owl:minQualifiedCardinality>
                <owl:onClass rdf:resource="traveller"/>
            </owl:Restriction>
        </rdfs:subClassOf>
        <skos:historyNote>Introduced in ISO/TS 14812:2022</skos:historyNote>
    </owl:Class>
    <owl:Class rdf:about="publicInformationDevice">
        <clause>3.2.4.4</clause>
        <skos:prefLabel xml:lang="en">public information device</skos:prefLabel>
        <altPrefLabel xml:lang="en">ITS public information device</altPrefLabel>
        <skos:definition>personal system (3.2.1.3) that provides public (3.5.8.2) access to
            traveller (3.6.1.1) information</skos:definition>
        <skos:example>Kiosk.</skos:example>
        <rdfs:subClassOf rdf:resource="personalSystem"/>
        <skos:historyNote>Introduced in ISO/TS 14812:2022</skos:historyNote>
    </owl:Class>
    <owl:Class rdf:about="cooperativeItsCredentialsManagementSystem">
        <clause>3.2.5.1</clause>
        <skos:prefLabel xml:lang="en">cooperative ITS credentials management system</skos:prefLabel>
        <altPrefLabel xml:lang="en">CCMS</altPrefLabel>
        <skos:definition>support system (3.2.1.4) that enables trusted communications among ITS
            components (3.1.8.2) and protects data from unauthorized access</skos:definition>
        <rdfs:subClassOf rdf:resource="supportSystem"/>
        <skos:historyNote>Introduced in ISO/TS 14812:2022</skos:historyNote>
    </owl:Class>
    <owl:Class rdf:about="mapProvisionSystem">
        <clause>3.2.5.2</clause>
        <skos:prefLabel xml:lang="en">map provision system</skos:prefLabel>
        <altPrefLabel xml:lang="en">ITS map provision system</altPrefLabel>
        <skos:definition>support system (3.2.1.4) that provides map databases used to support ITS
            services (3.5.3.1)</skos:definition>
        <rdfs:subClassOf rdf:resource="supportSystem"/>
        <skos:historyNote>Introduced in ISO/TS 14812:2022</skos:historyNote>
    </owl:Class>
    <owl:Class rdf:about="itsOn-boardEquipment">
        <clause>3.2.6.1</clause>
        <skos:prefLabel xml:lang="en">ITS on-board equipment</skos:prefLabel>
        <altPrefLabel xml:lang="en">on-board equipment</altPrefLabel>
        <altPrefLabel xml:lang="en">OBE</altPrefLabel>
        <skos:altLabel xml:lang="en">onboard equipment</skos:altLabel>
        <skos:definition>vehicle system (3.2.1.5) that provides all ITS functionality on-board the
            vehicle (3.7.1.1)</skos:definition>
        <skos:note>ITS on-board equipment relates to any functionality. When there
            is a need to distinguish between core functionality and that by a special vehicle, the
            term can be further refined by indicating the type of vehicle to which the on-board
            equipment relates. For example, emergency vehicle on-board equipment can provide
            specialized functionality.</skos:note>
        <skos:note>The on-board equipment may also perform other functions.</skos:note>
        <rdfs:subClassOf rdf:resource="vehicleSystem"/>
        <rdfs:subClassOf>
            <owl:Restriction>
                <owl:onProperty rdf:resource="comprises"/>
                <owl:someValuesFrom rdf:resource="itsOn-boardUnit"/>
            </owl:Restriction>
        </rdfs:subClassOf>
        <skos:historyNote>Introduced in ISO/TS 14812:2022</skos:historyNote>
    </owl:Class>
    <owl:Class rdf:about="itsOn-boardUnit">
        <clause>3.2.6.2</clause>
        <skos:prefLabel xml:lang="en">ITS on-board unit</skos:prefLabel>
        <altPrefLabel xml:lang="en">on-board unit</altPrefLabel>
        <altPrefLabel xml:lang="en">OBU</altPrefLabel>
        <skos:altLabel xml:lang="en">onboard unit</skos:altLabel>
        <skos:definition>part of on-board equipment (3.2.6.1) that provides wireless connectivity to
            other ITS components (3.1.8.2) external to the vehicle (3.7.1.1)</skos:definition>
        <skos:note>An OBU implementation can also include ITS functionality.</skos:note>
        <rdfs:subClassOf rdf:resource="connectedUnit"/>
        <skos:historyNote>Introduced in ISO/TS 14812:2022</skos:historyNote>
    </owl:Class>
    <owl:Class rdf:about="boundedSecuredManagedDomain">
        <clause>3.2.7.1</clause>
        <skos:prefLabel xml:lang="en">bounded secured managed domain</skos:prefLabel>
        <altPrefLabel xml:lang="en">BSMD</altPrefLabel>
        <skos:definition>abstract entity (3.1.1.1) representing a managed processing and memory
            environment (3.1.3.11) that provides protection from code and data that has not been
            determined to meet established security requirements</skos:definition>
        <rdfs:subClassOf rdf:resource="entity"/>
        <rdfs:subClassOf>
            <owl:Restriction>
                <owl:onProperty rdf:resource="represents"/>
                <owl:someValuesFrom rdf:resource="environment"/>
            </owl:Restriction>
        </rdfs:subClassOf>
        <skos:historyNote>Introduced in ISO/TS 14812:2022</skos:historyNote>
    </owl:Class>
    <owl:Class rdf:about="itsTrustDomain">
        <clause>3.2.7.2</clause>
        <skos:prefLabel xml:lang="en">ITS trust domain</skos:prefLabel>
        <skos:definition>set of bounded secured managed domains (3.2.7.1) that meet a defined set of
            ITS industry security requirements</skos:definition>
        <rdfs:subClassOf rdf:resource="boundedSecuredManagedDomain"/>
        <skos:historyNote>Introduced in ISO/TS 14812:2022</skos:historyNote>
    </owl:Class>
    <owl:Class rdf:about="itsStation">
        <clause>3.2.7.3</clause>
        <skos:prefLabel xml:lang="en">ITS station</skos:prefLabel>
        <altPrefLabel xml:lang="en">ITS-S</altPrefLabel>
        <skos:definition>bounded secured managed domain (3.2.7.1) that is able to meet requirements
            of the ITS trust domain (3.2.7.2) within which it is designed to participate</skos:definition>
        <skos:note>The ITS station reference architecture is defined in ISO 21217.</skos:note>
        <skos:note>This complements the ISO 21217:2020 definition (which identifies
            the component parts) and is consistent with the text of ISO 21217:2020.</skos:note>
        <rdfs:subClassOf rdf:resource="boundedSecuredManagedDomain"/>
        <rdfs:subClassOf>
            <owl:Restriction>
                <owl:onProperty rdf:resource="meetsRequirementsOf"/>
                <owl:someValuesFrom rdf:resource="itsTrustDomain"/>
            </owl:Restriction>
        </rdfs:subClassOf>
        <rdfs:subClassOf>
            <owl:Restriction>
                <owl:onProperty rdf:resource="describedBy"/>
                <owl:someValuesFrom rdf:resource="its-sReferenceArchitecture"/>
            </owl:Restriction>
        </rdfs:subClassOf>
        <skos:historyNote>Introduced in ISO/TS 14812:2022. Revised in 2025 to indicate the "design"
            and to add Note 2 to entry.</skos:historyNote>
    </owl:Class>
    <owl:Class rdf:about="its-sUnit">
        <clause>3.2.7.4</clause>
        <skos:prefLabel xml:lang="en">ITS-S unit</skos:prefLabel>
        <altPrefLabel xml:lang="en">ITS station unit</altPrefLabel>
        <altPrefLabel xml:lang="en">ITS-SU</altPrefLabel>
        <skos:definition>instance (3.1.15.3) of an physical unit produced by an ITS station
            (3.2.7.3) implementation (3.1.15.2)</skos:definition>
        <skos:note>This is a clarification of the definition provided in ISO
            21217:2020. While the definition for ITS station unit in ISO 21217:2020 refers to an
            implementation, the full text interchangeably describes it as an implementation or a
            physical instantiation, but does not define those terms explicitly.</skos:note>
        <rdfs:subClassOf>
            <owl:Restriction>
                <owl:onProperty rdf:resource="instantiationOf"/>
                <owl:someValuesFrom rdf:resource="itsStation"/>
            </owl:Restriction>
        </rdfs:subClassOf>
        <rdfs:subClassOf>
            <owl:Restriction>
                <owl:onProperty rdf:resource="comprises"/>
                <owl:someValuesFrom rdf:resource="its-sCommunicationUnit"/>
            </owl:Restriction>
        </rdfs:subClassOf>
        <skos:historyNote>Introduced in ISO/TS 14812:2022; revised in 2025. The original definition
            resulted in confusion as to whether it was intended to reference merely an implementation,
            which is an instance of a realization (e.g., something with a model number) or an instance 
            of an implementation (e.g., something that would have a serial number). Added Note 1 to 
            entry.</skos:historyNote>
    </owl:Class>
    <owl:Class rdf:about="its-sCommunicationUnit">
        <clause>3.2.7.5</clause>
        <skos:prefLabel xml:lang="en">ITS-S communication unit</skos:prefLabel>
        <altPrefLabel xml:lang="en">ITS station communication unit</altPrefLabel>
        <altPrefLabel xml:lang="en">ITS-SCU</altPrefLabel>
        <skos:definition>physical unit in an ITS-S unit (3.2.7.4) containing part or all of the
            functionality of the ITS-S (3.2.7.3)</skos:definition>
        <skos:note>In case an ITS-SU consists of a single physical unit, the ITS-SU
            and the ITS-SCU are identical. In case an ITS-SU consists of more than one ITS-SCU, then
            these ITS-SCUs are interconnected via the ITS station-internal network of the ITS-SU.</skos:note>
        <rdfs:subClassOf>
            <owl:Restriction>
                <owl:onProperty rdf:resource="contains"/>
                <owl:someValuesFrom rdf:resource="functionalObject"/>
            </owl:Restriction>
        </rdfs:subClassOf>
        <skos:historyNote>Introduced in ISO/TS 14812:2022; revised in 2025. Added Note 1 to 
            entry and revised to "the" ITS-S rather than "an" ITS-S.</skos:historyNote>
    </owl:Class>
    <owl:Class rdf:about="its-sHost">
        <clause>3.2.7.6</clause>
        <skos:prefLabel xml:lang="en">ITS-S host</skos:prefLabel>
        <altPrefLabel xml:lang="en">management host</altPrefLabel>
        <skos:definition>ITS-S node (3.2.7.8) comprised of ITS-S (3.2.7.3) functionalities other
            than the functionalities of an ITS-S router (3.2.7.7), ITS-S border router, ITS-S mobile
            router or an ITS-S gateway</skos:definition>
        <skos:note>ITS-S border router and ITS-S mobile router are ITS-S routers
            with added functionalities, which is why they are separately excluded in the above
            definition.</skos:note>
        <skos:note>ITS-S border router, ITS-S mobile router, and ITS-S gateway are
            defined in ISO 21217.</skos:note>
        <rdfs:subClassOf rdf:resource="its-sNode"/>
        <skos:historyNote>Introduced in ISO/TS 14812:2022 as functionality. Revised in ISO/TS 14812:2025 to be an ITS-S node.</skos:historyNote>
    </owl:Class>
    <owl:Class rdf:about="its-sRouter">
        <clause>3.2.7.7</clause>
        <skos:prefLabel xml:lang="en">ITS-S router</skos:prefLabel>
        <skos:definition>ITS-S node (3.2.7.8) comprised of routing functionalities of an ITS station
            unit (3.2.7.4) used to connect two networks and to forward packets not explicitly
            addressed to itself</skos:definition>
        <rdfs:subClassOf rdf:resource="its-sNode"/>
        <skos:historyNote>Introduced in ISO/TS 14812:2022 as functionality. Revised in ISO/TS 14812:2025 to be an ITS-S node.</skos:historyNote>
    </owl:Class>
    <owl:Class rdf:about="its-sNode">
        <clause>3.2.7.8</clause>
        <skos:prefLabel xml:lang="en">ITS-S node</skos:prefLabel>
        <skos:definition>node comprised of a set of functionalities in an ITS-S unit
            (3.2.7.4) that is connected (3.2.3.6) to the ITS station (3.2.7.3)-internal network or
            comprises an entire ITS-S unit</skos:definition>
        <rdfs:subClassOf>
            <owl:Restriction>
                <owl:onProperty rdf:resource="containedIn"/>
                <owl:someValuesFrom rdf:resource="its-sUnit"/>
            </owl:Restriction>
        </rdfs:subClassOf>
        <rdfs:subClassOf>
            <owl:Restriction>
                <owl:onProperty rdf:resource="comprises"/>
                <owl:someValuesFrom rdf:resource="functionality"/>
            </owl:Restriction>
        </rdfs:subClassOf>
        <skos:historyNote>Introduced in ISO/TS 14812:2022</skos:historyNote>
    </owl:Class>
    <owl:Class rdf:about="itsApplication">
        <clause>3.2.8.1</clause>
        <skos:prefLabel xml:lang="en">ITS application</skos:prefLabel>
        <skos:definition>requirements for an ITS service (3.5.3.1) that involves an association of
            two or more complementary ITS-S application processes (3.2.9.2)</skos:definition>
        <skos:note>An ITS application can also involve associations with nodes that
            are not ITS stations.</skos:note>
        <skos:note>This is a clarification of the ISO 21217:2020 definition that
            described this as an instantiation.</skos:note>
        <rdfs:subClassOf>
            <owl:Restriction>
                <owl:onProperty rdf:resource="involves"/>
                <owl:minQualifiedCardinality rdf:datatype="xsd:nonNegativeInteger">2</owl:minQualifiedCardinality>
                <owl:onClass rdf:resource="its-sApplicationProcess"/>
            </owl:Restriction>
        </rdfs:subClassOf>
        <rdfs:subClassOf>
            <owl:Restriction>
                <owl:onProperty rdf:resource="realizationOf"/>
                <owl:someValuesFrom rdf:resource="itsService"/>
            </owl:Restriction>
        </rdfs:subClassOf>
        <skos:historyNote>Introduced in ISO/TS 14812:2022</skos:historyNote>
    </owl:Class>
    <owl:Class rdf:about="interoperabilityDesign">
        <clause>3.2.8.2</clause>
        <skos:prefLabel xml:lang="en">interoperability design</skos:prefLabel>
        <skos:definition>characteristics necessary to fully define how various physical objects
            (3.1.8.1) interoperate to provide a service (3.5.1.1)</skos:definition>
        <skos:note>Characteristics often include but are not limited to functional,
            performance and interface requirements.</skos:note>
        <rdfs:subClassOf>
            <owl:Restriction>
                <owl:onProperty rdf:resource="definesHowToProvide"/>
                <owl:someValuesFrom rdf:resource="service"/>
            </owl:Restriction>
        </rdfs:subClassOf>
        <rdfs:subClassOf>
            <owl:Restriction>
                <owl:onProperty rdf:resource="using"/>
                <owl:someValuesFrom rdf:resource="physicalObject"/>
            </owl:Restriction>
        </rdfs:subClassOf>
        <skos:historyNote>Introduced in ISO/TS 14812:2022</skos:historyNote>
    </owl:Class>
    <owl:Class rdf:about="itsApplicationSpecification">
        <clause>3.2.8.3</clause>
        <skos:prefLabel xml:lang="en">ITS application specification</skos:prefLabel>
        <skos:definition>one or more documents (3.1.6.3) that detail the interoperability design
            (3.2.8.2) for an ITS application (3.2.8.1)</skos:definition>
        <rdfs:subClassOf>
            <owl:Restriction>
                <owl:onProperty rdf:resource="details"/>
                <owl:someValuesFrom rdf:resource="interoperabilityDesign"/>
            </owl:Restriction>
        </rdfs:subClassOf>
        <rdfs:subClassOf>
            <owl:Restriction>
                <owl:onProperty rdf:resource="for"/>
                <owl:someValuesFrom rdf:resource="itsApplication"/>
            </owl:Restriction>
        </rdfs:subClassOf>
        <skos:historyNote>Introduced in ISO/TS 14812:2022</skos:historyNote>
    </owl:Class>
    <owl:Class rdf:about="applicationTemplate">
        <clause>3.2.8.4</clause>
        <skos:prefLabel xml:lang="en">application template</skos:prefLabel>
        <altPrefLabel xml:lang="en">ITS application template</altPrefLabel>
        <skos:definition>defined annotated outline for an ITS application specification (3.2.8.3)</skos:definition>
        <rdfs:subClassOf>
            <owl:Restriction>
                <owl:onProperty rdf:resource="annotatedOutlineFor"/>
                <owl:someValuesFrom rdf:resource="itsApplicationSpecification"/>
            </owl:Restriction>
        </rdfs:subClassOf>
        <skos:historyNote>Introduced in ISO/TS 14812:2022</skos:historyNote>
    </owl:Class>
    <owl:Class rdf:about="itsImplementation">
        <clause>3.2.8.5</clause>
        <skos:prefLabel xml:lang="en">ITS implementation</skos:prefLabel>
        <skos:definition>integration of each physical object (3.1.8.1) necessary to implement one or
            more ITS applications (3.2.8.1)</skos:definition>
        <skos:note>An ITS application typically requires multiple components (e.g.
            an ITS-S acting as a user and another ITS-S acting as a provider). An ITS implementation
            includes a sample of each component necessary for the service but often does not
            represent a complete deployment.</skos:note>
        <skos:note>An ITS implementation is typically used for a laboratory or
            other experimental environment (3.1.3.11) prior to a full-scale deployment.</skos:note>
        <rdfs:subClassOf>
            <owl:Restriction>
                <owl:onProperty rdf:resource="implements"/>
                <owl:someValuesFrom rdf:resource="itsApplication"/>
            </owl:Restriction>
        </rdfs:subClassOf>
        <skos:historyNote>Introduced in ISO/TS 14812:2022</skos:historyNote>
    </owl:Class>
    <owl:Class rdf:about="itsDeployment">
        <clause>3.2.8.6</clause>
        <skos:prefLabel xml:lang="en">ITS deployment</skos:prefLabel>
        <skos:definition>installation capable of performing one or more ITS applications (3.2.8.1)</skos:definition>
        <skos:note>An ITS deployment typically refers to the support, central and
            roadside ITS stations coupled with a tacit acknowledgement of the mobile ITS stations
            that will communicate with the support, central or roadside ITS stations.</skos:note>
        <rdfs:subClassOf>
            <owl:Restriction>
                <owl:onProperty rdf:resource="installationOf"/>
                <owl:someValuesFrom rdf:resource="itsImplementation"/>
            </owl:Restriction>
        </rdfs:subClassOf>
        <skos:historyNote>Introduced in ISO/TS 14812:2022</skos:historyNote>
    </owl:Class>
    <owl:Class rdf:about="itsApplicationRole">
        <clause>3.2.9.1</clause>
        <skos:prefLabel xml:lang="en">ITS application role</skos:prefLabel>
        <skos:definition>ITS-S user need (3.5.4.4) expressed as a formal set of interoperability
            requirements that need to be fulfilled to satisfy a portion of functionality of an ITS
            application (3.2.8.1)</skos:definition>
        <rdfs:subClassOf rdf:resource="its-sUserNeed"/>
        <skos:historyNote>Introduced in ISO/TS 14812:2022</skos:historyNote>
    </owl:Class>
    <owl:Class rdf:about="its-sApplicationProcess">
        <clause>3.2.9.2</clause>
        <skos:prefLabel xml:lang="en">ITS-S application process</skos:prefLabel>
        <skos:definition>information manipulation within an ITS station (3.2.7.3) for an ITS-SU
            service (3.5.4.1)</skos:definition>
        <skos:note>ITS-S application processes use ITS-S services to communicate
            with other nodes.</skos:note>
        <skos:note>This clarifies the ISO 21217:2020 definition to remove ambiguity
            and a circular reference to "application".</skos:note>
        <rdfs:subClassOf>
            <owl:Restriction>
                <owl:onProperty rdf:resource="performsInformationProcessingFor"/>
                <owl:someValuesFrom rdf:resource="its-sService"/>
            </owl:Restriction>
        </rdfs:subClassOf>
        <rdfs:subClassOf>
            <owl:Restriction>
                <owl:onProperty rdf:resource="elementIn"/>
                <owl:someValuesFrom rdf:resource="itsStation"/>
            </owl:Restriction>
        </rdfs:subClassOf>
        <skos:historyNote>Introduced in ISO/TS 14812:2022</skos:historyNote>
    </owl:Class>
    <owl:Class rdf:about="its-sApplication">
        <clause>3.2.9.3</clause>
        <skos:prefLabel xml:lang="en">ITS-S application</skos:prefLabel>
        <skos:definition>ITS-S application process (3.2.9.2) residing in the application entity
            (3.1.5.1)</skos:definition>
        <rdfs:subClassOf rdf:resource="its-sApplicationProcess"/>
        <rdfs:subClassOf>
            <owl:Restriction>
                <owl:onProperty rdf:resource="residesIn"/>
                <owl:someValuesFrom rdf:resource="applicationEntity"/>
            </owl:Restriction>
        </rdfs:subClassOf>
        <skos:historyNote>Introduced in ISO/TS 14812:2022</skos:historyNote>
    </owl:Class>
    <owl:Class rdf:about="its-sApplicationImplementation">
        <clause>3.2.9.4</clause>
        <skos:prefLabel xml:lang="en">ITS-S application implementation</skos:prefLabel>
        <skos:definition>implementation of an ITS-S application process (3.2.9.2) within the
            application entity (3.1.5.1)</skos:definition>
        <skos:note>An implementation is typically associated with an implementation
            name, a version and release number.</skos:note>
        <rdfs:subClassOf>
            <owl:Restriction>
                <owl:onProperty rdf:resource="implementationOf"/>
                <owl:someValuesFrom rdf:resource="its-sApplication"/>
            </owl:Restriction>
        </rdfs:subClassOf>
        <skos:historyNote>Introduced in ISO/TS 14812:2022</skos:historyNote>
    </owl:Class>
    <owl:Class rdf:about="its-sApplicationProcessInstallation">
        <clause>3.2.9.5</clause>
        <skos:prefLabel xml:lang="en">ITS-S application process installation</skos:prefLabel>
        <skos:definition>installation of an implementation of an ITS-S application process (3.2.9.2)
            on an ITS station (3.2.7.3)</skos:definition>
        <skos:note>An implementation is typically associated with an implementation
            name, a version and release number.</skos:note>
        <skos:note>An installation is typically associated with a specific licence
            code or serial number.</skos:note>
        <rdfs:subClassOf>
            <owl:Restriction>
                <owl:onProperty rdf:resource="installationOf"/>
                <owl:someValuesFrom rdf:resource="its-sApplicationProcess"/>
            </owl:Restriction>
        </rdfs:subClassOf>
        <skos:historyNote>Introduced in ISO/TS 14812:2022</skos:historyNote>
    </owl:Class>
    <owl:Class rdf:about="its-sApplicationInstallation">
        <clause>3.2.9.6</clause>
        <skos:prefLabel xml:lang="en">ITS-S application installation</skos:prefLabel>
        <skos:definition>ITS-S application process installation (3.2.9.5) within the application
            entity (3.1.5.1)</skos:definition>
        <rdfs:subClassOf rdf:resource="its-sApplicationProcessInstallation"/>
        <skos:historyNote>Introduced in ISO/TS 14812:2022</skos:historyNote>
    </owl:Class>
    <owl:Class rdf:about="actuator">
        <clause>3.2.10.1</clause>
        <skos:prefLabel xml:lang="en">actuator</skos:prefLabel>
        <skos:definition>device (ISO/IEC 24765:2017, 3.1187) with the capability to convert
            meaningful signals (ISO/IEC 24765:2017, 3.3738) into changes to one or more properties
            (ISO/IEC 24765:2017, 3.3207) of a material entity (3.1.1.3)</skos:definition>
        <rdfs:subClassOf>
            <owl:Restriction>
                <owl:onProperty rdf:resource="changesPropertyOf"/>
                <owl:someValuesFrom rdf:resource="materialEntity"/>
            </owl:Restriction>
        </rdfs:subClassOf>
        <skos:historyNote>Introduced in ISO/TS 14812:2025</skos:historyNote>
    </owl:Class>
    <owl:Class rdf:about="sensor">
        <clause>3.2.10.2</clause>
        <skos:prefLabel xml:lang="en">sensor</skos:prefLabel>
        <skos:definition>device (ISO/IEC 24765:2017, 3.1187) with the capability of observing one or
            more properties (ISO/IEC 24765:2017, 3.3207) of a material entity (3.1.1.3) and
            converting those properties into meaningful signals (ISO/IEC 24765:2017, 3.3738)</skos:definition>
        <rdfs:subClassOf>
            <owl:Restriction>
                <owl:onProperty rdf:resource="observesPropertyOf"/>
                <owl:someValuesFrom rdf:resource="materialEntity"/>
            </owl:Restriction>
        </rdfs:subClassOf>
        <skos:historyNote>Introduced in ISO/TS 14812:2025</skos:historyNote>
    </owl:Class>
    <owl:Class rdf:about="cross-section">
        <clause>3.3.1.1</clause>
        <skos:prefLabel xml:lang="en">cross-section</skos:prefLabel>
        <skos:definition>transverse view of road (3.3.5.1) geometry</skos:definition>
        <skos:example>Figure A.28.</skos:example>
        <skos:note>The transverse view provides a vertical section of the ground
            and carriageway (3.3.1.5) at right angles to the centre line of the carriageway.</skos:note>
        <rdfs:subClassOf>
            <owl:Restriction>
                <owl:onProperty rdf:resource="comprises"/>
                <owl:someValuesFrom rdf:resource="roadReservation"/>
            </owl:Restriction>
        </rdfs:subClassOf>
        <skos:historyNote>Introduced in ISO/TS 14812:2022</skos:historyNote>
    </owl:Class>
    <owl:Class rdf:about="roadReservation">
        <clause>3.3.1.2</clause>
        <skos:prefLabel xml:lang="en">road reservation</skos:prefLabel>
        <altPrefLabel xml:lang="en">easement</altPrefLabel>
        <skos:definition>area legally reserved for road (3.3.5.1) transport purposes and support</skos:definition>
        <skos:note>Support includes physical equipment such as safety devices,
            signage and controller cabinets as well as access by maintenance vehicles and personnel.</skos:note>
        <skos:note>The road reservation includes all carriageways (3.3.1.5) as well
            as width to allow for roadside (3.3.1.10) devices, shoulders (3.3.1.18), verges
            (3.3.1.11), footways (3.3.3.3), drainage facilities, sound walls, slopes, embankments,
            etc.</skos:note>
        <rdfs:subClassOf>
            <owl:Restriction>
                <owl:onProperty rdf:resource="comprises"/>
                <owl:someValuesFrom rdf:resource="roadside"/>
            </owl:Restriction>
        </rdfs:subClassOf>
        <rdfs:subClassOf>
            <owl:Restriction>
                <owl:onProperty rdf:resource="comprises"/>
                <owl:someValuesFrom rdf:resource="lane"/>
            </owl:Restriction>
        </rdfs:subClassOf>
        <rdfs:subClassOf>
            <owl:Restriction>
                <owl:onProperty rdf:resource="comprises"/>
                <owl:someValuesFrom rdf:resource="roadway"/>
            </owl:Restriction>
        </rdfs:subClassOf>
        <skos:historyNote>Introduced in ISO/TS 14812:2022</skos:historyNote>
    </owl:Class>
    <owl:Class rdf:about="roadway">
        <clause>3.3.1.3</clause>
        <skos:prefLabel xml:lang="en">roadway</skos:prefLabel>
        <skos:definition>part of the surface of the road reservation (3.3.1.2) primarily designed
            for the movement of vehicles (3.7.1.1) that conform to a specified set of requirements</skos:definition>
        <skos:note>A roadway is characterized using a cross-section (3.3.1.1) of a
            road facility as the roadway characteristics often change along the length of the road.
            See "road" (3.3.5.1), "road section" (3.3.5.7), "road segment" (3.3.5.8), and "road
            link" (3.3.5.6) for different types of stretches of roadway.</skos:note>
        <skos:note>In practice, the roadway design considers a variety of issues,
            which can result in suboptimal road segments that violate normal design guidelines. Such
            locations (3.4.1.1) are typically posted with warning signs, but they are still designed
            for the movement of vehicles.</skos:note>
        <skos:note>While the roadway is designed with certain vehicle
            characteristics in mind, local regulations typically allow a wider set of vehicles to
            use the roadway.</skos:note>
        <skos:note>The roadway includes any contiguous hard shoulders (3.3.1.19),
            hardstanding (3.3.1.17) and reserved lanes (3.3.1.14).</skos:note>
        <rdfs:subClassOf>
            <owl:Restriction>
                <owl:onProperty rdf:resource="comprises"/>
                <owl:someValuesFrom rdf:resource="travelledWay"/>
            </owl:Restriction>
        </rdfs:subClassOf>
        <skos:historyNote>Introduced in ISO/TS 14812:2022</skos:historyNote>
    </owl:Class>
    <owl:Class rdf:about="drivingSpace">
        <clause>3.3.1.4</clause>
        <skos:prefLabel xml:lang="en">driving space</skos:prefLabel>
        <skos:definition>area above the roadway (3.3.1.3) that is primarily designed for the
            movement of vehicles (3.7.1.1)</skos:definition>
        <skos:note>In practice, the driving space design considers a variety of
            issues, which can result in suboptimal road (3.3.5.1) segments that violate normal
            design guidelines. Such locations (3.4.1.1) are typically posted with warning signs, but
            they are still designed for the movement of vehicles.</skos:note>
        <skos:note>While the driving space is designed with certain vehicle
            characteristics in mind, local regulations typically allow a wider set of vehicles to
            use the driving space.</skos:note>
        <rdfs:subClassOf>
            <owl:Restriction>
                <owl:onProperty rdf:resource="areaAbove"/>
                <owl:someValuesFrom rdf:resource="roadway"/>
            </owl:Restriction>
        </rdfs:subClassOf>
        <rdfs:subClassOf>
            <owl:Restriction>
                <owl:onProperty rdf:resource="forMovementOf"/>
                <owl:someValuesFrom rdf:resource="vehicle"/>
            </owl:Restriction>
        </rdfs:subClassOf>
        <skos:historyNote>Introduced in ISO/TS 14812:2022</skos:historyNote>
    </owl:Class>
    <owl:Class rdf:about="carriageway">
        <clause>3.3.1.5</clause>
        <skos:prefLabel xml:lang="en">carriageway</skos:prefLabel>
        <skos:definition>contiguous area of paved roadway (3.3.1.3) designed for the use of vehicles
            along a road segment (3.3.5.8)</skos:definition>
        <skos:note>A carriageway is comprised of one or more traffic lanes
            (3.3.1.13) [i.e. the usable width (3.3.1.15)] and could include shoulders (3.3.1.18) and
            lay-bys (3.3.1.16).</skos:note>
        <skos:note>Carriageways are separated by physical traffic separators
            (3.3.2.1).</skos:note>
        <skos:note>When looking at a cross-section (3.3.1.1) of the road
            reservation (3.3.1.2), the roadway consists of all of the carriageways.</skos:note>
        <rdfs:subClassOf>
            <owl:Restriction>
                <owl:onProperty rdf:resource="comprises"/>
                <owl:minQualifiedCardinality rdf:datatype="xsd:nonNegativeInteger">0</owl:minQualifiedCardinality>
                <owl:onClass rdf:resource="lay-by"/>
            </owl:Restriction>
        </rdfs:subClassOf>
        <rdfs:subClassOf>
            <owl:Restriction>
                <owl:onProperty rdf:resource="comprises"/>
                <owl:minQualifiedCardinality rdf:datatype="xsd:nonNegativeInteger">0</owl:minQualifiedCardinality>
                <owl:onClass rdf:resource="hardstanding"/>
            </owl:Restriction>
        </rdfs:subClassOf>
        <rdfs:subClassOf>
            <owl:Restriction>
                <owl:onProperty rdf:resource="comprises"/>
                <owl:minQualifiedCardinality rdf:datatype="xsd:nonNegativeInteger">0</owl:minQualifiedCardinality>
                <owl:onClass rdf:resource="hardshoulder"/>
            </owl:Restriction>
        </rdfs:subClassOf>
        <rdfs:subClassOf>
            <owl:Restriction>
                <owl:onProperty rdf:resource="comprises"/>
                <owl:someValuesFrom rdf:resource="usableWidth"/>
            </owl:Restriction>
        </rdfs:subClassOf>
        <skos:historyNote>Introduced in ISO/TS 14812:2022</skos:historyNote>
    </owl:Class>
    <owl:Class rdf:about="travelledWay">
        <clause>3.3.1.6</clause>
        <skos:prefLabel xml:lang="en">travelled way</skos:prefLabel>
        <skos:definition>part of the roadway (3.3.1.3) that is currently intended for transport
            purposes</skos:definition>
        <skos:note>The travelled way does not include hard shoulders (3.3.1.19),
            hardstanding (3.3.1.17), or other areas that are not currently intended for normal
            operational use. In other words, while these other areas are "designed" for transport
            purposes, they are not "intended" for normal transport purposes (at present); rather
            these extra areas exist for safety and other exceptional use conditions.</skos:note>
        <skos:note>While the limits of the roadway are defined by the design of the
            physical infrastructure and are generally static; the limits of the travelled way can be
            dynamic, such as in the case of a hard shoulder for emergency use (3.3.4.1) being
            converted into hard shoulder running (3.3.4.2) operation.</skos:note>
        <skos:historyNote>Introduced in ISO/TS 14812:2022</skos:historyNote>
    </owl:Class>
    <owl:Class rdf:about="singleCarriageway">
        <clause>3.3.1.7</clause>
        <skos:prefLabel xml:lang="en">single carriageway</skos:prefLabel>
        <skos:definition>having exactly one carriageway (3.3.1.5)</skos:definition>
        <skos:note>The "single carriageway" term can be used to describe a road,
            road section, road link, or road segment.</skos:note>
        <skos:note>A single carriageway road segment could have multiple lanes
            (3.3.1.12) and could allow travel in opposite directions</skos:note>
        <rdfs:subClassOf rdf:resource="roadway"/>
        <rdfs:subClassOf>
            <owl:Restriction>
                <owl:onProperty rdf:resource="comprises"/>
                <owl:qualifiedCardinality rdf:datatype="xsd:nonNegativeInteger">1</owl:qualifiedCardinality>
                <owl:onClass rdf:resource="carriageway"/>
            </owl:Restriction>
        </rdfs:subClassOf>
        <skos:historyNote>Introduced in ISO/TS 14812:2022</skos:historyNote>
    </owl:Class>
    <owl:Class rdf:about="dualCarriageway">
        <clause>3.3.1.8</clause>
        <skos:prefLabel xml:lang="en">dual carriageway</skos:prefLabel>
        <skos:definition>having exactly two carriageways (3.3.1.5)</skos:definition>
        <skos:note>The "dual carriageway" term can be used to describe a road, road
            section, road link, or road segment.</skos:note>
        <skos:note>The two carriageways are typically designed for travel in
            opposite directions.</skos:note>
        <rdfs:subClassOf rdf:resource="roadway"/>
        <rdfs:subClassOf>
            <owl:Restriction>
                <owl:onProperty rdf:resource="comprises"/>
                <owl:qualifiedCardinality rdf:datatype="xsd:nonNegativeInteger">2</owl:qualifiedCardinality>
                <owl:onClass rdf:resource="carriageway"/>
            </owl:Restriction>
        </rdfs:subClassOf>
        <rdfs:subClassOf>
            <owl:Restriction>
                <owl:onProperty rdf:resource="has"/>
                <owl:qualifiedCardinality rdf:datatype="xsd:nonNegativeInteger">1</owl:qualifiedCardinality>
                <owl:onClass rdf:resource="physicalTrafficSeparator"/>
            </owl:Restriction>
        </rdfs:subClassOf>
        <skos:historyNote>Introduced in ISO/TS 14812:2022</skos:historyNote>
    </owl:Class>
    <owl:Class rdf:about="multipleCarriageway">
        <clause>3.3.1.9</clause>
        <skos:prefLabel xml:lang="en">multiple carriageway</skos:prefLabel>
        <skos:definition>having more than one carriageway (3.3.1.5)</skos:definition>
        <skos:note>The "multiple carriageway" term can be used to describe a road,
            road section, road link, or road segment.</skos:note>
        <skos:note>The separate carriageways are typically designed for separate
            traffic for (often multiple) specific operational reasons, such as direction of travel,
            category of vehicle (e.g. high occupancy vehicle), local versus through travel, etc.</skos:note>
        <rdfs:subClassOf rdf:resource="roadway"/>
        <rdfs:subClassOf>
            <owl:Restriction>
                <owl:onProperty rdf:resource="comprises"/>
                <owl:minQualifiedCardinality rdf:datatype="xsd:nonNegativeInteger">3</owl:minQualifiedCardinality>
                <owl:onClass rdf:resource="carriageway"/>
            </owl:Restriction>
        </rdfs:subClassOf>
        <rdfs:subClassOf>
            <owl:Restriction>
                <owl:onProperty rdf:resource="has"/>
                <owl:minQualifiedCardinality rdf:datatype="xsd:nonNegativeInteger">2</owl:minQualifiedCardinality>
                <owl:onClass rdf:resource="physicalTrafficSeparator"/>
            </owl:Restriction>
        </rdfs:subClassOf>
        <skos:historyNote>Introduced in ISO/TS 14812:2022</skos:historyNote>
    </owl:Class>
    <owl:Class rdf:about="roadside">
        <clause>3.3.1.10</clause>
        <skos:prefLabel xml:lang="en">roadside</skos:prefLabel>
        <skos:definition>portion of the road reservation (3.3.1.2) excluding all roadway (3.3.1.3)
            and driving space(s) (3.3.1.4)</skos:definition>
        <skos:note>Roadside, shoulder (3.3.1.18) and verge (3.3.1.11) define
            similar but slightly different concepts</skos:note>
        <rdfs:subClassOf>
            <owl:Restriction>
                <owl:onProperty rdf:resource="comprises"/>
                <owl:someValuesFrom rdf:resource="verge"/>
            </owl:Restriction>
        </rdfs:subClassOf>
        <skos:historyNote>Introduced in ISO/TS 14812:2022</skos:historyNote>
    </owl:Class>
    <owl:Class rdf:about="verge">
        <clause>3.3.1.11</clause>
        <skos:prefLabel xml:lang="en">verge</skos:prefLabel>
        <skos:definition>unpaved part of the roadside (3.3.1.10) designed for travel safety purposes</skos:definition>
        <skos:note>A verge can separate two lanes (3.3.1.12) of different modes,
            separate a traffic lane (3.3.1.13) from a ditch, or separate a lane from another safety
            hazard.</skos:note>
        <skos:note>Roadside, shoulder (3.3.1.18) and verge define similar but
            slightly different concepts.</skos:note>
        <skos:historyNote>Introduced in ISO/TS 14812:2022</skos:historyNote>
    </owl:Class>
    <owl:Class rdf:about="lane">
        <clause>3.3.1.12</clause>
        <skos:prefLabel xml:lang="en">lane</skos:prefLabel>
        <altPrefLabel xml:lang="en">generic lane</altPrefLabel>
        <skos:definition>&lt;generic&gt; portion of road reservation (3.3.1.2) intended to
            accommodate a single line of moving material entities (3.1.1.3) along its length</skos:definition>
        <skos:example>Traffic lane (3.3.1.13), cycle lane (3.3.3.1), sidewalk (3.3.3.4).</skos:example>
        <skos:note>Lanes (3.3.1.12) are often bounded by lane markings.</skos:note>
        <skos:note>Lanes may be significantly wider than the normal vehicle width
            to allow variance in lane position of the vehicle as well as for various vehicle
            dimensions.</skos:note>
        <skos:note>The "lane" nomenclature typically refers to motor vehicle
            (3.7.6.3) usage, but can also refer to other purposes, such as sidewalks (3.3.3.4).</skos:note>
        <skos:historyNote>Introduced in ISO/TS 14812:2022</skos:historyNote>
    </owl:Class>
    <owl:Class rdf:about="trafficLane">
        <clause>3.3.1.13</clause>
        <skos:prefLabel xml:lang="en">traffic lane</skos:prefLabel>
        <altPrefLabel xml:lang="en">lane</altPrefLabel>
        <skos:definition>portion of carriageway (3.3.1.5) designed to accommodate a single line of
            moving road vehicles (3.7.6.1)</skos:definition>
        <skos:note>The term "lane" is often used to refer to a "traffic lane" when
            the context is known to be "traffic".</skos:note>
        <skos:note>A traffic lane can be bi-directional, such as a single lane road
            (3.3.5.1), a two-way turn/overtaking lane, or a reversible flow lane.</skos:note>
        <skos:note>Some jurisdictions allow supplemental uses of a traffic lane,
            such as multiple motorcycles sharing the width of a traffic lane or allowing a bicycle
            to use the edge of a lane.</skos:note>
        <rdfs:subClassOf rdf:resource="lane"/>
        <skos:historyNote>Introduced in ISO/TS 14812:2022</skos:historyNote>
    </owl:Class>
    <owl:Class rdf:about="reservedLane">
        <clause>3.3.1.14</clause>
        <skos:prefLabel xml:lang="en">reserved lane</skos:prefLabel>
        <skos:definition>traffic lane (3.3.1.13) restricted to a specific subset of road vehicles
            (3.7.6.1) or user (3.5.1.3) categories</skos:definition>
        <skos:example>1 Bus lane.</skos:example>
        <skos:example>2 High-occupancy vehicle lane.</skos:example>
        <skos:note>A traffic lane may be reserved permanently or under certain
            conditions or times.</skos:note>
        <rdfs:subClassOf rdf:resource="trafficLane"/>
        <skos:historyNote>Introduced in ISO/TS 14812:2022</skos:historyNote>
    </owl:Class>
    <owl:Class rdf:about="usableWidth">
        <clause>3.3.1.15</clause>
        <skos:prefLabel xml:lang="en">usable width</skos:prefLabel>
        <skos:definition>all traffic lanes (3.3.1.13) of a carriageway (3.3.1.5)</skos:definition>
        <rdfs:subClassOf>
            <owl:Restriction>
                <owl:onProperty rdf:resource="comprises"/>
                <owl:someValuesFrom rdf:resource="trafficLane"/>
            </owl:Restriction>
        </rdfs:subClassOf>
        <skos:historyNote>Introduced in ISO/TS 14812:2022</skos:historyNote>
    </owl:Class>
    <owl:Class rdf:about="lay-by">
        <clause>3.3.1.16</clause>
        <skos:prefLabel xml:lang="en">lay-by</skos:prefLabel>
        <skos:definition>short length of paved carriageway (3.3.1.5) at its edge designed to allow a
            vehicle (3.7.1.1) to draw out of the traffic lanes (3.3.1.13) and stop temporarily</skos:definition>
        <skos:note>Lay-bys are not part of a hard shoulder (3.3.1.19).</skos:note>
        <skos:note>Lay-bys can be used for emergency situations, picking
            up/dropping off passengers (3.6.2.1), etc.</skos:note>
        <skos:historyNote>Introduced in ISO/TS 14812:2022</skos:historyNote>
    </owl:Class>
    <owl:Class rdf:about="hardstanding">
        <clause>3.3.1.17</clause>
        <skos:prefLabel xml:lang="en">hardstanding</skos:prefLabel>
        <skos:definition>part of a paved carriageway (3.3.1.5) that is not a traffic lane
            (3.3.1.13), hard shoulder (3.3.1.19), or lay-by (3.3.1.16).</skos:definition>
        <skos:example>See Figure A.23.</skos:example>
        <skos:note>Hardstanding can include edges of a hard shoulder outside of
            designated lane markings, slips for future connector roads (3.3.5.1), etc.</skos:note>
        <skos:historyNote>Introduced in ISO/TS 14812:2022</skos:historyNote>
    </owl:Class>
    <owl:Class rdf:about="shoulder">
        <clause>3.3.1.18</clause>
        <skos:prefLabel xml:lang="en">shoulder</skos:prefLabel>
        <skos:definition>either a hard shoulder (3.3.1.19) or a soft shoulder (3.3.1.20)</skos:definition>
        <skos:note>In some jurisdictions, a shoulder can be used for emergency
            stops and/or other purposes in addition to providing a clear zone for safety purposes.</skos:note>
        <skos:note>Roadside (3.3.1.10), shoulder, and verge (3.3.1.11) define
            similar but slightly different concepts</skos:note>
        <skos:historyNote>Introduced in ISO/TS 14812:2022</skos:historyNote>
    </owl:Class>
    <owl:Class rdf:about="hardShoulder">
        <clause>3.3.1.19</clause>
        <skos:prefLabel xml:lang="en">hard shoulder</skos:prefLabel>
        <skos:definition>part of the paved carriageway (3.3.1.5) designed to support traffic loads
            but not normally intended for driving</skos:definition>
        <skos:note>A hard shoulder can be narrow or wide enough for a traffic lane
            (3.3.1.13).</skos:note>
        <skos:note>A hard shoulder can have a surface that discourages usage as a
            driving surface in some countries.</skos:note>
        <rdfs:subClassOf rdf:resource="shoulder"/>
        <skos:historyNote>Introduced in ISO/TS 14812:2022</skos:historyNote>
    </owl:Class>
    <owl:Class rdf:about="softShoulder">
        <clause>3.3.1.20</clause>
        <skos:prefLabel xml:lang="en">soft shoulder</skos:prefLabel>
        <skos:definition>unpaved part of the road reservation (3.3.1.2) not belonging to the
            carriageway (3.3.1.5) but providing lateral support to it</skos:definition>
        <skos:note>Soft shoulders are not normally intended for driving.</skos:note>
        <skos:note>Soft shoulders often have a grass or gravel surface.</skos:note>
        <rdfs:subClassOf rdf:resource="shoulder"/>
        <skos:historyNote>Introduced in ISO/TS 14812:2022</skos:historyNote>
    </owl:Class>
    <owl:Class rdf:about="motorway">
        <clause>3.3.1.21</clause>
        <skos:prefLabel xml:lang="en">motorway</skos:prefLabel>
        <skos:altLabel xml:lang="en">interstate highway</skos:altLabel>
        <skos:altLabel xml:lang="en">freeway</skos:altLabel>
        <skos:definition>road (3.3.5.1) with separate carriageways for each direction, with limited
            access that prevents cross traffic on the same level, and for the exclusive use of
            certain classes of motor vehicles</skos:definition>
        <skos:note>The terms "interstate highway" and "freeway" are US terms.</skos:note>
        <rdfs:subClassOf rdf:resource="road"/>
        <skos:historyNote>Introduced in ISO/TS 14812:2025</skos:historyNote>
    </owl:Class>
    <owl:Class rdf:about="physicalTrafficSeparator">
        <clause>3.3.2.1</clause>
        <skos:prefLabel xml:lang="en">physical traffic separator</skos:prefLabel>
        <skos:definition>mechanism used to physically separate a travelled way or pathway from the
            adjacent environment</skos:definition>
        <skos:note>Mechanisms include various types of barriers, such as walls,
            rails, pylons, kerbs and ditches, as well as open, unpaved space. If two streams of
            traffic are only separated by paved space (including any markings and rumble strips),
            they share a common carriageway.</skos:note>
        <skos:note>The adjacent environment can be an opposing direction of travel,
            a different mode of travel, the edge of a bridge, etc.</skos:note>
        <skos:historyNote>Introduced in ISO/TS 14812:2022</skos:historyNote>
    </owl:Class>
    <owl:Class rdf:about="centralReservation">
        <clause>3.3.2.2</clause>
        <skos:prefLabel xml:lang="en">central reservation</skos:prefLabel>
        <skos:altLabel xml:lang="en">median</skos:altLabel>
        <skos:altLabel xml:lang="en">median strip</skos:altLabel>
        <skos:altLabel xml:lang="en">neutral ground</skos:altLabel>
        <skos:definition>part of the road reservation (3.3.1.2) between carriageways (3.3.1.5)
            designed for travel safety purposes</skos:definition>
        <skos:note>A central reservation can be paved or unpaved and can be
            equipped with a safety barrier, rails, or other devices.</skos:note>
        <rdfs:subClassOf rdf:resource="physicalTrafficSeparator"/>
        <skos:historyNote>Introduced in ISO/TS 14812:2022</skos:historyNote>
    </owl:Class>
    <owl:Class rdf:about="jerseyBarrier">
        <clause>3.3.2.3</clause>
        <skos:prefLabel xml:lang="en">Jersey barrier</skos:prefLabel>
        <skos:altLabel xml:lang="en">city block</skos:altLabel>
        <skos:altLabel xml:lang="en">concrete barrier</skos:altLabel>
        <skos:definition>physical traffic separator (3.3.2.1) that consists of a wall with a wide,
            sloped base designed to divert vehicles (3.7.1.1) back into their traffic lane
            (3.3.1.13)</skos:definition>
        <skos:note>Jersey barriers are typically modular. They are typically made
            of concrete but can also be made with other materials such as plastic filled with water
            or sand.</skos:note>
        <rdfs:subClassOf rdf:resource="physicalTrafficSeparator"/>
        <skos:historyNote>Introduced in ISO/TS 14812:2022</skos:historyNote>
    </owl:Class>
    <owl:Class rdf:about="kerb">
        <clause>3.3.2.4</clause>
        <skos:prefLabel xml:lang="en">kerb</skos:prefLabel>
        <skos:altLabel xml:lang="en">curb</skos:altLabel>
        <skos:definition>physical traffic separator, usually upstanding, at the edge of a
            carriageway, hard strip, hard shoulder, or footway Note 1 to entry: "Curb" is the US
            spelling.</skos:definition>
        <rdfs:subClassOf rdf:resource="physicalTrafficSeparator"/>
        <skos:historyNote>Introduced in ISO/TS 14812:2025</skos:historyNote>
    </owl:Class>
    <owl:Class rdf:about="cycleLane">
        <clause>3.3.3.1</clause>
        <skos:prefLabel xml:lang="en">cycle lane</skos:prefLabel>
        <skos:definition>lane (3.3.1.12) designed for the through movement of cycles</skos:definition>
        <skos:note>Cycle lanes are typically much narrower than traffic lanes
            (3.3.1.13).</skos:note>
        <skos:note>Cycle lanes are typically part of either a carriageway
            (3.3.1.15) or a cycleway (3.3.3.2).</skos:note>
        <skos:note>Cycle lanes could also allow and be designed for motorized
            vehicles (3.7.6.2) (e.g. e-scooters, mopeds, etc.) with similar performance
            characteristics as human-powered cycles, subject to local regulations.</skos:note>
        <rdfs:subClassOf rdf:resource="lane"/>
        <skos:historyNote>Introduced in ISO/TS 14812:2022</skos:historyNote>
    </owl:Class>
    <owl:Class rdf:about="cycleway">
        <clause>3.3.3.2</clause>
        <skos:prefLabel xml:lang="en">cycleway</skos:prefLabel>
        <altPrefLabel xml:lang="en">cycle track</altPrefLabel>
        <skos:definition>infrastructure primarily designed for the use of cycles and separate from a
            carriageway (3.3.1.5)</skos:definition>
        <skos:note>Local legislation can allow cycleways to be used by a variety of
            low-speed vehicles (3.7.5.2) (e.g. low-speed scooters, skateboards, etc.) and can share
            usage of other low-speed modes such as pedestrians (3.6.1.4), horseback riders, etc.</skos:note>
        <rdfs:subClassOf>
            <owl:Restriction>
                <owl:onProperty rdf:resource="comprises"/>
                <owl:someValuesFrom rdf:resource="cycleLane"/>
            </owl:Restriction>
        </rdfs:subClassOf>
        <skos:historyNote>Introduced in ISO/TS 14812:2022</skos:historyNote>
    </owl:Class>
    <owl:Class rdf:about="footpath">
        <clause>3.3.3.3</clause>
        <skos:prefLabel xml:lang="en">footpath</skos:prefLabel>
        <skos:definition>area designed for the longitudinal movement of pedestrians</skos:definition>
        <skos:note>Regulations typically allow footpaths to be used by other
            ultra-low speed users (3.5.1.3), such as the users of wheelchairs and strollers.</skos:note>
        <skos:historyNote>Introduced in ISO/TS 14812:2022; revised in 2025 to distinguish between a 
            footpath, which can be crossing areas and footways, which are curvilinear and form lanes.</skos:historyNote>
    </owl:Class>
    <owl:Class rdf:about="sidewalk">
        <clause>3.3.3.4</clause>
        <skos:prefLabel xml:lang="en">sidewalk</skos:prefLabel>
        <altPrefLabel xml:lang="en">footway</altPrefLabel>
        <skos:altLabel xml:lang="en">pavement</skos:altLabel>
        <skos:definition>footpath (3.3.3.3) along a roadside (3.3.1.10)</skos:definition>
        <skos:note>A paved footway is called a "pavement" in the British English.</skos:note>
        <rdfs:subClassOf rdf:resource="lane"/>
        <rdfs:subClassOf rdf:resource="footpath"/>
        <rdfs:subClassOf>
            <owl:Restriction>
                <owl:onProperty rdf:resource="along"/>
                <owl:someValuesFrom rdf:resource="roadside"/>
            </owl:Restriction>
        </rdfs:subClassOf>
        <skos:historyNote>Introduced in ISO/TS 14812:2022; footway added as a synonym in 2025.</skos:historyNote>
    </owl:Class>
    <owl:Class rdf:about="escalator">
        <clause>3.3.3.5</clause>
        <skos:prefLabel xml:lang="en">escalator</skos:prefLabel>
        <skos:definition>rising or falling stairway that assists pedestrians in vertical transitions</skos:definition>
        <rdfs:subClassOf rdf:resource="footpath"/>
        <skos:historyNote>Introduced in ISO/TS 14812:2025</skos:historyNote>
    </owl:Class>
    <owl:Class rdf:about="movingWalkway">
        <clause>3.3.3.6</clause>
        <skos:prefLabel xml:lang="en">moving walkway</skos:prefLabel>
        <skos:altLabel xml:lang="en">travellator</skos:altLabel>
        <skos:definition>footpath consisting of a conveyor belt for pedestrians Note 1 to entry:
            Moving walkways are often used in airports with long footpaths Note 2 to entry: Moving
            walkways assist pedestrians in traversing longer distances. Note 3 to entry:
            "Travellator" is a term used in Singapore.</skos:definition>
        <rdfs:subClassOf rdf:resource="footpath"/>
        <skos:historyNote>Introduced in ISO/TS 14812:2025</skos:historyNote>
    </owl:Class>
    <owl:Class rdf:about="pedestrianCrossing">
        <clause>3.3.3.7</clause>
        <skos:prefLabel xml:lang="en">pedestrian crossing</skos:prefLabel>
        <altPrefLabel xml:lang="en">crosswalk</altPrefLabel>
        <skos:definition>physically marked location to enhance the safety of pedestrians crossing
            one or more lanes of a different mode of travel</skos:definition>
        <skos:note>Pedestrian permission and/or priority at crossing can be managed
            when traffic signals are present.</skos:note>
        <skos:note>In some cases, local regulations can require vehicles to give
            way to the pedestrians in the pedestrian crossing and/or restrict pedestrians to only
            cross at pedestrian crossings.</skos:note>
        <rdfs:subClassOf rdf:resource="footpath"/>
        <skos:historyNote>Introduced in ISO/TS 14812:2025</skos:historyNote>
    </owl:Class>
    <owl:Class rdf:about="sharedSpace">
        <clause>3.3.3.8</clause>
        <skos:prefLabel xml:lang="en">shared space</skos:prefLabel>
        <skos:definition>public area space for use by users with distinctly different
            characteristics</skos:definition>
        <skos:example>facility designed for the use of pedestrians, cycles, and motor
            vehicles</skos:example>
        <skos:note>The space can be for travel, gatherings, rest, or other purposes.</skos:note>
        <skos:historyNote>Introduced in ISO/TS 14812:2025</skos:historyNote>
    </owl:Class>
    <owl:Class rdf:about="blockFace">
        <clause>3.3.3.9</clause>
        <skos:prefLabel xml:lang="en">block-face</skos:prefLabel>
        <skos:definition>extent of sidewalk on one side of a street between two consecutive
            intersections crossing that street</skos:definition>
        <rdfs:subClassOf>
            <owl:Restriction>
                <owl:onProperty rdf:resource="extentOf"/>
                <owl:someValuesFrom rdf:resource="sidewalk"/>
            </owl:Restriction>
        </rdfs:subClassOf>
        <rdfs:subClassOf>
            <owl:Restriction>
                <owl:onProperty rdf:resource="startsAt"/>
                <owl:someValuesFrom rdf:resource="intersection"/>
            </owl:Restriction>
        </rdfs:subClassOf>
        <rdfs:subClassOf>
            <owl:Restriction>
                <owl:onProperty rdf:resource="endsAt"/>
                <owl:someValuesFrom rdf:resource="intersection"/>
            </owl:Restriction>
        </rdfs:subClassOf>
        <skos:historyNote>Introduced in ISO/TS 14812:2025</skos:historyNote>
    </owl:Class>
    <owl:Class rdf:about="hardShoulderForEmergencyUse">
        <clause>3.3.4.1</clause>
        <skos:prefLabel xml:lang="en">hard shoulder for emergency use</skos:prefLabel>
        <skos:definition>operating mode of a hard shoulder (3.3.1.19) that allows operation of
            emergency, construction, maintenance, or other special use vehicles (3.7.1.1) or for
            emergency stopping and is prohibited for other vehicle usage</skos:definition>
        <rdfs:subClassOf>
            <owl:Restriction>
                <owl:onProperty rdf:resource="operatingModeOf"/>
                <owl:someValuesFrom rdf:resource="hardShoulder"/>
            </owl:Restriction>
        </rdfs:subClassOf>
        <skos:historyNote>Introduced in ISO/TS 14812:2022</skos:historyNote>
    </owl:Class>
    <owl:Class rdf:about="hardShoulderRunning">
        <clause>3.3.4.2</clause>
        <skos:prefLabel xml:lang="en">hard shoulder running</skos:prefLabel>
        <skos:definition>operating mode of a hard shoulder (3.3.1.19) that allows operation of
            general-purpose motor vehicles (3.7.6.3) as an extra lane (3.3.1.12)</skos:definition>
        <rdfs:subClassOf>
            <owl:Restriction>
                <owl:onProperty rdf:resource="operatingModeOf"/>
                <owl:someValuesFrom rdf:resource="hardShoulder"/>
            </owl:Restriction>
        </rdfs:subClassOf>
        <skos:historyNote>Introduced in ISO/TS 14812:2022</skos:historyNote>
    </owl:Class>
    <owl:Class rdf:about="road">
        <clause>3.3.5.1</clause>
        <skos:prefLabel xml:lang="en">road</skos:prefLabel>
        <skos:definition>curvilinear length of roadway (3.3.1.3) that shares the same road
            identifier (3.3.5.13)</skos:definition>
        <skos:note>A length of the road network (3.3.5.2) may be referenced by
            multiple designators (e.g. Main Street and Route 7). In this case, there would be two
            "roads" that share the same set of "carriageways" (3.3.1.5).</skos:note>
        <skos:note>A road can change directions at a junction (3.3.6.2).</skos:note>
        <skos:note>The identification is generally a name or number.</skos:note>
        <skos:historyNote>Introduced in ISO/TS 14812:2022</skos:historyNote>
    </owl:Class>
    <owl:Class rdf:about="roadNetwork">
        <clause>3.3.5.2</clause>
        <skos:prefLabel xml:lang="en">road network</skos:prefLabel>
        <skos:definition>interconnected collection of roads (3.3.5.1)</skos:definition>
        <rdfs:subClassOf>
            <owl:Restriction>
                <owl:onProperty rdf:resource="aggregates"/>
                <owl:someValuesFrom rdf:resource="road"/>
            </owl:Restriction>
        </rdfs:subClassOf>
        <skos:historyNote>Introduced in ISO/TS 14812:2022</skos:historyNote>
    </owl:Class>
    <owl:Class rdf:about="roadModel">
        <clause>3.3.5.3</clause>
        <skos:prefLabel xml:lang="en">road model</skos:prefLabel>
        <skos:definition>representation of a road network (3.3.5.2)</skos:definition>
        <skos:note>Road models for different systems (3.1.2.1) will often define
            different models. For example, a public transport system (3.1.2.2) can define road links
            (3.3.5.6) based on the location (3.4.1.1) of bus stops while a traffic system can define
            road links based on the location of junctions (3.3.6.2).</skos:note>
        <rdfs:subClassOf>
            <owl:Restriction>
                <owl:onProperty rdf:resource="represents"/>
                <owl:someValuesFrom rdf:resource="roadNetwork"/>
            </owl:Restriction>
        </rdfs:subClassOf>
        <rdfs:subClassOf>
            <owl:Restriction>
                <owl:onProperty rdf:resource="constitutes"/>
                <owl:someValuesFrom rdf:resource="node"/>
            </owl:Restriction>
        </rdfs:subClassOf>
        <rdfs:subClassOf>
            <owl:Restriction>
                <owl:onProperty rdf:resource="constitutes"/>
                <owl:someValuesFrom rdf:resource="link"/>
            </owl:Restriction>
        </rdfs:subClassOf>
        <skos:historyNote>Introduced in ISO/TS 14812:2022</skos:historyNote>
    </owl:Class>
    <owl:Class rdf:about="node">
        <clause>3.3.5.4</clause>
        <skos:prefLabel xml:lang="en">node</skos:prefLabel>
        <altPrefLabel xml:lang="en">road network node</altPrefLabel>
        <skos:definition>&lt;road network&gt; component of a road model (3.3.5.3) representing a
            point location (3.4.1.3) of the road network (3.3.5.2) graph</skos:definition>
        <skos:note>The point location typically represents a point along the road
            (3.3.5.1) which can be used to designate the location (3.4.1.1) of a junction (3.3.6.2),
            public transport (3.5.6.1) stop, jurisdictional boundary, termination point, etc.</skos:note>
        <skos:historyNote>Introduced in ISO/TS 14812:2022</skos:historyNote>
    </owl:Class>
    <owl:Class rdf:about="link">
        <clause>3.3.5.5</clause>
        <skos:prefLabel xml:lang="en">link</skos:prefLabel>
        <skos:definition>&lt;road network&gt; component of a road model (3.3.5.3) that represents a
            connection between two nodes (3.3.5.4)</skos:definition>
        <skos:note>A link can be curvilinear and can have various attributes such
            as width.</skos:note>
        <rdfs:subClassOf>
            <owl:Restriction>
                <owl:onProperty rdf:resource="connects"/>
                <owl:qualifiedCardinality rdf:datatype="xsd:nonNegativeInteger">2</owl:qualifiedCardinality>
                <owl:onClass rdf:resource="instant"/>
            </owl:Restriction>
        </rdfs:subClassOf>
        <skos:historyNote>Introduced in ISO/TS 14812:2022</skos:historyNote>
    </owl:Class>
    <owl:Class rdf:about="roadLink">
        <clause>3.3.5.6</clause>
        <skos:prefLabel xml:lang="en">road link</skos:prefLabel>
        <skos:definition>link (3.3.5.5) representing a contiguous length of a road (3.3.5.1) between
            two nodes (3.3.5.4) of operational or managerial significance</skos:definition>
        <skos:note>The operational characteristics of the nodes would relate to the
            type of road model (3.3.5.3). For example, a traffic system (3.1.2.1) can base its road
            links on nodes that represent junctions (3.3.6.2) and road terminators (3.1.8.3).</skos:note>
        <rdfs:subClassOf rdf:resource="link"/>
        <rdfs:subClassOf>
            <owl:Restriction>
                <owl:onProperty rdf:resource="aggregates"/>
                <owl:someValuesFrom rdf:resource="laneLink"/>
            </owl:Restriction>
        </rdfs:subClassOf>
        <rdfs:subClassOf>
            <owl:Restriction>
                <owl:onProperty rdf:resource="constitutes"/>
                <owl:someValuesFrom rdf:resource="roadSegment"/>
            </owl:Restriction>
        </rdfs:subClassOf>
        <skos:historyNote>Introduced in ISO/TS 14812:2022</skos:historyNote>
    </owl:Class>
    <owl:Class rdf:about="roadSection">
        <clause>3.3.5.7</clause>
        <skos:prefLabel xml:lang="en">road section</skos:prefLabel>
        <skos:definition>aggregation of one or more road links (3.3.5.6) that represents a
            contiguous length of a road (3.3.5.1) that shares the same management and operational
            strategies</skos:definition>
        <skos:example>1 A traffic signal timing plan is applied to one road section.</skos:example>
        <skos:example>2 A speed limit regulation can be applied to a road section.</skos:example>
        <skos:note>Different road models (3.3.5.3) can divide the same road into
            different road sections.</skos:note>
        <rdfs:subClassOf>
            <owl:Restriction>
                <owl:onProperty rdf:resource="aggregates"/>
                <owl:someValuesFrom rdf:resource="roadLink"/>
            </owl:Restriction>
        </rdfs:subClassOf>
        <skos:historyNote>Introduced in ISO/TS 14812:2022</skos:historyNote>
    </owl:Class>
    <owl:Class rdf:about="roadSegment">
        <clause>3.3.5.8</clause>
        <skos:prefLabel xml:lang="en">road segment</skos:prefLabel>
        <skos:definition>link (3.3.5.5) that represents a contiguous length of a road link (3.3.5.6)
            characterized by the same physical characteristics</skos:definition>
        <skos:note>The definition of road segments is highly dependent on which
            characteristics are modelled by the implementation. Characteristics that can result in a
            new road segment include addition or subtraction of a lane (3.3.1.12), a change in
            roadway (3.3.1.3) width, the change of road (3.3.5.1) type (e.g. start/end of a bridge),
            etc.</skos:note>
        <rdfs:subClassOf rdf:resource="link"/>
        <skos:historyNote>Introduced in ISO/TS 14812:2022</skos:historyNote>
    </owl:Class>
    <owl:Class rdf:about="laneLink">
        <clause>3.3.5.9</clause>
        <skos:prefLabel xml:lang="en">lane link</skos:prefLabel>
        <skos:definition>link (3.3.5.5) that represents a lane (3.3.1.12) of a road link (3.3.5.6)</skos:definition>
        <skos:note>A lane segment (3.3.5.10) can start or end at locations
            (3.4.1.1) other than the start or end of the corresponding road segment (3.3.5.8) (e.g.
            a lane can start mid-block).</skos:note>
        <skos:note>A lane segment only includes the sequential (3.5.9.2) lane
            links, it does not include lane links from adjacent lanes.</skos:note>
        <rdfs:subClassOf rdf:resource="link"/>
        <rdfs:subClassOf>
            <owl:Restriction>
                <owl:onProperty rdf:resource="constitutes"/>
                <owl:someValuesFrom rdf:resource="laneSegment"/>
            </owl:Restriction>
        </rdfs:subClassOf>
        <skos:historyNote>Introduced in ISO/TS 14812:2022</skos:historyNote>
    </owl:Class>
    <owl:Class rdf:about="laneSegment">
        <clause>3.3.5.10</clause>
        <skos:prefLabel xml:lang="en">lane segment</skos:prefLabel>
        <skos:definition>link (3.3.5.1) that represents a contiguous length of a lane link (3.3.5.9)
            characterized by the same physical characteristics</skos:definition>
        <rdfs:subClassOf rdf:resource="link"/>
        <skos:historyNote>Introduced in ISO/TS 14812:2022</skos:historyNote>
    </owl:Class>
    <owl:Class rdf:about="alley">
        <clause>3.3.5.11</clause>
        <skos:prefLabel xml:lang="en">alley</skos:prefLabel>
        <skos:definition>road (3.3.1.2) that has buildings, walls or fences on each side</skos:definition>
        <rdfs:subClassOf rdf:resource="road"/>
        <skos:historyNote>Introduced in ISO/TS 14812:2025</skos:historyNote>
    </owl:Class>
    <owl:Class rdf:about="roadIdentifier">
        <clause>3.3.5.12</clause>
        <skos:prefLabel xml:lang="en">road identifier</skos:prefLabel>
        <skos:definition>designator by a road authority to uniquely identify one or more curvilinear
            lengths of roadway (3.3.5.3) within the context of the road authority</skos:definition>
        <skos:note>A single road identifier can be assigned to non-contiguous lengths of roadway.</skos:note>
        <skos:note>The same road identifier can be allocated by different road authorities to
            different, physically distinct, curvilinear lengths of roadway.</skos:note>
        <skos:note>The identifier is typically either a name (e.g., Main Street), a class of road coupled with
            a number (e.g., "M25" meaning "motorway no. 25").</skos:note>
        <rdfs:subClassOf>
            <owl:Restriction>
                <owl:onProperty rdf:resource="identifies"/>
                <owl:someValuesFrom rdf:resource="road"/>
            </owl:Restriction>
        </rdfs:subClassOf>
        <skos:historyNote>Introduced in ISO/TS 14812:2025</skos:historyNote>
    </owl:Class>
    <owl:Class rdf:about="serviceRoad">
        <clause>3.3.5.13</clause>
        <skos:prefLabel xml:lang="en">service road</skos:prefLabel>
        <skos:definition>road designed to facilitate the provision of services to customers</skos:definition>
        <skos:example>road used to access parking spaces or pick-up/drop-off area</skos:example>
        <rdfs:subClassOf rdf:resource="road"/>
        <skos:historyNote>Introduced in ISO/TS 14812:2025</skos:historyNote>
    </owl:Class>
    <owl:Class rdf:about="serviceAlley">
        <clause>3.3.5.14</clause>
        <skos:prefLabel xml:lang="en">service alley</skos:prefLabel>
        <skos:definition>alley designed to facilitate the provision of services for adjacent
            locations</skos:definition>
        <skos:example>alley for trash collection</skos:example>
        <skos:example>alley that provides access to an electrical substation</skos:example>
        <rdfs:subClassOf rdf:resource="alley"/>
        <skos:historyNote>Introduced in ISO/TS 14812:2025</skos:historyNote>
    </owl:Class>
    <owl:Class rdf:about="intersection">
        <clause>3.3.6.1</clause>
        <skos:prefLabel xml:lang="en">intersection</skos:prefLabel>
        <skos:definition>space where two or more roads (3.3.5.1) meet or cross</skos:definition>
        <skos:note>Intersections can be associated with zero junctions (3.3.6.2),
            such as a motorway crossing a road without any connecting ramps, or can be associated
            with one or more junctions, such as a diamond interchange (3.3.6.9).</skos:note>
        <skos:note>Complex intersections can be viewed as multiple intersections by
            providing separate designations for distinct road links (3.3.5.6). For example, one
            model could depict a complex intersection as being associated with multiple junctions;
            another model could depict the same physical infrastructure as being multiple
            intersections that are interconnected by different roads, each with its own designator
            (e.g. "ramp from northbound Road A to eastbound Road B").</skos:note>
        <rdfs:subClassOf>
            <owl:Restriction>
                <owl:onProperty rdf:resource="meetingOrCrossing"/>
                <owl:minQualifiedCardinality rdf:datatype="xsd:nonNegativeInteger">2</owl:minQualifiedCardinality>
                <owl:onClass rdf:resource="road"/>
            </owl:Restriction>
        </rdfs:subClassOf>
        <skos:historyNote>Introduced in ISO/TS 14812:2022</skos:historyNote>
    </owl:Class>
    <owl:Class rdf:about="junction">
        <clause>3.3.6.2</clause>
        <skos:prefLabel xml:lang="en">junction</skos:prefLabel>
        <skos:altLabel xml:lang="en">intersection (3.3.6.1) that allows travellers (3.6.1.1) to
            change roads (3.3.5.1)</skos:altLabel>
        <skos:altLabel xml:lang="en"></skos:altLabel>
        <rdfs:subClassOf rdf:resource="intersection"/>
        <rdfs:subClassOf>
            <owl:Restriction>
                <owl:onProperty rdf:resource="aggregates"/>
                <owl:someValuesFrom rdf:resource="ingressLane"/>
            </owl:Restriction>
        </rdfs:subClassOf>
        <rdfs:subClassOf>
            <owl:Restriction>
                <owl:onProperty rdf:resource="aggregates"/>
                <owl:someValuesFrom rdf:resource="egressLane"/>
            </owl:Restriction>
        </rdfs:subClassOf>
        <skos:historyNote>Introduced in ISO/TS 14812:2022</skos:historyNote>
    </owl:Class>
    <owl:Class rdf:about="ingressLane">
        <clause>3.3.6.3</clause>
        <skos:prefLabel xml:lang="en">ingress lane</skos:prefLabel>
        <skos:definition>traffic lane (3.3.1.13) designed for entering a junction (3.3.6.2)</skos:definition>
        <rdfs:subClassOf>
            <owl:Restriction>
                <owl:onProperty rdf:resource="entryFor"/>
                <owl:someValuesFrom rdf:resource="junction"/>
            </owl:Restriction>
        </rdfs:subClassOf>
        <skos:historyNote>Introduced in ISO/TS 14812:2022</skos:historyNote>
    </owl:Class>
    <owl:Class rdf:about="ingressLink">
        <clause>3.3.6.4</clause>
        <skos:prefLabel xml:lang="en">ingress link</skos:prefLabel>
        <skos:definition>all ingress lanes (3.3.6.3) on a road link (3.3.5.6)</skos:definition>
        <rdfs:subClassOf>
            <owl:Restriction>
                <owl:onProperty rdf:resource="aggregates"/>
                <owl:someValuesFrom rdf:resource="ingressLane"/>
            </owl:Restriction>
        </rdfs:subClassOf>
        <skos:historyNote>Introduced in ISO/TS 14812:2022</skos:historyNote>
    </owl:Class>
    <owl:Class rdf:about="egressLane">
        <clause>3.3.6.5</clause>
        <skos:prefLabel xml:lang="en">egress lane</skos:prefLabel>
        <skos:definition>traffic lane (3.3.1.13) designed for exiting a junction (3.3.6.2)</skos:definition>
        <rdfs:subClassOf>
            <owl:Restriction>
                <owl:onProperty rdf:resource="exitFor"/>
                <owl:someValuesFrom rdf:resource="junction"/>
            </owl:Restriction>
        </rdfs:subClassOf>
        <skos:historyNote>Introduced in ISO/TS 14812:2022</skos:historyNote>
    </owl:Class>
    <owl:Class rdf:about="egressLink">
        <clause>3.3.6.6</clause>
        <skos:prefLabel xml:lang="en">egress link</skos:prefLabel>
        <skos:definition>all egress lanes (3.3.6.5) on a road link (3.3.5.6)</skos:definition>
        <rdfs:subClassOf>
            <owl:Restriction>
                <owl:onProperty rdf:resource="aggregates"/>
                <owl:someValuesFrom rdf:resource="egressLane"/>
            </owl:Restriction>
        </rdfs:subClassOf>
        <skos:historyNote>Introduced in ISO/TS 14812:2022</skos:historyNote>
    </owl:Class>
    <owl:Class rdf:about="intersectionManoeuvre">
        <clause>3.3.6.7</clause>
        <skos:prefLabel xml:lang="en">intersection manoeuvre</skos:prefLabel>
        <altPrefLabel xml:lang="en">manoeuvre</altPrefLabel>
        <skos:altLabel xml:lang="en">maneuver</skos:altLabel>
        <skos:definition>&lt;junction&gt; movement from an ingress lane (3.3.6.3) to an egress lane
            (3.3.6.5)</skos:definition>
        <skos:note>The term "maneuver" is the American English spelling.</skos:note>
        <rdfs:subClassOf>
            <owl:Restriction>
                <owl:onProperty rdf:resource="from"/>
                <owl:someValuesFrom rdf:resource="ingressLane"/>
            </owl:Restriction>
        </rdfs:subClassOf>
        <rdfs:subClassOf>
            <owl:Restriction>
                <owl:onProperty rdf:resource="to"/>
                <owl:someValuesFrom rdf:resource="egressLane"/>
            </owl:Restriction>
        </rdfs:subClassOf>
        <skos:historyNote>Introduced in ISO/TS 14812:2022</skos:historyNote>
    </owl:Class>
    <owl:Class rdf:about="junctionAtGrade">
        <clause>3.3.6.8</clause>
        <skos:prefLabel xml:lang="en">junction at grade</skos:prefLabel>
        <altPrefLabel xml:lang="en">at-grade intersection</altPrefLabel>
        <skos:altLabel xml:lang="en">grade junction</skos:altLabel>
        <skos:definition>junction (3.3.6.2) without any grade separated manoeuvres (3.3.6.10)</skos:definition>
        <rdfs:subClassOf rdf:resource="junction"/>
        <skos:historyNote>Introduced in ISO/TS 14812:2022</skos:historyNote>
    </owl:Class>
    <owl:Class rdf:about="interchange">
        <clause>3.3.6.9</clause>
        <skos:prefLabel xml:lang="en">interchange</skos:prefLabel>
        <skos:definition>junction (3.3.6.2) with at least one grade separated manoeuvre (3.3.6.10)</skos:definition>
        <skos:note>The term "interchange" typically refers to the facilities that
            enable all available manoeuvres at the grade separated intersection (3.3.6.1), which
            typically includes multiple junctions.</skos:note>
        <skos:note>The grade separation allows travellers (3.6.1.1) on the link
            (3.3.5.5) to pass unimpeded through the interchange when congestion is not present.</skos:note>
        <rdfs:subClassOf rdf:resource="junction"/>
        <rdfs:subClassOf>
            <owl:Restriction>
                <owl:onProperty rdf:resource="aggregates"/>
                <owl:someValuesFrom rdf:resource="gradeSeparatedManoeuvre"/>
            </owl:Restriction>
        </rdfs:subClassOf>
        <skos:historyNote>Introduced in ISO/TS 14812:2022</skos:historyNote>
    </owl:Class>
    <owl:Class rdf:about="gradeSeparatedManoeuvre">
        <clause>3.3.6.10</clause>
        <skos:prefLabel xml:lang="en">grade separated manoeuvre</skos:prefLabel>
        <skos:definition>manoeuvre (3.3.6.7) that is vertically separated from one or more
            manoeuvres that cross its two-dimensional path</skos:definition>
        <rdfs:subClassOf rdf:resource="intersectionManoeuvre"/>
        <skos:historyNote>Introduced in ISO/TS 14812:2022</skos:historyNote>
    </owl:Class>
    <owl:Class rdf:about="transportFacility">
        <clause>3.3.7.1</clause>
        <skos:prefLabel xml:lang="en">transport facility</skos:prefLabel>
        <skos:definition>physical structure or installation, including related site works, serving
            one or more transport-related purposes</skos:definition>
        <skos:historyNote>Introduced in ISO/TS 14812:2025</skos:historyNote>
    </owl:Class>
    <owl:Class rdf:about="transportInfrastructure">
        <clause>3.3.7.2</clause>
        <skos:prefLabel xml:lang="en">transport infrastructure</skos:prefLabel>
        <skos:definition>system of transport facilities (3.3.7.1) and equipment needed for a
            transport system</skos:definition>
        <skos:note>Transport infrastructure typically includes or shares
            telecommunications infrastructure in the case of ITS.</skos:note>
        <rdfs:subClassOf rdf:resource="system"/>
        <rdfs:subClassOf>
            <owl:Restriction>
                <owl:onProperty rdf:resource="systemOf"/>
                <owl:someValuesFrom rdf:resource="transportFacility"/>
            </owl:Restriction>
        </rdfs:subClassOf>
        <skos:historyNote>Introduced in ISO/TS 14812:2025</skos:historyNote>
    </owl:Class>
    <owl:Class rdf:about="bridge">
        <clause>3.3.7.3</clause>
        <skos:prefLabel xml:lang="en">bridge</skos:prefLabel>
        <skos:definition>transport facility (3.3.7.1) built over a gap to provide a continuous
            travel path</skos:definition>
        <rdfs:subClassOf rdf:resource="transportFacility"/>
        <skos:historyNote>Introduced in ISO/TS 14812:2025</skos:historyNote>
    </owl:Class>
    <owl:Class rdf:about="movableBridge">
        <clause>3.3.7.4</clause>
        <skos:prefLabel xml:lang="en">movable bridge</skos:prefLabel>
        <skos:definition>bridge (3.3.7.3) with a deck that can be moved in a way that disrupts the
            continuous travel path</skos:definition>
        <skos:note>Movable bridges can be used over waterways to allow for the
            passage of tall ships.</skos:note>
        <skos:note>Movable bridges include, but are not limited to, bascule
            bridges, vertical lift bridges, and swing bridges.</skos:note>
        <rdfs:subClassOf rdf:resource="bridge"/>
        <skos:historyNote>Introduced in ISO/TS 14812:2025</skos:historyNote>
    </owl:Class>
    <owl:Class rdf:about="designatedParkingSpace">
        <clause>3.3.8.1</clause>
        <skos:prefLabel xml:lang="en">designated parking space</skos:prefLabel>
        <skos:definition>parking space (3.3.8.3) for a designated purpose Note 1 to entry:  Note 2 to entry: </skos:definition>
        <skos:note>The term "designated parking space" is often specialized to indicate the type of designation
            (e.g., "electric vehicle parking space").</skos:note>
        <skos:note>Designated parking spaces include those that require permits (e.g., reserved for 
            those with disabilities) as well as advisory notices that rely upon voluntary compliance 
            (e.g., reserved for expectant mothers).</skos:note>
        <rdfs:subClassOf rdf:resource="parkingSpace"/>
        <skos:historyNote>Introduced in ISO/TS 14812:2025</skos:historyNote>
    </owl:Class>
    <owl:Class rdf:about="loadingArea">
        <clause>3.3.8.2</clause>
        <skos:prefLabel xml:lang="en">loading area</skos:prefLabel>
        <altPrefLabel xml:lang="en">unloading area</altPrefLabel>
        <skos:definition>area designated for vehicles (3.7.1.1) to load and/or unload goods</skos:definition>
        <skos:note>The area can include the vehicle waiting area and the goods waiting area.</skos:note>
        <rdfs:subClassOf>
            <owl:Restriction>
                <owl:onProperty rdf:resource="forDesignated"/>
                <owl:someValuesFrom rdf:resource="vehicles"/>
            </owl:Restriction>
        </rdfs:subClassOf>
        <skos:historyNote>Introduced in ISO/TS 14812:2025</skos:historyNote>
    </owl:Class>
    <owl:Class rdf:about="parkingSpace">
        <clause>3.3.8.3</clause>
        <skos:prefLabel xml:lang="en">parking space</skos:prefLabel>
        <skos:definition>location for storing a vehicle (3.7.1.1) Note 1 to entry: The vehicle can
            be a motor vehicle, cycle, or any other type of vehicle. Note 2 to entry: A parking
            space is usually designed for a single vehicle. Note 3 to entry: Parking spaces can be,
            but are not necessarily, denoted by painted or other road surface markings.</skos:definition>
        <rdfs:subClassOf>
            <owl:Restriction>
                <owl:onProperty rdf:resource="store"/>
                <owl:maxQualifiedCardinality rdf:datatype="xsd:nonNegativeInteger">1</owl:maxQualifiedCardinality>
                <owl:onClass rdf:resource="vehicle"/>
            </owl:Restriction>
        </rdfs:subClassOf>
        <skos:historyNote>Introduced in ISO/TS 14812:2025</skos:historyNote>
    </owl:Class>
    <owl:Class rdf:about="parkingSpaceForPermitHolders">
        <clause>3.3.8.4</clause>
        <skos:prefLabel xml:lang="en">parking space for permit holders</skos:prefLabel>
        <skos:definition>designated parking space (3.3.8.3) that requires a special permit from an
            appropriate authority</skos:definition>
        <skos:note>The permit can be physically displayed or linked to a database, per authority policies.</skos:note>
        <rdfs:subClassOf rdf:resource="designatedParkingSpace"/>
        <skos:historyNote>Introduced in ISO/TS 14812:2025</skos:historyNote>
    </owl:Class>
    <owl:Class rdf:about="pick-upDrop-offArea">
        <clause>3.3.8.5</clause>
        <skos:prefLabel xml:lang="en">pick-up&#47;drop-off area</skos:prefLabel>
        <altPrefLabel xml:lang="en">PUDO area</altPrefLabel>
        <skos:definition>area intended to allow passengers to board and/or alight from vehicles
            (3.7.1.1)</skos:definition>
        <skos:example>kerbside passenger pick-up area at an airport arrivals zone</skos:example>
        <skos:note>The area can include the vehicle waiting area and the pedestrian waiting area.</skos:note>
        <rdfs:subClassOf>
            <owl:Restriction>
                <owl:onProperty rdf:resource="for"/>
                <owl:someValuesFrom rdf:resource="passenger"/>
            </owl:Restriction>
        </rdfs:subClassOf>
        <rdfs:subClassOf>
            <owl:Restriction>
                <owl:onProperty rdf:resource="toBoardOrAlightFrom"/>
                <owl:someValuesFrom rdf:resource="vehicle"/>
            </owl:Restriction>
        </rdfs:subClassOf>
        <skos:historyNote>Introduced in ISO/TS 14812:2025</skos:historyNote>
    </owl:Class>
    <owl:Class rdf:about="publicTransportVehicleStop">
        <clause>3.3.8.6</clause>
        <skos:prefLabel xml:lang="en">public transport vehicle stop</skos:prefLabel>
        <altPrefLabel xml:lang="en">PTV stop</altPrefLabel>
        <skos:definition>pick-up/drop-off area (3.3.8.5) area for public transport vehicles</skos:definition>
        <skos:note>The term "PTV stop" is often specialized to indicate the type of public
            transport vehicle (e.g., "bus stop", "tram stop").</skos:note>
        <rdfs:subClassOf rdf:resource="pick-upDrop-offArea"/>
        <rdfs:subClassOf>
            <owl:Restriction>
                <owl:onProperty rdf:resource="for"/>
                <owl:someValuesFrom rdf:resource="publicTransportVehicle"/>
            </owl:Restriction>
        </rdfs:subClassOf>
        <skos:historyNote>Introduced in ISO/TS 14812:2025</skos:historyNote>
    </owl:Class>
    <owl:Class rdf:about="roadEquipment">
        <clause>3.3.9.1</clause>
        <skos:prefLabel xml:lang="en">road equipment</skos:prefLabel>
        <skos:altLabel xml:lang="en">road furniture</skos:altLabel>
        <skos:definition>component of transport infrastructure (3.3.7.2) along the roadway intended
            to contribute to the safety, operations, management, awareness, and comfort of movements
            of the road users (3.6.1.2)</skos:definition>
        <skos:example>sign, traffic signal, safety rail, gantry, bus stop structure,
            highway safety lighting</skos:example>
        <skos:note>Road equipment can be next to, over, on and/or in the roadway.</skos:note>
        <skos:note>ITS roadside equipment is a type of roadside equipment.</skos:note>
        <skos:note>Road equipment is sometimes referred to as "roadside equipment".</skos:note>
        <skos:historyNote>Introduced in ISO/TS 14812:2022</skos:historyNote>
    </owl:Class>
    <owl:Class rdf:about="trafficControlDevice">
        <clause>3.3.9.2</clause>
        <skos:prefLabel xml:lang="en">traffic control device</skos:prefLabel>
        <skos:definition>road equipment (3.3.9.1) used to visually, audibly, or tangibly convey
            regulatory, advisory, or guidance information to road users (3.6.1.2)</skos:definition>
        <rdfs:subClassOf rdf:resource="roadEquipment"/>
        <skos:historyNote>Introduced in ISO/TS 14812:2022</skos:historyNote>
    </owl:Class>
    <owl:Class rdf:about="location">
        <clause>3.4.1.1</clause>
        <skos:prefLabel xml:lang="en">location</skos:prefLabel>
        <skos:definition>particular place or position</skos:definition>
        <skos:note>The term "location" by itself is a broad term that can be used
            to reference spatial, computer memory, imaginary and other locations.</skos:note>
        <skos:historyNote>Introduced in ISO/TS 14812:2022</skos:historyNote>
    </owl:Class>
    <owl:Class rdf:about="spatialLocation">
        <clause>3.4.1.2</clause>
        <skos:prefLabel xml:lang="en">spatial location</skos:prefLabel>
        <altPrefLabel xml:lang="en">ITS spatial location</altPrefLabel>
        <skos:definition>location (3.4.1.1) within three-dimensional space</skos:definition>
        <skos:note>The "location" could be a point (consuming no space) or could
            consume space in one, two, or three dimensions. In any case, the location is identified
            within a larger space.</skos:note>
        <skos:note>Within ITS, locations are typically locations on or near the
            surface of the earth.</skos:note>
        <rdfs:subClassOf rdf:resource="location"/>
        <skos:historyNote>Introduced in ISO/TS 14812:2022</skos:historyNote>
    </owl:Class>
    <owl:Class rdf:about="pointLocation">
        <clause>3.4.1.3</clause>
        <skos:prefLabel xml:lang="en">point location</skos:prefLabel>
        <skos:definition>spatial location (3.4.1.2) with no length in any of the spatial dimensions</skos:definition>
        <rdfs:subClassOf rdf:resource="spatialLocation"/>
        <skos:historyNote>Introduced in ISO/TS 14812:2022</skos:historyNote>
    </owl:Class>
    <owl:Class rdf:about="geographicPointLocation">
        <clause>3.4.1.4</clause>
        <skos:prefLabel xml:lang="en">geographic point location</skos:prefLabel>
        <skos:altLabel xml:lang="en">geolocation</skos:altLabel>
        <skos:definition>well defined geographic place described by one coordinate tuple</skos:definition>
        <skos:note>The "geolocation" term is a short version of the term used
            within some ITS communities.</skos:note>
        <dcterms:source>ISO 19145:2013, 4.1.11, modified - Note 1 to entry added.</dcterms:source>
        <rdfs:subClassOf rdf:resource="pointLocation"/>
        <skos:historyNote>Introduced in ISO/TS 14812:2022</skos:historyNote>
    </owl:Class>
    <owl:Class rdf:about="linearLocation">
        <clause>3.4.1.5</clause>
        <skos:prefLabel xml:lang="en">linear location</skos:prefLabel>
        <altPrefLabel xml:lang="en">ITS linear location</altPrefLabel>
        <skos:definition>spatial location (3.4.1.2) that extends between two point locations
            (3.4.1.3) along a defined path</skos:definition>
        <skos:note>The path can exhibit 3-dimensional characteristics.</skos:note>
        <rdfs:subClassOf rdf:resource="spatialLocation"/>
        <skos:historyNote>Introduced in ISO/TS 14812:2022</skos:historyNote>
    </owl:Class>
    <owl:Class rdf:about="areaLocation">
        <clause>3.4.1.6</clause>
        <skos:prefLabel xml:lang="en">area location</skos:prefLabel>
        <altPrefLabel xml:lang="en">ITS area location</altPrefLabel>
        <skos:definition>spatial location (3.4.1.2) enclosed within a two-dimensional boundary or
            boundaries across a defined surface</skos:definition>
        <skos:example>The British Isles.</skos:example>
        <skos:note>The boundary can consist of a single curvilinear line (e.g. a
            circle) or multiple curvilinear lines (e.g. the boundaries of city limits) and can
            consist of multiple enclosed areas.</skos:note>
        <rdfs:subClassOf rdf:resource="spatialLocation"/>
        <skos:historyNote>Introduced in ISO/TS 14812:2022</skos:historyNote>
    </owl:Class>
    <owl:Class rdf:about="geographicFeature">
        <clause>3.4.1.7</clause>
        <skos:prefLabel xml:lang="en">geographic feature</skos:prefLabel>
        <skos:definition>abstraction of real-world phenomena</skos:definition>
        <skos:note>Geographic features can be defined for any geographic entity
            that can be defined with geospatial boundaries, such as landmarks, buildings, transport
            infrastructure (e.g., road, pathway, railway, bridge structures, intersections, traffic
            signal cabinet, traffic signal pole, waterway), jurisdictional areas (e.g., country,
            city), etc.</skos:note>
        <dcterms:source>ISO 19101-1:2014, 4.1.11, "geographic" has been added to the term
            to clarify context; note 1 to entry has been replaced.</dcterms:source>
        <skos:historyNote>Introduced in ISO/TS 14812:2025</skos:historyNote>
    </owl:Class>
    <owl:Class rdf:about="pointDestination">
        <clause>3.4.1.8</clause>
        <skos:prefLabel xml:lang="en">point destination</skos:prefLabel>
        <skos:definition>point location, which is the destination of a defined route or itinerary</skos:definition>
        <rdfs:subClassOf rdf:resource="pointLocation"/>
        <skos:historyNote>Introduced in ISO/TS 14812:2025</skos:historyNote>
    </owl:Class>
    <owl:Class rdf:about="areaDestination">
        <clause>3.4.1.9</clause>
        <skos:prefLabel xml:lang="en">area destination</skos:prefLabel>
        <skos:definition>area location, which is the destination of a defined route or itinerary</skos:definition>
        <rdfs:subClassOf rdf:resource="areaLocation"/>
        <skos:historyNote>Introduced in ISO/TS 14812:2025</skos:historyNote>
    </owl:Class>
    <owl:Class rdf:about="coordinateTuple">
        <clause>3.4.1.10</clause>
        <skos:prefLabel xml:lang="en">coordinate tuple</skos:prefLabel>
        <skos:definition>ordered list of numbers that jointly designate the position of a point</skos:definition>
        <skos:note>The number of values in a coordinate tuple is immutable.</skos:note>
        <skos:note>This definition was derived by consolidating the definitions of "coordinate tuple",
            "coordinate", and "tuple" from ISO 19136:2020.</skos:note>
        <rdfs:subClassOf>
            <owl:Restriction>
                <owl:onProperty rdf:resource="designates"/>
                <owl:someValuesFrom rdf:resource="pointLocation"/>
            </owl:Restriction>
        </rdfs:subClassOf>
        <skos:historyNote>Introduced in ISO/TS 14812:2025</skos:historyNote>
    </owl:Class>
    <owl:Class rdf:about="pointCoordinates">
        <clause>3.4.1.11</clause>
        <skos:prefLabel xml:lang="en">point coordinates</skos:prefLabel>
        <skos:definition>coordinate tuple defining the geodetic position of a single point location
            (3.4.1.3) using a known geodetic reference system</skos:definition>
        <rdfs:subClassOf rdf:resource="coordinateTuple"/>
        <skos:historyNote>Introduced in ISO/TS 14812:2025</skos:historyNote>
    </owl:Class>
    <owl:Class rdf:about="locationReferencing">
        <clause>3.4.2.1</clause>
        <skos:prefLabel xml:lang="en">location referencing</skos:prefLabel>
        <altPrefLabel xml:lang="en">ITS location referencing</altPrefLabel>
        <skos:definition>process used to develop a spatial reference (3.4.2.2)</skos:definition>
        <rdfs:subClassOf>
            <owl:Restriction>
                <owl:onProperty rdf:resource="processToDevelop"/>
                <owl:someValuesFrom rdf:resource="spatialReference"/>
            </owl:Restriction>
        </rdfs:subClassOf>
        <skos:historyNote>Introduced in ISO/TS 14812:2022</skos:historyNote>
    </owl:Class>
    <owl:Class rdf:about="spatialReference">
        <clause>3.4.2.2</clause>
        <skos:prefLabel xml:lang="en">spatial reference</skos:prefLabel>
        <altPrefLabel xml:lang="en">ITS spatial reference</altPrefLabel>
        <skos:altLabel xml:lang="en">location reference</skos:altLabel>
        <skos:definition>description of a spatial location (3.4.1.2) in the real world according to
            a defined reference system</skos:definition>
        <skos:example>Coordinate tuple: 51.476852, -0.000500.</skos:example>
        <skos:note>It is not necessary for the rules be formal coordinates but they
            could be descriptive.</skos:note>
        <skos:note>The term "location reference" has been used within ITS, but the
            term "spatial reference" is preferred to better align with the activities of ISO/TC 211.</skos:note>
        <rdfs:subClassOf>
            <owl:Restriction>
                <owl:onProperty rdf:resource="specificationOf"/>
                <owl:someValuesFrom rdf:resource="spatialLocation"/>
            </owl:Restriction>
        </rdfs:subClassOf>
        <skos:historyNote>Introduced in ISO/TS 14812:2022</skos:historyNote>
    </owl:Class>
    <owl:Class rdf:about="dynamicSpatialReference">
        <clause>3.4.2.3</clause>
        <skos:prefLabel xml:lang="en">dynamic spatial reference</skos:prefLabel>
        <skos:altLabel xml:lang="en">dynamic location reference</skos:altLabel>
        <skos:definition>spatial reference (3.4.2.2) generated on-the-fly based on geographic
            properties in a digital map database</skos:definition>
        <rdfs:subClassOf rdf:resource="spatialReference"/>
        <skos:historyNote>Introduced in ISO/TS 14812:2022</skos:historyNote>
    </owl:Class>
    <owl:Class rdf:about="pre-codedSpatialReference">
        <clause>3.4.2.4</clause>
        <skos:prefLabel xml:lang="en">pre-coded spatial reference</skos:prefLabel>
        <skos:altLabel xml:lang="en">pre-coded location reference</skos:altLabel>
        <skos:definition>spatial reference (3.4.2.2) using a unique identifier that is agreed upon
            in both the sender and receiver system (3.1.2.1) to select a location (3.4.1.1) from a
            set of pre-coded locations</skos:definition>
        <rdfs:subClassOf rdf:resource="spatialReference"/>
        <skos:historyNote>Introduced in ISO/TS 14812:2022</skos:historyNote>
    </owl:Class>
    <owl:Class rdf:about="linkLocation">
        <clause>3.4.2.5</clause>
        <skos:prefLabel xml:lang="en">link location</skos:prefLabel>
        <skos:definition>pre-coded spatial reference (3.4.2.4) defined within the road network
            (3.3.5.2) database</skos:definition>
        <rdfs:subClassOf rdf:resource="pre-codedSpatialReference"/>
        <skos:historyNote>Introduced in ISO/TS 14812:2022</skos:historyNote>
    </owl:Class>
    <owl:Class rdf:about="geographicIdentifier">
        <clause>3.4.2.6</clause>
        <skos:prefLabel xml:lang="en">geographic identifier</skos:prefLabel>
        <skos:hiddenLabel xml:lang="en">location code</skos:hiddenLabel>
        <skos:definition>spatial reference (3.4.2.2) in the form of a label or code that identifies
            a location (3.4.1.1)</skos:definition>
        <skos:example>"Spain" is an example of a label (country name); "SW1P 3AD" is an
            example of a code (postcode).</skos:example>
        <skos:note>The term "location code" has been used previously in ISO/TC 204
            documents, but "geographic identifier" is preferred to better align with the activities
            of ISO/TC 211.</skos:note>
        <dcterms:source>ISO 19112:2019, 3.1.2, modified - Note 1 to entry and deprecated
            term added.</dcterms:source>
        <rdfs:subClassOf>
            <owl:Restriction>
                <owl:onProperty rdf:resource="referenceUsedBy"/>
                <owl:someValuesFrom rdf:resource="spatialReference"/>
            </owl:Restriction>
        </rdfs:subClassOf>
        <skos:historyNote>Introduced in ISO/TS 14812:2022</skos:historyNote>
    </owl:Class>
    <owl:Class rdf:about="gazetteer">
        <clause>3.4.2.7</clause>
        <skos:prefLabel xml:lang="en">gazetteer</skos:prefLabel>
        <skos:altLabel xml:lang="en">location table</skos:altLabel>
        <skos:definition>register of spatial references (3.4.2.2) of one or more location (3.4.1.1)
            sub-types containing some information regarding position</skos:definition>
        <skos:note>The positional information need not be coordinates but could be
            descriptive.</skos:note>
        <dcterms:source>ISO 19112:2019, 3.1.1, modified - "register of location
            instances..." changed to "register of spatial references..." in order to fit the
            relevant concept model.</dcterms:source>
        <rdfs:subClassOf>
            <owl:Restriction>
                <owl:onProperty rdf:resource="aggregates"/>
                <owl:someValuesFrom rdf:resource="spatialReference"/>
            </owl:Restriction>
        </rdfs:subClassOf>
        <skos:historyNote>Introduced in ISO/TS 14812:2022</skos:historyNote>
    </owl:Class>
    <owl:Class rdf:about="networkLocation">
        <clause>3.4.2.8</clause>
        <skos:prefLabel xml:lang="en">network location</skos:prefLabel>
        <skos:definition>point or linear location on a network</skos:definition>
        <skos:historyNote>Introduced in ISO/TS 14812:2022</skos:historyNote>
    </owl:Class>
    <owl:Class rdf:about="geographicDescriptor">
        <clause>3.4.2.9</clause>
        <skos:prefLabel xml:lang="en">geographic descriptor</skos:prefLabel>
        <skos:definition>descriptor that identifies a geographic characteristic to help identify a
            specific location</skos:definition>
        <rdfs:subClassOf>
            <owl:Restriction>
                <owl:onProperty rdf:resource="helpsIdentify"/>
                <owl:someValuesFrom rdf:resource="spatialLocation"/>
            </owl:Restriction>
        </rdfs:subClassOf>
        <skos:historyNote>Introduced in ISO/TS 14812:2022</skos:historyNote>
    </owl:Class>
    <owl:Class rdf:about="infrastructureDescriptor">
        <clause>3.4.2.10</clause>
        <skos:prefLabel xml:lang="en">infrastructure descriptor</skos:prefLabel>
        <skos:definition>descriptor that identifies infrastructure to help identify a specific
            location</skos:definition>
        <rdfs:subClassOf>
            <owl:Restriction>
                <owl:onProperty rdf:resource="helpsIdentify"/>
                <owl:someValuesFrom rdf:resource="transportFacility"/>
            </owl:Restriction>
        </rdfs:subClassOf>
        <skos:historyNote>Introduced in ISO/TS 14812:2022</skos:historyNote>
    </owl:Class>
    <owl:Class rdf:about="campus">
        <clause>3.4.3.1</clause>
        <skos:prefLabel xml:lang="en">campus</skos:prefLabel>
        <skos:definition>jurisdictional area (3.4.3.4) with a jurisdictional entity (3.4.3.6) who is
            the owner of the area but excluding transport facilities managed by the local government</skos:definition>
        <skos:example>A point of interest (e.g., airport, university, business park,
            industrial area, shopping centre) that manages its own transport infrastructure
            separately from that managed by the local government. In this case, the point of
            interest and its own transport system are a part of the campus.</skos:example>
        <skos:example>A point of interest (e.g., airport, university, business park,
            industrial area, shopping centre) that includes transport infrastructure that is managed
            by the local government. In this case, the government-managed transport infrastructure
            is a governmental area while the campus is represented by the remainder of the area.</skos:example>
        <skos:note>A campus can be privately or publicly owned.</skos:note>
        <rdfs:subClassOf rdf:resource="jurisdictionalArea"/>
        <skos:historyNote>Introduced in ISO/TS 14812:2025</skos:historyNote>
    </owl:Class>
    <owl:Class rdf:about="governmentalArea">
        <clause>3.4.3.2</clause>
        <skos:prefLabel xml:lang="en">governmental area</skos:prefLabel>
        <skos:definition>transport-related, jurisdictional area (3.4.3.4) whose only jurisdictional
            entities (3.4.3.6) are governmental entities</skos:definition>
        <skos:example>A subway station owned by a governmental entity is a governmental
            area.</skos:example>
        <skos:note>The boundaries of a jurisdictional area can include or exclude
            geofenced areas to indicate which jurisdictional entities have authority over transport
            facilities (3.4.3) as needed.</skos:note>
        <rdfs:subClassOf rdf:resource="jurisdictionalArea"/>
        <skos:historyNote>Introduced in ISO/TS 14812:2025</skos:historyNote>
    </owl:Class>
    <owl:Class rdf:about="isoNamedArea">
        <clause>3.4.3.3</clause>
        <skos:prefLabel xml:lang="en">ISO named area</skos:prefLabel>
        <altPrefLabel xml:lang="en">area identified using ISO 3166-2 identifiers</altPrefLabel>
        <skos:definition>Note 1 to entry: ISO 3166-2 includes codes for major subdivisions of
            countries and states.</skos:definition>
        <skos:historyNote>Introduced in ISO/TS 14812:2025</skos:historyNote>
    </owl:Class>
    <owl:Class rdf:about="jurisdiction">
        <clause>3.4.3.4</clause>
        <skos:prefLabel xml:lang="en">jurisdiction</skos:prefLabel>
        <skos:definition>legal power to issue rules of behaviour for a defined area</skos:definition>
        <skos:historyNote>Introduced in ISO/TS 14812:2025</skos:historyNote>
    </owl:Class>
    <owl:Class rdf:about="jurisdictionalArea">
        <clause>3.4.3.5</clause>
        <skos:prefLabel xml:lang="en">jurisdictional area</skos:prefLabel>
        <skos:definition>territory for which a jurisdictional entity (3.4.3.6) has the power to
            define rules of behaviour</skos:definition>
        <skos:note>A jurisdictional area might include non-contiguous locations.</skos:note>
        <rdfs:subClassOf>
            <owl:Restriction>
                <owl:onProperty rdf:resource="rulesDefinedBy"/>
                <owl:someValuesFrom rdf:resource="jurisdictionalEntity"/>
            </owl:Restriction>
        </rdfs:subClassOf>
        <skos:historyNote>Introduced in ISO/TS 14812:2025</skos:historyNote>
    </owl:Class>
    <owl:Class rdf:about="jurisdictionalBoundary">
        <clause>3.4.3.6</clause>
        <skos:prefLabel xml:lang="en">jurisdictional boundary</skos:prefLabel>
        <skos:definition>territorial limit associated with a jurisdictional area (3.4.3.5)</skos:definition>
        <skos:note>A geofence can be used to electronically represent a
            jurisdictional boundary.</skos:note>
        <rdfs:subClassOf>
            <owl:Restriction>
                <owl:onProperty rdf:resource="limitOf"/>
                <owl:someValuesFrom rdf:resource="jurisdictionalArea"/>
            </owl:Restriction>
        </rdfs:subClassOf>
        <skos:historyNote>Introduced in ISO/TS 14812:2025</skos:historyNote>
    </owl:Class>
    <owl:Class rdf:about="jurisdictionalEntity">
        <clause>3.4.3.7</clause>
        <skos:prefLabel xml:lang="en">jurisdictional entity</skos:prefLabel>
        <skos:definition>person (3.1.1.6) or organization who has jurisdiction (3.4.3.3)</skos:definition>
        <skos:example>A city government</skos:example>
        <skos:note>In the case of a geopolitical jurisdiction, the jurisdictional
            entity is typically the recognized government for the territory; in the case of a
            campus, the jurisdictional entity is typically the landowner. </skos:note>
        <skos:note>A jurisdictional entity assigns its authority to one or more
            rule-makers, which may be itself (e.g., the individual owner or a campus) or other
            divisions of the entity (e.g., police department, traffic department).</skos:note>
        <rdfs:subClassOf>
            <owl:Restriction>
                <owl:onProperty rdf:resource="has"/>
                <owl:someValuesFrom rdf:resource="jurisdiction"/>
            </owl:Restriction>
        </rdfs:subClassOf>
        <skos:historyNote>Introduced in ISO/TS 14812:2025</skos:historyNote>
    </owl:Class>
    <owl:Class rdf:about="service">
        <clause>3.5.1.1</clause>
        <skos:prefLabel xml:lang="en">service</skos:prefLabel>
        <skos:definition>provision of one or more capabilities, functionalities or facilities to
            fulfil or enable the fulfilment of a user need (3.5.1.4)</skos:definition>
        <rdfs:subClassOf>
            <owl:Restriction>
                <owl:onProperty rdf:resource="fulfils"/>
                <owl:someValuesFrom rdf:resource="userNeed"/>
            </owl:Restriction>
        </rdfs:subClassOf>
        <rdfs:subClassOf>
            <owl:Restriction>
                <owl:onProperty rdf:resource="for"/>
                <owl:someValuesFrom rdf:resource="user"/>
            </owl:Restriction>
        </rdfs:subClassOf>
        <skos:historyNote>Introduced in ISO/TS 14812:2022</skos:historyNote>
    </owl:Class>
    <owl:Class rdf:about="serviceProvider">
        <clause>3.5.1.2</clause>
        <skos:prefLabel xml:lang="en">service provider</skos:prefLabel>
        <skos:definition>entity (3.1.1.1) that delivers one or more services (3.5.1.1)</skos:definition>
        <rdfs:subClassOf rdf:resource="entity"/>
        <rdfs:subClassOf>
            <owl:Restriction>
                <owl:onProperty rdf:resource="delivers"/>
                <owl:someValuesFrom rdf:resource="service"/>
            </owl:Restriction>
        </rdfs:subClassOf>
        <skos:historyNote>Introduced in ISO/TS 14812:2022</skos:historyNote>
    </owl:Class>
    <owl:Class rdf:about="user">
        <clause>3.5.1.3</clause>
        <skos:prefLabel xml:lang="en">user</skos:prefLabel>
        <altPrefLabel xml:lang="en">consumer</altPrefLabel>
        <skos:definition>entity (3.1.1.1) for whom the system (3.1.2.1) of interest is designed</skos:definition>
        <skos:note>The term "consumer" can be used when fulfilling the need results
            in the consumption of a resource (3.1.6.2).</skos:note>
        <rdfs:subClassOf rdf:resource="entity"/>
        <skos:historyNote>Introduced in ISO/TS 14812:2022</skos:historyNote>
    </owl:Class>
    <owl:Class rdf:about="userNeed">
        <clause>3.5.1.4</clause>
        <skos:prefLabel xml:lang="en">user need</skos:prefLabel>
        <altPrefLabel xml:lang="en">need</altPrefLabel>
        <skos:definition>desired results of a user (3.5.1.3) within a specified context of use</skos:definition>
        <rdfs:subClassOf>
            <owl:Restriction>
                <owl:onProperty rdf:resource="desiredResultsOf"/>
                <owl:someValuesFrom rdf:resource="user"/>
            </owl:Restriction>
        </rdfs:subClassOf>
        <skos:historyNote>Introduced in ISO/TS 14812:2022</skos:historyNote>
    </owl:Class>
    <owl:Class rdf:about="transportService">
        <clause>3.5.2.1</clause>
        <skos:prefLabel xml:lang="en">transport service</skos:prefLabel>
        <altPrefLabel xml:lang="en">service</altPrefLabel>
        <skos:definition>service (3.5.1.1) that transports one or more material entities (3.1.1.3)
            from one location (3.4.1.1) to another</skos:definition>
        <skos:note>The material entities transported can be people and/or goods.</skos:note>
        <rdfs:subClassOf rdf:resource="service"/>
        <rdfs:subClassOf>
            <owl:Restriction>
                <owl:onProperty rdf:resource="fulfils"/>
                <owl:someValuesFrom rdf:resource="transportUserNeed"/>
            </owl:Restriction>
        </rdfs:subClassOf>
        <rdfs:subClassOf>
            <owl:Restriction>
                <owl:onProperty rdf:resource="for"/>
                <owl:someValuesFrom rdf:resource="transportUser"/>
            </owl:Restriction>
        </rdfs:subClassOf>
        <rdfs:subClassOf>
            <owl:Restriction>
                <owl:onProperty rdf:resource="transports"/>
                <owl:someValuesFrom rdf:resource="materialEntity"/>
            </owl:Restriction>
        </rdfs:subClassOf>
        <skos:historyNote>Introduced in ISO/TS 14812:2022</skos:historyNote>
    </owl:Class>
    <owl:Class rdf:about="transportProvider">
        <clause>3.5.2.2</clause>
        <skos:prefLabel xml:lang="en">transport provider</skos:prefLabel>
        <altPrefLabel xml:lang="en">service provider</altPrefLabel>
        <altPrefLabel xml:lang="en">provider</altPrefLabel>
        <skos:definition>entity (3.1.1.1) that delivers one or more transport services (3.5.2.1)</skos:definition>
        <rdfs:subClassOf rdf:resource="serviceProvider"/>
        <rdfs:subClassOf>
            <owl:Restriction>
                <owl:onProperty rdf:resource="delivers"/>
                <owl:someValuesFrom rdf:resource="transportService"/>
            </owl:Restriction>
        </rdfs:subClassOf>
        <skos:historyNote>Introduced in ISO/TS 14812:2022</skos:historyNote>
    </owl:Class>
    <owl:Class rdf:about="transportUser">
        <clause>3.5.2.3</clause>
        <skos:prefLabel xml:lang="en">transport user</skos:prefLabel>
        <altPrefLabel xml:lang="en">user</altPrefLabel>
        <altPrefLabel xml:lang="en">consumer</altPrefLabel>
        <skos:definition>entity (3.1.1.1) that has a desire to transport a material entity (3.1.1.3)</skos:definition>
        <rdfs:subClassOf rdf:resource="user"/>
        <skos:historyNote>Introduced in ISO/TS 14812:2022</skos:historyNote>
    </owl:Class>
    <owl:Class rdf:about="transportUserNeed">
        <clause>3.5.2.4</clause>
        <skos:prefLabel xml:lang="en">transport user need</skos:prefLabel>
        <altPrefLabel xml:lang="en">user need</altPrefLabel>
        <altPrefLabel xml:lang="en">need</altPrefLabel>
        <skos:definition>user need (3.5.1.4) to transport one or more material entities (3.1.1.3) to
            a different location (3.4.1.1)</skos:definition>
        <rdfs:subClassOf rdf:resource="userNeed"/>
        <rdfs:subClassOf>
            <owl:Restriction>
                <owl:onProperty rdf:resource="desiredResultsOf"/>
                <owl:someValuesFrom rdf:resource="transportUser"/>
            </owl:Restriction>
        </rdfs:subClassOf>
        <rdfs:subClassOf>
            <owl:Restriction>
                <owl:onProperty rdf:resource="desireToTransport"/>
                <owl:someValuesFrom rdf:resource="materialEntity"/>
            </owl:Restriction>
        </rdfs:subClassOf>
        <skos:historyNote>Introduced in ISO/TS 14812:2022</skos:historyNote>
    </owl:Class>
    <owl:Class rdf:about="itsService">
        <clause>3.5.3.1</clause>
        <skos:prefLabel xml:lang="en">ITS service</skos:prefLabel>
        <altPrefLabel xml:lang="en">service</altPrefLabel>
        <skos:definition>provision of functionality that fulfils one or more ITS user needs
            (3.5.3.4)</skos:definition>
        <rdfs:subClassOf rdf:resource="service"/>
        <rdfs:subClassOf>
            <owl:Restriction>
                <owl:onProperty rdf:resource="fulfils"/>
                <owl:someValuesFrom rdf:resource="itsUserNeed"/>
            </owl:Restriction>
        </rdfs:subClassOf>
        <rdfs:subClassOf>
            <owl:Restriction>
                <owl:onProperty rdf:resource="for"/>
                <owl:someValuesFrom rdf:resource="itsUser"/>
            </owl:Restriction>
        </rdfs:subClassOf>
        <skos:historyNote>Introduced in ISO/TS 14812:2022</skos:historyNote>
    </owl:Class>
    <owl:Class rdf:about="itsServiceProvider">
        <clause>3.5.3.2</clause>
        <skos:prefLabel xml:lang="en">ITS service provider</skos:prefLabel>
        <altPrefLabel xml:lang="en">service provider</altPrefLabel>
        <skos:definition>entity (3.1.1.1) that delivers one or more ITS services (3.5.3.1)</skos:definition>
        <skos:note>Cooperative ITS (3.1.2.5) services often require multiple
            entities cooperatively working together to provide a unified service (3.5.1.1) where the
            individual entities are simultaneously ITS service providers and ITS users.</skos:note>
        <rdfs:subClassOf rdf:resource="serviceProvider"/>
        <rdfs:subClassOf>
            <owl:Restriction>
                <owl:onProperty rdf:resource="delivers"/>
                <owl:someValuesFrom rdf:resource="itsService"/>
            </owl:Restriction>
        </rdfs:subClassOf>
        <skos:historyNote>Introduced in ISO/TS 14812:2022</skos:historyNote>
    </owl:Class>
    <owl:Class rdf:about="itsUser">
        <clause>3.5.3.3</clause>
        <skos:prefLabel xml:lang="en">ITS user</skos:prefLabel>
        <altPrefLabel xml:lang="en">user</altPrefLabel>
        <skos:definition>entity (3.1.1.1) that uses information, communication, and transducer
            technologies to achieve benefits when using a surface transport system (3.1.2.3)</skos:definition>
        <rdfs:subClassOf rdf:resource="user"/>
        <rdfs:subClassOf>
            <owl:Restriction>
                <owl:onProperty rdf:resource="uses"/>
                <owl:someValuesFrom rdf:resource="surfaceTransportSystem"/>
            </owl:Restriction>
        </rdfs:subClassOf>
        <skos:historyNote>Introduced in ISO/TS 14812:2022</skos:historyNote>
    </owl:Class>
    <owl:Class rdf:about="itsUserNeed">
        <clause>3.5.3.4</clause>
        <skos:prefLabel xml:lang="en">ITS user need</skos:prefLabel>
        <altPrefLabel xml:lang="en">user need</altPrefLabel>
        <skos:definition>user need (3.5.1.4) for a surface transport system (3.1.2.3) benefit that
            can be met with the use of information, communication, and transducer technologies</skos:definition>
        <skos:example>Increasing safety, sustainability, efficiency and/or comfort.</skos:example>
        <rdfs:subClassOf rdf:resource="userNeed"/>
        <rdfs:subClassOf>
            <owl:Restriction>
                <owl:onProperty rdf:resource="desiredResultsOf"/>
                <owl:someValuesFrom rdf:resource="itsUser"/>
            </owl:Restriction>
        </rdfs:subClassOf>
        <skos:historyNote>Introduced in ISO/TS 14812:2022</skos:historyNote>
    </owl:Class>
    <owl:Class rdf:about="its-suService">
        <clause>3.5.4.1</clause>
        <skos:prefLabel xml:lang="en">ITS-SU service</skos:prefLabel>
        <skos:definition>provision of functionality to fulfil an ITS-SU user need (3.5.4.4)</skos:definition>
        <skos:note>An ITS-SU service refers to the services provided by
            realizations of ITS-S application processes while an ITS-S service refers to the
            communication services that these processes use to communicate to other nodes.</skos:note>
        <rdfs:subClassOf rdf:resource="service"/>
        <rdfs:subClassOf>
            <owl:Restriction>
                <owl:onProperty rdf:resource="fulfils"/>
                <owl:someValuesFrom rdf:resource="its-suUserNeed"/>
            </owl:Restriction>
        </rdfs:subClassOf>
        <rdfs:subClassOf>
            <owl:Restriction>
                <owl:onProperty rdf:resource="for"/>
                <owl:someValuesFrom rdf:resource="its-suUser"/>
            </owl:Restriction>
        </rdfs:subClassOf>
        <skos:historyNote>Introduced in ISO/TS 14812:2022</skos:historyNote>
    </owl:Class>
    <owl:Class rdf:about="its-suServiceProvider">
        <clause>3.5.4.2</clause>
        <skos:prefLabel xml:lang="en">ITS-SU service provider</skos:prefLabel>
        <skos:definition>ITS-SU (3.2.7.4) that delivers one or more ITS-SU services (3.5.4.1)</skos:definition>
        <rdfs:subClassOf rdf:resource="serviceProvider"/>
        <rdfs:subClassOf>
            <owl:Restriction>
                <owl:onProperty rdf:resource="delivers"/>
                <owl:someValuesFrom rdf:resource="its-suService"/>
            </owl:Restriction>
        </rdfs:subClassOf>
        <rdfs:subClassOf>
            <owl:Restriction>
                <owl:onProperty rdf:resource="isA"/>
                <owl:someValuesFrom rdf:resource="its-sUnit"/>
            </owl:Restriction>
        </rdfs:subClassOf>
        <skos:historyNote>Introduced in ISO/TS 14812:2022</skos:historyNote>
    </owl:Class>
    <owl:Class rdf:about="its-suUser">
        <clause>3.5.4.3</clause>
        <skos:prefLabel xml:lang="en">ITS-SU user</skos:prefLabel>
        <skos:definition>entity (3.1.1.1) that has a need to perform processing within a bounded,
            secure, managed domain (3.2.7.1)</skos:definition>
        <rdfs:subClassOf rdf:resource="user"/>
        <rdfs:subClassOf>
            <owl:Restriction>
                <owl:onProperty rdf:resource="has"/>
                <owl:someValuesFrom rdf:resource="its-suUserNeed"/>
            </owl:Restriction>
        </rdfs:subClassOf>
        <skos:historyNote>Introduced in ISO/TS 14812:2022</skos:historyNote>
    </owl:Class>
    <owl:Class rdf:about="its-suUserNeed">
        <clause>3.5.4.4</clause>
        <skos:prefLabel xml:lang="en">ITS-SU user need</skos:prefLabel>
        <skos:definition>user need (3.5.1.4) for processing within a bounded, secure, managed domain
            (3.2.7.1)</skos:definition>
        <rdfs:subClassOf rdf:resource="userNeed"/>
        <rdfs:subClassOf>
            <owl:Restriction>
                <owl:onProperty rdf:resource="requiresProcessingWithin"/>
                <owl:someValuesFrom rdf:resource="boundedSecureManagedDomain"/>
            </owl:Restriction>
        </rdfs:subClassOf>
        <skos:historyNote>Introduced in ISO/TS 14812:2022</skos:historyNote>
    </owl:Class>
    <owl:Class rdf:about="its-sService">
        <clause>3.5.4.5</clause>
        <skos:prefLabel xml:lang="en">ITS-S service</skos:prefLabel>
        <skos:definition>communication functionality of an ITS station (3.2.7.3) that provides the
            capability to connect to other nodes</skos:definition>
        <skos:note>The definition of ITS-S service predates the adoption of the
            concept model used for the other service terms in this standard. It is an outlier in
            that it describes a portion of the functionality contained within the ITS station
            reference architecture (i.e., the communication functionality) rather than the end
            functionality of the conceptual ITS station.</skos:note>
        <skos:note>[ISO 21217:2020, 3.51; note added]</skos:note>
        <rdfs:subClassOf rdf:resource="service"/>
        <skos:historyNote>Introduced in ISO/TS 14812:2022</skos:historyNote>
    </owl:Class>
    <owl:Class rdf:about="mobilityApp">
        <clause>3.5.5.1</clause>
        <skos:prefLabel xml:lang="en">mobility app</skos:prefLabel>
        <skos:definition>ITS-S application implementation (3.2.9.4) designed to assist an individual
            transport consumer in understanding transport-related information, making decisions,
            and/or acting upon decisions</skos:definition>
        <rdfs:subClassOf rdf:resource="its-sApplicationImplementation"/>
        <skos:historyNote>Introduced in ISO/TS 14812:2022</skos:historyNote>
    </owl:Class>
    <owl:Class rdf:about="b2cMobilitySharingApp">
        <clause>3.5.5.2</clause>
        <skos:prefLabel xml:lang="en">B2C mobility sharing app</skos:prefLabel>
        <skos:definition>mobility app (3.5.13.1) that assists a transport user (3.5.2.3) in
            acquiring a transport service (3.5.2.1) from a specific business</skos:definition>
        <rdfs:subClassOf rdf:resource="mobilityApp"/>
        <skos:historyNote>Introduced in ISO/TS 14812:2022</skos:historyNote>
    </owl:Class>
    <owl:Class rdf:about="navigationApp">
        <clause>3.5.5.4</clause>
        <skos:prefLabel xml:lang="en">navigation app</skos:prefLabel>
        <skos:definition>mobility app (3.5.13.1) that assists a transport user (3.5.2.3) to
            determine the best route to a destination</skos:definition>
        <rdfs:subClassOf rdf:resource="mobilityApp"/>
        <skos:historyNote>Introduced in ISO/TS 14812:2022</skos:historyNote>
    </owl:Class>
    <owl:Class rdf:about="p2pMobilitySharingApp">
        <clause>3.5.5.5</clause>
        <skos:prefLabel xml:lang="en">P2P mobility sharing app</skos:prefLabel>
        <skos:definition>mobility app (3.5.13.1) that assists a transport user (3.5.2.3) in
            acquiring transport service (3.5.2.1) from an individual that participates in the
            mobility app's network</skos:definition>
        <rdfs:subClassOf rdf:resource="mobilityApp"/>
        <skos:historyNote>Introduced in ISO/TS 14812:2022</skos:historyNote>
    </owl:Class>
    <owl:Class rdf:about="ridesourcingApp">
        <clause>3.5.5.6</clause>
        <skos:prefLabel xml:lang="en">ridesourcing app</skos:prefLabel>
        <skos:definition>P2P mobility sharing app (3.5.13.5) for acquiring a ridesourced service
            (3.5.11.5)</skos:definition>
        <rdfs:subClassOf rdf:resource="p2pMobilitySharingApp"/>
        <skos:historyNote>Introduced in ISO/TS 14812:2022</skos:historyNote>
    </owl:Class>
    <owl:Class rdf:about="publicTransportApp">
        <clause>3.5.5.7</clause>
        <skos:prefLabel xml:lang="en">public transport app</skos:prefLabel>
        <skos:definition>mobility app (3.5.13.1) that assists a transport user (3.5.2.3) in using a
            public transport (3.5.6.1) system (3.1.2.1)</skos:definition>
        <skos:note>A public transport app can include features such as viewing
            maps, searching routes and schedules, real-time arrival information, ticketing,
            electronic boarding pass, etc.</skos:note>
        <rdfs:subClassOf rdf:resource="mobilityApp"/>
        <skos:historyNote>Introduced in ISO/TS 14812:2022</skos:historyNote>
    </owl:Class>
    <owl:Class rdf:about="real-timeTravellerInformationApp">
        <clause>3.5.5.8</clause>
        <skos:prefLabel xml:lang="en">real-time traveller information app</skos:prefLabel>
        <skos:definition>mobility app (3.5.13.1) that provides information about current travel
            conditions to a transport user (3.5.2.3)</skos:definition>
        <rdfs:subClassOf rdf:resource="mobilityApp"/>
        <skos:historyNote>Introduced in ISO/TS 14812:2022</skos:historyNote>
    </owl:Class>
    <owl:Class rdf:about="taxiHailingApp">
        <clause>3.5.5.9</clause>
        <skos:prefLabel xml:lang="en">taxi hailing app</skos:prefLabel>
        <skos:definition>mobility app (3.5.13.1) that assists a transport user (3.5.2.3) in
            electronically requesting a taxi</skos:definition>
        <rdfs:subClassOf rdf:resource="mobilityApp"/>
        <skos:historyNote>Introduced in ISO/TS 14812:2022</skos:historyNote>
    </owl:Class>
    <owl:Class rdf:about="tripAggregatorApp">
        <clause>3.5.5.10</clause>
        <skos:prefLabel xml:lang="en">trip aggregator app</skos:prefLabel>
        <skos:definition>mobility app (3.5.13.1) that assists a transport user (3.5.2.3) in planning
            trips that may span multiple vehicle modes or transport providers (3.5.2.2)</skos:definition>
        <skos:note>The assistance can include reservations, ticketing and similar
            services (3.5.1.1).</skos:note>
        <rdfs:subClassOf rdf:resource="mobilityApp"/>
        <skos:historyNote>Introduced in ISO/TS 14812:2022</skos:historyNote>
    </owl:Class>
    <owl:Class rdf:about="publicTransport">
        <clause>3.5.6.1</clause>
        <skos:prefLabel xml:lang="en">public transport</skos:prefLabel>
        <altPrefLabel xml:lang="en">public transport service</altPrefLabel>
        <skos:definition>transport service (3.5.2.1) that is publicly accessible enabling the
            movement of one or more persons (3.1.1.6)</skos:definition>
        <skos:example>1 Bus, tram, cable car, metro, train and ferry are examples of public
            transport means for collective use.</skos:example>
        <skos:example>2 Publicly-accessible shared cars, shared bikes and shared el-scooters
            are examples of public transport means for shared and individual use.</skos:example>
        <skos:note>A public transport service can be scheduled or on-demand.</skos:note>
        <skos:note>A public transport service is based on the use of publicly
            accessible transport means for collective, shared or individual use.</skos:note>
        <rdfs:subClassOf rdf:resource="transportService"/>
        <skos:historyNote>Introduced in ISO/TS 14812:2022</skos:historyNote>
    </owl:Class>
    <owl:Class rdf:about="sharedTransportService">
        <clause>3.5.6.2</clause>
        <skos:prefLabel xml:lang="en">shared transport service</skos:prefLabel>
        <skos:definition>transport service (3.5.2.1) that relies upon the same resources (3.1.6.2)
            to fulfil the transport needs (3.5.2.4) of multiple unrelated transport users (3.5.2.3)
            and where the transport provider (3.5.2.2) has the primary responsibility for the
            operation of the transport mode</skos:definition>
        <skos:note>A shared transport service might not be dependent upon a vehicle
            and/or could be multi-modal. For example, a letter courier service could rely on walking
            and public transport (3.5.6.1).</skos:note>
        <skos:note>Responsibilities of the transport service can be further
            delegated to others. For example, a courier service relying on public transport would
            delegate the operation of the transport mode to the public transport operator.</skos:note>
        <rdfs:subClassOf rdf:resource="transportService"/>
        <skos:historyNote>Introduced in ISO/TS 14812:2022</skos:historyNote>
    </owl:Class>
    <owl:Class rdf:about="sharedVehicleService">
        <clause>3.5.6.3</clause>
        <skos:prefLabel xml:lang="en">shared vehicle service</skos:prefLabel>
        <skos:definition>transport service (3.5.2.1) that sequentially (3.5.9.2) provides the same
            vehicles (3.7.1.1) to multiple unrelated transport users (3.5.2.3) and where the
            transport user has the primary responsibility for the operation of the vehicle</skos:definition>
        <skos:note>As there should only be one operator of a vehicle at any time, a
            shared vehicle service should use a sequential operational model.</skos:note>
        <skos:note>This term can be specialized by replacing "vehicle" with any
            defined vehicle type (e.g. "automated vehicle sharing").</skos:note>
        <rdfs:subClassOf rdf:resource="transportService"/>
        <skos:historyNote>Introduced in ISO/TS 14812:2022</skos:historyNote>
    </owl:Class>
    <owl:Class rdf:about="transportSharing">
        <clause>3.5.6.4</clause>
        <skos:prefLabel xml:lang="en">transport sharing</skos:prefLabel>
        <skos:definition>using a shared transport service (3.5.6.2)</skos:definition>
        <rdfs:subClassOf>
            <owl:Restriction>
                <owl:onProperty rdf:resource="using"/>
                <owl:someValuesFrom rdf:resource="sharedTransportService"/>
            </owl:Restriction>
        </rdfs:subClassOf>
        <skos:historyNote>Introduced in ISO/TS 14812:2022</skos:historyNote>
    </owl:Class>
    <owl:Class rdf:about="vehicleSharing">
        <clause>3.5.6.5</clause>
        <skos:prefLabel xml:lang="en">vehicle sharing</skos:prefLabel>
        <skos:definition>using a shared vehicle service (3.5.6.3)</skos:definition>
        <skos:note>This term can be specialized by replacing "vehicle" with any
            defined vehicle type. However, in some cases the preferred form is to consolidate terms
            (e.g. "carsharing" rather than "passenger car sharing").</skos:note>
        <rdfs:subClassOf>
            <owl:Restriction>
                <owl:onProperty rdf:resource="using"/>
                <owl:someValuesFrom rdf:resource="sharedVehicleService"/>
            </owl:Restriction>
        </rdfs:subClassOf>
        <skos:historyNote>Introduced in ISO/TS 14812:2022</skos:historyNote>
    </owl:Class>
    <owl:Class rdf:about="contractualModel">
        <clause>3.5.7.1</clause>
        <skos:prefLabel xml:lang="en">contractual model</skos:prefLabel>
        <altPrefLabel xml:lang="en">shared mobility contract model</altPrefLabel>
        <skos:definition>legal framework for the agreement between a service provider (3.5.1.2) and
            a user (3.5.1.3)</skos:definition>
        <skos:note>Contracts can be via a third party, implied or verbal,
            especially in the case of peer-to-peer (3.5.7.5).</skos:note>
        <skos:historyNote>Introduced in ISO/TS 14812:2022</skos:historyNote>
    </owl:Class>
    <owl:Class rdf:about="corporateCustomerModel">
        <clause>3.5.7.2</clause>
        <skos:prefLabel xml:lang="en">corporate customer model</skos:prefLabel>
        <skos:definition>contractual model (3.5.7.1) where the user (3.5.1.3) is a commercial
            (3.5.8.2) entity (3.1.1.1)</skos:definition>
        <skos:example>1 A business purchasing monthly public transport (3.5.6.1) passes for
            its employees.</skos:example>
        <skos:example>2 A commercial entity using a commercial courier service for package
            delivery.</skos:example>
        <rdfs:subClassOf rdf:resource="contractualModel"/>
        <skos:historyNote>Introduced in ISO/TS 14812:2022</skos:historyNote>
    </owl:Class>
    <owl:Class rdf:about="privateCustomerModel">
        <clause>3.5.7.3</clause>
        <skos:prefLabel xml:lang="en">private customer model</skos:prefLabel>
        <skos:definition>contractual model (3.5.7.1) where the user (3.5.1.3) is an individual</skos:definition>
        <rdfs:subClassOf rdf:resource="contractualModel"/>
        <skos:historyNote>Introduced in ISO/TS 14812:2022</skos:historyNote>
    </owl:Class>
    <owl:Class rdf:about="governmentCustomerModel">
        <clause>3.5.7.4</clause>
        <skos:prefLabel xml:lang="en">government customer model</skos:prefLabel>
        <skos:definition>contractual model (3.5.7.1) where the user (3.5.1.3) is a governmental
            entity (3.1.1.1)</skos:definition>
        <skos:example>A governmental entity using a commercial (3.5.8.2) courier service for
            package delivery.</skos:example>
        <rdfs:subClassOf rdf:resource="contractualModel"/>
        <skos:historyNote>Introduced in ISO/TS 14812:2022</skos:historyNote>
    </owl:Class>
    <owl:Class rdf:about="peer-to-peer">
        <clause>3.5.7.5</clause>
        <skos:prefLabel xml:lang="en">peer-to-peer</skos:prefLabel>
        <skos:definition>&lt;transport service&gt; private customer model (3.5.7.3) where the
            service provider (3.5.1.2) is an individual</skos:definition>
        <skos:example>Ridesourcing.</skos:example>
        <skos:note>The customer and provider can connect and/or contract through a
            third-party service (3.5.1.1).</skos:note>
        <rdfs:subClassOf rdf:resource="contractualModel"/>
        <skos:historyNote>Introduced in ISO/TS 14812:2022</skos:historyNote>
    </owl:Class>
    <owl:Class rdf:about="financialModel">
        <clause>3.5.8.1</clause>
        <skos:prefLabel xml:lang="en">financial model</skos:prefLabel>
        <skos:definition>economic framework for the agreement between a service provider (3.5.1.2)
            and a user (3.5.1.3)</skos:definition>
        <skos:historyNote>Introduced in ISO/TS 14812:2022</skos:historyNote>
    </owl:Class>
    <owl:Class rdf:about="commercial">
        <clause>3.5.8.2</clause>
        <skos:prefLabel xml:lang="en">commercial</skos:prefLabel>
        <skos:definition>type of financial model (3.5.8.1) where services (3.5.1.1) are provided
            with a profit motive</skos:definition>
        <rdfs:subClassOf rdf:resource="financialModel"/>
        <skos:historyNote>Introduced in ISO/TS 14812:2022</skos:historyNote>
    </owl:Class>
    <owl:Class rdf:about="public">
        <clause>3.5.8.3</clause>
        <skos:prefLabel xml:lang="en">public</skos:prefLabel>
        <skos:definition>type of financial model (3.5.8.1) where services (3.5.1.1) are provided by
            an administrative authority in an attempt to better serve societal interests</skos:definition>
        <skos:note>The transport service (3.5.2.1) is typically offered to the
            transport consumer for less than the full capital and operating cost of providing the
            service, but this is not a requirement.</skos:note>
        <skos:note>Typically, the administrative authority is a local government
            agency; but it could be another administrative authority, such as the national
            government or a commercial (3.5.8.2) entity (3.1.1.1) managing transport needs (3.5.2.4)
            on their campus.</skos:note>
        <rdfs:subClassOf rdf:resource="financialModel"/>
        <skos:historyNote>Introduced in ISO/TS 14812:2022</skos:historyNote>
    </owl:Class>
    <owl:Class rdf:about="cooperative">
        <clause>3.5.8.4</clause>
        <skos:prefLabel xml:lang="en">cooperative</skos:prefLabel>
        <skos:definition>type of financial model (3.5.8.1) where users (3.5.1.3) partner to defray
            the costs of services (3.5.1.1)</skos:definition>
        <skos:note>Cooperative models are exclusive commercial (3.5.8.2) and public
            (3.5.8.3) models.</skos:note>
        <rdfs:subClassOf rdf:resource="financialModel"/>
        <skos:historyNote>Introduced in ISO/TS 14812:2022</skos:historyNote>
    </owl:Class>
    <owl:Class rdf:about="mutualBenefit">
        <clause>3.5.8.5</clause>
        <skos:prefLabel xml:lang="en">mutual benefit</skos:prefLabel>
        <skos:definition>cooperative (3.5.8.4) financial model (3.5.8.1) where users (3.5.1.3)
            partner on a per-use basis</skos:definition>
        <rdfs:subClassOf rdf:resource="cooperative"/>
        <skos:historyNote>Introduced in ISO/TS 14812:2022</skos:historyNote>
    </owl:Class>
    <owl:Class rdf:about="fractionalOwnership">
        <clause>3.5.8.6</clause>
        <skos:prefLabel xml:lang="en">fractional ownership</skos:prefLabel>
        <skos:definition>&lt;transport service&gt; cooperative (3.5.8.4) financial model (3.5.8.1)
            where users (3.5.1.3) partner to support the purchase, maintenance and overhead costs
            associated with a service (3.5.1.1)</skos:definition>
        <rdfs:subClassOf rdf:resource="cooperative"/>
        <skos:historyNote>Introduced in ISO/TS 14812:2022</skos:historyNote>
    </owl:Class>
    <owl:Class rdf:about="private">
        <clause>3.5.8.7</clause>
        <skos:prefLabel xml:lang="en">private</skos:prefLabel>
        <skos:definition>&lt;transport service&gt; financial model (3.5.8.1) where services
            (3.5.1.1) are provided to members of the owning organization without usage fees</skos:definition>
        <skos:example>Fleet vehicles of an employer.</skos:example>
        <rdfs:subClassOf rdf:resource="financialModel"/>
        <skos:historyNote>Introduced in ISO/TS 14812:2022</skos:historyNote>
    </owl:Class>
    <owl:Class rdf:about="membership-based">
        <clause>3.5.8.8</clause>
        <skos:prefLabel xml:lang="en">membership-based</skos:prefLabel>
        <skos:definition>characteristic of a financial model (3.5.8.1) that requires users (3.5.1.3)
            to enter into an agreement prior to receiving services (3.5.1.1)</skos:definition>
        <skos:note>The agreement can be associated with fees.</skos:note>
        <skos:note>The agreement can be minimal, such as collecting user
            information for business purposes.</skos:note>
        <skos:note>The membership can be granted as a part of a broader agreement.
            For example, a university bus system (3.1.2.1) can restrict access to students and
            faculty.</skos:note>
        <rdfs:subClassOf>
            <owl:Restriction>
                <owl:onProperty rdf:resource="describes"/>
                <owl:someValuesFrom rdf:resource="financialModel"/>
            </owl:Restriction>
        </rdfs:subClassOf>
        <skos:historyNote>Introduced in ISO/TS 14812:2022</skos:historyNote>
    </owl:Class>
    <owl:Class rdf:about="open-access">
        <clause>3.5.8.9</clause>
        <skos:prefLabel xml:lang="en">open-access</skos:prefLabel>
        <skos:definition>characteristic of a financial model (3.5.8.1) that does not require
            membership within an organization to receive services (3.5.1.1)</skos:definition>
        <skos:note>This includes models where membership is optional and can
            provide extra benefits.</skos:note>
        <rdfs:subClassOf>
            <owl:Restriction>
                <owl:onProperty rdf:resource="describes"/>
                <owl:someValuesFrom rdf:resource="financialModel"/>
            </owl:Restriction>
        </rdfs:subClassOf>
        <skos:historyNote>Introduced in ISO/TS 14812:2022</skos:historyNote>
    </owl:Class>
    <owl:Class rdf:about="operationalModel">
        <clause>3.5.9.1</clause>
        <skos:prefLabel xml:lang="en">operational model</skos:prefLabel>
        <skos:definition>logistical framework for the agreement between a service provider (3.5.1.2)
            and a user (3.5.1.3)</skos:definition>
        <skos:note>The logistical framework can set restrictions on how a passenger
            (3.6.2.1) and/or good is received, transported and/or delivered.</skos:note>
        <skos:historyNote>Introduced in ISO/TS 14812:2022</skos:historyNote>
    </owl:Class>
    <owl:Class rdf:about="sequential">
        <clause>3.5.9.2</clause>
        <skos:prefLabel xml:lang="en">sequential</skos:prefLabel>
        <skos:definition>operational model (3.5.9.1) where services (3.5.1.1) are provided to a
            single user (3.5.1.3) at any one time</skos:definition>
        <skos:example>Traditional taxi service.</skos:example>
        <skos:note>A single transport consumer can request the transport of
            multiple passengers (3.6.2.1).</skos:note>
        <rdfs:subClassOf rdf:resource="operationalModel"/>
        <skos:historyNote>Introduced in ISO/TS 14812:2022</skos:historyNote>
    </owl:Class>
    <owl:Class rdf:about="concurrent">
        <clause>3.5.9.3</clause>
        <skos:prefLabel xml:lang="en">concurrent</skos:prefLabel>
        <skos:definition>operational model (3.5.9.1) where services (3.5.1.1) can be provided to
            multiple users (3.5.1.3) at any one time</skos:definition>
        <rdfs:subClassOf rdf:resource="operationalModel"/>
        <skos:historyNote>Introduced in ISO/TS 14812:2022</skos:historyNote>
    </owl:Class>
    <owl:Class rdf:about="fixedRoute">
        <clause>3.5.9.4</clause>
        <skos:prefLabel xml:lang="en">fixed route</skos:prefLabel>
        <skos:definition>&lt;transport service&gt; concurrent (3.5.9.3) operation where transported
            items can only be received or delivered at stopping points contained in a pre-defined
            sequence</skos:definition>
        <skos:example>Traditional fixed-route bus line.</skos:example>
        <rdfs:subClassOf rdf:resource="concurrent"/>
        <skos:historyNote>Introduced in ISO/TS 14812:2022</skos:historyNote>
    </owl:Class>
    <owl:Class rdf:about="dynamicRoute">
        <clause>3.5.9.5</clause>
        <skos:prefLabel xml:lang="en">dynamic route</skos:prefLabel>
        <skos:definition>&lt;transport service&gt; concurrent (3.5.9.3) operation where transported
            items can only be received or delivered at stopping points within a pre-defined service
            (3.5.1.1) corridor</skos:definition>
        <skos:example>Airport shuttle.</skos:example>
        <skos:note>The service corridor is defined by the provider, who may impose
            further restrictions on where stops are allowed.</skos:note>
        <skos:note>The service corridor often includes a communal point of interest
            (e.g. an airport, transit hub, etc.) as a fixed stopping point.</skos:note>
        <rdfs:subClassOf rdf:resource="concurrent"/>
        <skos:historyNote>Introduced in ISO/TS 14812:2022</skos:historyNote>
    </owl:Class>
    <owl:Class rdf:about="pairedOn-demand">
        <clause>3.5.9.6</clause>
        <skos:prefLabel xml:lang="en">paired on-demand</skos:prefLabel>
        <skos:definition>&lt;transport service&gt; concurrent (3.5.9.3) operation where the
            transport provider (3.5.2.2) may choose to divert from its path to service a new request
            from another transport users (3.5.2.3) while servicing an earlier transport user</skos:definition>
        <skos:example>Ridesplitting.</skos:example>
        <rdfs:subClassOf rdf:resource="concurrent"/>
        <skos:historyNote>Introduced in ISO/TS 14812:2022</skos:historyNote>
    </owl:Class>
    <owl:Class rdf:about="networkModel">
        <clause>3.5.10.1</clause>
        <skos:prefLabel xml:lang="en">network model</skos:prefLabel>
        <skos:definition>infrastructure framework for the agreement between a service provider
            (3.5.1.2) and a user (3.5.1.3)</skos:definition>
        <skos:historyNote>Introduced in ISO/TS 14812:2022</skos:historyNote>
    </owl:Class>
    <owl:Class rdf:about="station-basedRoundtrip">
        <clause>3.5.10.2</clause>
        <skos:prefLabel xml:lang="en">station-based roundtrip</skos:prefLabel>
        <skos:definition>&lt;transport service&gt; operational mode (3.5.9.1) where the transport
            service (3.5.2.1) is initiated and terminated at the same facility managed by the
            transport provider (3.5.2.2)</skos:definition>
        <rdfs:subClassOf rdf:resource="networkModel"/>
        <skos:historyNote>Introduced in ISO/TS 14812:2022</skos:historyNote>
    </owl:Class>
    <owl:Class rdf:about="station-basedOne-way">
        <clause>3.5.10.3</clause>
        <skos:prefLabel xml:lang="en">station-based one-way</skos:prefLabel>
        <skos:definition>&lt;transport service&gt; operational mode (3.5.9.1) where the transport
            service (3.5.2.1) is initiated and terminated at two different facilities managed by the
            transport provider (3.5.2.2)</skos:definition>
        <rdfs:subClassOf rdf:resource="networkModel"/>
        <skos:historyNote>Introduced in ISO/TS 14812:2022</skos:historyNote>
    </owl:Class>
    <owl:Class rdf:about="free-floating">
        <clause>3.5.10.4</clause>
        <skos:prefLabel xml:lang="en">free-floating</skos:prefLabel>
        <skos:definition>&lt;transport service&gt; network model (3.5.10.1) where the transport
            service (3.5.2.1) may be initiated and terminated at any location (3.4.1.1) meeting
            basic criteria</skos:definition>
        <skos:note>The basic criteria typically include geographic limits and
            requirements related to legal and safe locations.</skos:note>
        <rdfs:subClassOf rdf:resource="networkModel"/>
        <skos:historyNote>Introduced in ISO/TS 14812:2022</skos:historyNote>
    </owl:Class>
    <owl:Class rdf:about="shuttleService">
        <clause>3.5.11.1</clause>
        <skos:prefLabel xml:lang="en">shuttle service</skos:prefLabel>
        <skos:definition>shared transport service (3.5.6.2) that transports passengers (3.6.2.1)
            between two specified locations (3.4.1.1)</skos:definition>
        <skos:note>Each location can be defined as point, linear or area locations
            (3.4.1.6). However, the areas of the two locations should not overlap.</skos:note>
        <rdfs:subClassOf rdf:resource="sharedTransportService"/>
        <skos:historyNote>Introduced in ISO/TS 14812:2022</skos:historyNote>
    </owl:Class>
    <owl:Class rdf:about="taxiService">
        <clause>3.5.11.2</clause>
        <skos:prefLabel xml:lang="en">taxi service</skos:prefLabel>
        <skos:definition>commercial (3.5.8.2) shared transport service (3.5.6.2) that transports
            passengers (3.6.2.1) sequentially (3.5.9.2)</skos:definition>
        <rdfs:subClassOf rdf:resource="sharedTransportService"/>
        <skos:historyNote>Introduced in ISO/TS 14812:2022</skos:historyNote>
    </owl:Class>
    <owl:Class rdf:about="taxi-shareService">
        <clause>3.5.11.3</clause>
        <skos:prefLabel xml:lang="en">taxi-share service</skos:prefLabel>
        <skos:definition>commercial (3.5.8.2) shared transport service (3.5.6.2) that transports
            passengers (3.6.2.1) concurrently (3.5.9.3)</skos:definition>
        <rdfs:subClassOf rdf:resource="sharedTransportService"/>
        <skos:historyNote>Introduced in ISO/TS 14812:2022</skos:historyNote>
    </owl:Class>
    <owl:Class rdf:about="rideshareService">
        <clause>3.5.11.4</clause>
        <skos:prefLabel xml:lang="en">rideshare service</skos:prefLabel>
        <skos:definition>cooperative (3.5.8.4) shared transport service (3.5.6.2) that transports
            passengers (3.6.2.1) concurrently (3.5.9.3)</skos:definition>
        <rdfs:subClassOf rdf:resource="sharedTransportService"/>
        <skos:historyNote>Introduced in ISO/TS 14812:2022</skos:historyNote>
    </owl:Class>
    <owl:Class rdf:about="ridesourcedService">
        <clause>3.5.11.5</clause>
        <skos:prefLabel xml:lang="en">ridesourced service</skos:prefLabel>
        <skos:definition>commercial (3.5.8.2), peer-to-peer (3.5.7.5) shared transport service
            (3.5.6.2) that transports passengers (3.6.2.1)</skos:definition>
        <rdfs:subClassOf rdf:resource="sharedTransportService"/>
        <skos:historyNote>Introduced in ISO/TS 14812:2022</skos:historyNote>
    </owl:Class>
    <owl:Class rdf:about="ridesplitService">
        <clause>3.5.11.6</clause>
        <skos:prefLabel xml:lang="en">ridesplit service</skos:prefLabel>
        <skos:definition>ridesourced service (3.5.11.5) that serves passengers (3.6.2.1)
            concurrently (3.5.9.3)</skos:definition>
        <rdfs:subClassOf rdf:resource="ridesourcedService"/>
        <skos:historyNote>Introduced in ISO/TS 14812:2022</skos:historyNote>
    </owl:Class>
    <owl:Class rdf:about="courierNetworkService">
        <clause>3.5.11.7</clause>
        <skos:prefLabel xml:lang="en">courier network service</skos:prefLabel>
        <skos:definition>commercial (3.5.8.2), peer-to-peer (3.5.7.5) shared transport service
            (3.5.6.2) that transports goods</skos:definition>
        <skos:note>The goods are typically small packages, letters, food, etc.</skos:note>
        <rdfs:subClassOf rdf:resource="sharedTransportService"/>
        <skos:historyNote>Introduced in ISO/TS 14812:2022</skos:historyNote>
    </owl:Class>
    <owl:Class rdf:about="bikesharingService">
        <clause>3.5.12.1</clause>
        <skos:prefLabel xml:lang="en">bikesharing service</skos:prefLabel>
        <skos:altLabel xml:lang="en">bicycle sharing service</skos:altLabel>
        <skos:definition>shared vehicle service (3.5.6.3) that shares bicycles</skos:definition>
        <skos:note>The term "bicycle sharing service" is admitted, but "bikesharing
            service" is preferred as it has fewer syllables.</skos:note>
        <rdfs:subClassOf rdf:resource="sharedVehicleService"/>
        <skos:historyNote>Introduced in ISO/TS 14812:2022</skos:historyNote>
    </owl:Class>
    <owl:Class rdf:about="carsharingService">
        <clause>3.5.12.2</clause>
        <skos:prefLabel xml:lang="en">carsharing service</skos:prefLabel>
        <skos:altLabel xml:lang="en">passenger car sharing service</skos:altLabel>
        <skos:definition>shared vehicle service (3.5.6.3) that shares passenger (3.6.2.1) cars</skos:definition>
        <skos:note>The term "passenger car sharing service" is admitted but has the
            same meaning.</skos:note>
        <rdfs:subClassOf rdf:resource="sharedVehicleService"/>
        <skos:historyNote>Introduced in ISO/TS 14812:2022</skos:historyNote>
    </owl:Class>
    <owl:Class rdf:about="traveller">
        <clause>3.6.1.1</clause>
        <skos:prefLabel xml:lang="en">traveller</skos:prefLabel>
        <skos:definition>person (3.1.1.6) who is headed to a destination</skos:definition>
        <rdfs:subClassOf>
            <owl:Restriction>
                <owl:onProperty rdf:resource="isA"/>
                <owl:someValuesFrom rdf:resource="person"/>
            </owl:Restriction>
        </rdfs:subClassOf>
        <skos:historyNote>Introduced in ISO/TS 14812:2022</skos:historyNote>
    </owl:Class>
    <owl:Class rdf:about="roadUser">
        <clause>3.6.1.2</clause>
        <skos:prefLabel xml:lang="en">road user</skos:prefLabel>
        <skos:definition>mobile material entity (3.1.1.3) within the road reservation (3.3.1.2)</skos:definition>
        <skos:example>Pedestrians (3.6.1.4), road work personnel, vehicle occupants
            (3.6.2.2), occupied and unoccupied vehicles, horses, etc.</skos:example>
        <rdfs:subClassOf>
            <owl:Restriction>
                <owl:onProperty rdf:resource="locatedWithin"/>
                <owl:someValuesFrom rdf:resource="roadReservation"/>
            </owl:Restriction>
        </rdfs:subClassOf>
        <skos:historyNote>Introduced in ISO/TS 14812:2022</skos:historyNote>
    </owl:Class>
    <owl:Class rdf:about="pedestrian">
        <clause>3.6.1.4</clause>
        <skos:prefLabel xml:lang="en">pedestrian</skos:prefLabel>
        <skos:definition>person (3.1.1.6) who is travelling on foot</skos:definition>
        <rdfs:subClassOf rdf:resource="traveller"/>
        <skos:historyNote>Introduced in ISO/TS 14812:2022</skos:historyNote>
    </owl:Class>
    <owl:Class rdf:about="vulnerableRoadUser">
        <clause>3.6.1.5</clause>
        <skos:prefLabel xml:lang="en">vulnerable road user</skos:prefLabel>
        <skos:definition>road user (3.6.1.2) who is not protected by the body of a motor vehicle
            that meets local safety regulations</skos:definition>
        <skos:example>Pedestrian (3.6.1.4), cyclist, motorcyclist, road work personnel,
            horse, horseback rider, person with disabilities (e.g., wheelchair), etc.</skos:example>
        <rdfs:subClassOf rdf:resource="roadUser"/>
        <skos:historyNote>Introduced in ISO/TS 14812:2025</skos:historyNote>
    </owl:Class>
    <owl:Class rdf:about="protectedRoadUser">
        <clause>3.6.1.6</clause>
        <skos:prefLabel xml:lang="en">protected road user</skos:prefLabel>
        <skos:altLabel xml:lang="en">non-vulnerable road user</skos:altLabel>
        <skos:definition>road user (3.6.1.2) who is protected by the body of a motor vehicle that
            meets local safety regulations</skos:definition>
        <skos:example>vehicle occupants (3.6.2.2)</skos:example>
        <rdfs:subClassOf rdf:resource="roadUser"/>
        <skos:historyNote>Introduced in ISO/TS 14812:2025</skos:historyNote>
    </owl:Class>
    <owl:Class rdf:about="passenger">
        <clause>3.6.2.1</clause>
        <skos:prefLabel xml:lang="en">passenger</skos:prefLabel>
        <skos:definition>person (3.1.1.6) who has a reservation to travel or is travelling in a
            vehicle (3.7.1.1) except for any crew, staff or drivers (3.6.2.3)</skos:definition>
        <rdfs:subClassOf>
            <owl:Restriction>
                <owl:onProperty rdf:resource="isA"/>
                <owl:someValuesFrom rdf:resource="person"/>
            </owl:Restriction>
        </rdfs:subClassOf>
        <rdfs:subClassOf>
            <owl:Restriction>
                <owl:onProperty rdf:resource="travellingIn"/>
                <owl:someValuesFrom rdf:resource="vehicle"/>
            </owl:Restriction>
        </rdfs:subClassOf>
        <skos:historyNote>Introduced in ISO/TS 14812:2022</skos:historyNote>
    </owl:Class>
    <owl:Class rdf:about="vehicleOccupant">
        <clause>3.6.2.2</clause>
        <skos:prefLabel xml:lang="en">vehicle occupant</skos:prefLabel>
        <skos:definition>person (3.1.1.6) in or on a vehicle (3.7.1.1)</skos:definition>
        <skos:note>A vehicle occupant in a stationary vehicle is not necessarily a
            traveller (3.6.1.1).</skos:note>
        <rdfs:subClassOf>
            <owl:Restriction>
                <owl:onProperty rdf:resource="isA"/>
                <owl:someValuesFrom rdf:resource="person"/>
            </owl:Restriction>
        </rdfs:subClassOf>
        <rdfs:subClassOf>
            <owl:Restriction>
                <owl:onProperty rdf:resource="isIn"/>
                <owl:someValuesFrom rdf:resource="vehicle"/>
            </owl:Restriction>
        </rdfs:subClassOf>
        <skos:historyNote>Introduced in ISO/TS 14812:2022</skos:historyNote>
    </owl:Class>
    <owl:Class rdf:about="driver">
        <clause>3.6.2.3</clause>
        <skos:prefLabel xml:lang="en">driver</skos:prefLabel>
        <skos:definition>person (3.1.1.6) that is currently responsible for the dynamic driving task
            (3.7.3.1) for the vehicle (3.7.1.1)</skos:definition>
        <skos:note>The driver is typically on-board the vehicle but could be remote
            from the vehicle or automated logic.</skos:note>
        <rdfs:subClassOf>
            <owl:Restriction>
                <owl:onProperty rdf:resource="isA"/>
                <owl:someValuesFrom rdf:resource="person"/>
            </owl:Restriction>
        </rdfs:subClassOf>
        <skos:historyNote>Introduced in ISO/TS 14812:2022</skos:historyNote>
    </owl:Class>
    <owl:Class rdf:about="in-vehicleDriver">
        <clause>3.6.2.4</clause>
        <skos:prefLabel xml:lang="en">in-vehicle driver</skos:prefLabel>
        <altPrefLabel xml:lang="en">conventional driver</altPrefLabel>
        <skos:definition>driver (3.6.2.3) that performs the dynamic driving task (3.7.3.1) using the
            vehicle's (3.7.1.1) built-in input devices (3.7.1.5) to control the longitudinal and
            lateral movement of the vehicle</skos:definition>
        <rdfs:subClassOf rdf:resource="driver"/>
        <rdfs:subClassOf>
            <owl:Restriction>
                <owl:onProperty rdf:resource="uses"/>
                <owl:someValuesFrom rdf:resource="built-inVehicleInputDevice"/>
            </owl:Restriction>
        </rdfs:subClassOf>
        <skos:historyNote>Introduced in ISO/TS 14812:2022</skos:historyNote>
    </owl:Class>
    <owl:Class rdf:about="remoteDriver">
        <clause>3.6.2.5</clause>
        <skos:prefLabel xml:lang="en">remote driver</skos:prefLabel>
        <skos:definition>driver (3.6.2.3) that performs the dynamic driving task (3.7.3.1) without
            using the vehicle's (3.7.1.1) built-in input devices (3.7.1.5) to control the
            longitudinal and lateral movement of the vehicle</skos:definition>
        <skos:note>A remote driver can use a variety of physical input devices, but
            none that are built into the vehicle.</skos:note>
        <rdfs:subClassOf rdf:resource="driver"/>
        <rdfs:subClassOf>
            <owl:Restriction>
                <owl:onProperty rdf:resource="uses"/>
                <owl:minQualifiedCardinality rdf:datatype="xsd:nonNegativeInteger">1</owl:minQualifiedCardinality>
                <owl:onClass>
                    <owl:Class>
                        <owl:unionOf rdf:parseType="Collection">
                            <rdf:Description rdf:about="nomadicVehicleInputDevice"/>
                            <rdf:Description rdf:about="remoteVehicleInputDevice"/>
                        </owl:unionOf>
                    </owl:Class>
                </owl:onClass>
            </owl:Restriction>
        </rdfs:subClassOf>
        <skos:historyNote>Introduced in ISO/TS 14812:2022</skos:historyNote>
    </owl:Class>
    <owl:Class rdf:about="vehicle">
        <clause>3.7.1.1</clause>
        <skos:prefLabel xml:lang="en">vehicle</skos:prefLabel>
        <skos:definition>material entity (3.1.1.3) designed to transport people or physical goods by
            changing its physical position</skos:definition>
        <rdfs:subClassOf rdf:resource="materialEntity"/>
        <rdfs:subClassOf>
            <owl:Restriction>
                <owl:onProperty rdf:resource="ddtControlledBy"/>
                <owl:qualifiedCardinality rdf:datatype="xsd:nonNegativeInteger">1</owl:qualifiedCardinality>
                <owl:onClass>
                    <owl:Class>
                        <owl:unionOf rdf:parseType="Collection">
                            <rdf:Description rdf:about="driver"/>
                            <rdf:Description rdf:about="ads"/>
                        </owl:unionOf>
                    </owl:Class>
                </owl:onClass>
            </owl:Restriction>
        </rdfs:subClassOf>
        <rdfs:subClassOf>
            <owl:Restriction>
                <owl:onProperty rdf:resource="has"/>
                <owl:minQualifiedCardinality rdf:datatype="xsd:nonNegativeInteger">0</owl:minQualifiedCardinality>
                <owl:onClass rdf:resource="wheel"/>
            </owl:Restriction>
        </rdfs:subClassOf>
        <rdfs:subClassOf>
            <owl:Restriction>
                <owl:onProperty rdf:resource="has"/>
                <owl:minQualifiedCardinality rdf:datatype="xsd:nonNegativeInteger">0</owl:minQualifiedCardinality>
                <owl:onClass rdf:resource="motor"/>
            </owl:Restriction>
        </rdfs:subClassOf>
        <rdfs:subClassOf>
            <owl:Restriction>
                <owl:onProperty rdf:resource="has"/>
                <owl:someValuesFrom rdf:resource="vehicleInputDevice"/>
            </owl:Restriction>
        </rdfs:subClassOf>
        <rdfs:subClassOf>
            <owl:Restriction>
                <owl:onProperty rdf:resource="canBe"/>
                <owl:minQualifiedCardinality rdf:datatype="xsd:nonNegativeInteger">1</owl:minQualifiedCardinality>
                <owl:onClass>
                    <owl:Class>
                        <owl:unionOf rdf:parseType="Collection">
                            <rdf:Description rdf:about="off-grid"/>
                            <rdf:Description rdf:about="connected"/>
                        </owl:unionOf>
                    </owl:Class>
                </owl:onClass>
            </owl:Restriction>
        </rdfs:subClassOf>
        <skos:historyNote>Introduced in ISO/TS 14812:2022</skos:historyNote>
    </owl:Class>
    <owl:Class rdf:about="motor">
        <clause>3.7.1.2</clause>
        <skos:prefLabel xml:lang="en">motor</skos:prefLabel>
        <skos:altLabel xml:lang="en">engine</skos:altLabel>
        <skos:definition>material entity (3.1.1.3) that converts energy into mechanical motion</skos:definition>
        <rdfs:subClassOf rdf:resource="materialEntity"/>
        <skos:historyNote>Introduced in ISO/TS 14812:2022</skos:historyNote>
    </owl:Class>
    <owl:Class rdf:about="wheel">
        <clause>3.7.1.3</clause>
        <skos:prefLabel xml:lang="en">wheel</skos:prefLabel>
        <skos:definition>circular material entity (3.1.1.3) that rotates about an axle to facilitate
            movement of the vehicle (3.7.1.1)</skos:definition>
        <rdfs:subClassOf rdf:resource="materialEntity"/>
        <skos:historyNote>Introduced in ISO/TS 14812:2022</skos:historyNote>
    </owl:Class>
    <owl:Class rdf:about="vehicleInputDevice">
        <clause>3.7.1.4</clause>
        <skos:prefLabel xml:lang="en">vehicle input device</skos:prefLabel>
        <altPrefLabel xml:lang="en">input device</altPrefLabel>
        <skos:definition>material entity (3.1.1.3) that can affect the vehicle's (3.7.1.1) operation</skos:definition>
        <skos:example>steering wheel, lever, pedal, knob, button, touch screen</skos:example>
        <skos:note>Input devices include those used to control the motion of the
            vehicle (e.g. a brake pedal), the state of vehicular equipment (e.g. headlight control),
            the configuration of the vehicle (e.g. temperature control), etc.</skos:note>
        <rdfs:subClassOf rdf:resource="materialEntity"/>
        <skos:historyNote>Introduced in ISO/TS 14812:2022</skos:historyNote>
    </owl:Class>
    <owl:Class rdf:about="built-inVehicleInputDevice">
        <clause>3.7.1.5</clause>
        <skos:prefLabel xml:lang="en">built-in vehicle input device</skos:prefLabel>
        <altPrefLabel xml:lang="en">built-in input device</altPrefLabel>
        <skos:definition>input device (3.7.1.4) designed to be physically connected (3.2.3.6) to a
            vehicle (3.7.1.1) and to remain connected even when the vehicle is not in use</skos:definition>
        <skos:note>Built-in input devices include devices that can be temporarily
            disconnected (3.7.4.3) for security reasons (e.g. some radios are equipped with
            detachable front panels).</skos:note>
        <skos:note>Built-in input devices are typically considered to be a part of
            the vehicle.</skos:note>
        <skos:note>Built-in input devices require a maintenance operation to
            connect or disconnect.</skos:note>
        <rdfs:subClassOf rdf:resource="vehicleInputDevice"/>
        <skos:historyNote>Introduced in ISO/TS 14812:2022</skos:historyNote>
    </owl:Class>
    <owl:Class rdf:about="nomadicVehicleInputDevice">
        <clause>3.7.1.6</clause>
        <skos:prefLabel xml:lang="en">nomadic vehicle input device</skos:prefLabel>
        <altPrefLabel xml:lang="en">nomadic input device</altPrefLabel>
        <skos:definition>input device (3.7.1.4) that can be carried into, or in near proximity of, a
            vehicle (3.7.1.1) and connected (3.2.3.6) as desired</skos:definition>
        <skos:example>A smartphone connected to a vehicle (via USB or Bluetooth) to provide
            driver (3.6.2.3) navigation on the vehicle's large screen display</skos:example>
        <skos:note>NDs are often more closely associated with a person (3.1.1.6)
            than they are with the vehicle.</skos:note>
        <skos:note>Nomadic input devices do not require a maintenance operation to
            connect or disconnect.</skos:note>
        <rdfs:subClassOf rdf:resource="vehicleInputDevice"/>
        <skos:historyNote>Introduced in ISO/TS 14812:2022</skos:historyNote>
    </owl:Class>
    <owl:Class rdf:about="remoteVehicleInputDevice">
        <clause>3.7.1.7</clause>
        <skos:prefLabel xml:lang="en">remote vehicle input device</skos:prefLabel>
        <altPrefLabel xml:lang="en">remote input device</altPrefLabel>
        <skos:definition>input device (3.7.1.4) designed to be electronically connected (3.2.3.6) to
            a vehicle (3.7.1.1) even when the vehicle is not in close proximity</skos:definition>
        <rdfs:subClassOf rdf:resource="vehicleInputDevice"/>
        <skos:historyNote>Introduced in ISO/TS 14812:2022</skos:historyNote>
    </owl:Class>
    <owl:Class rdf:about="speed">
        <clause>3.7.2.1</clause>
        <skos:prefLabel xml:lang="en">speed</skos:prefLabel>
        <skos:definition>rate of change of a material entity's (3.1.1.3) position with respect to a
            frame of reference</skos:definition>
        <skos:note>Speed is a function of time.</skos:note>
        <skos:note>Speed is the scalar absolute value (magnitude) of velocity.</skos:note>
        <rdfs:subClassOf>
            <owl:Restriction>
                <owl:onProperty rdf:resource="rateOfChangeOfPositionOf"/>
                <owl:qualifiedCardinality rdf:datatype="xsd:nonNegativeInteger">1</owl:qualifiedCardinality>
                <owl:onClass rdf:resource="materialEntity"/>
            </owl:Restriction>
        </rdfs:subClassOf>
        <skos:historyNote>Introduced in ISO/TS 14812:2022</skos:historyNote>
    </owl:Class>
    <owl:Class rdf:about="designSpeed">
        <clause>3.7.2.2</clause>
        <skos:prefLabel xml:lang="en">design speed</skos:prefLabel>
        <altPrefLabel xml:lang="en">vehicle design speed</altPrefLabel>
        <skos:altLabel xml:lang="en">top speed</skos:altLabel>
        <skos:definition>&lt;vehicle&gt; maximum speed (3.7.2.1) at which a vehicle (3.7.1.1) is
            intended to operate for a sustained period of time</skos:definition>
        <skos:note>The term "top speed" is defined in SAE J3194 in relation to
            powered micromobility vehicles and is considered to be semantically equivalent to design
            speed.</skos:note>
        <rdfs:subClassOf>
            <owl:Restriction>
                <owl:onProperty rdf:resource="maximumSustainedSpeedOf"/>
                <owl:qualifiedCardinality rdf:datatype="xsd:nonNegativeInteger">1</owl:qualifiedCardinality>
                <owl:onClass rdf:resource="vehicle"/>
            </owl:Restriction>
        </rdfs:subClassOf>
        <skos:historyNote>Introduced in ISO/TS 14812:2022</skos:historyNote>
    </owl:Class>
    <owl:Class rdf:about="anonymizedVehicleReference">
        <clause>3.7.2.3</clause>
        <skos:prefLabel xml:lang="en">anonymized vehicle reference</skos:prefLabel>
        <skos:definition>reference for a vehicle derived from vehicle properties such as
            registration number but encoded so that it does not allow a human to identify the
            vehicle directly from the encoded value</skos:definition>
        <rdfs:subClassOf>
            <owl:Restriction>
                <owl:onProperty rdf:resource="encodedReferenceFor"/>
                <owl:qualifiedCardinality rdf:datatype="xsd:nonNegativeInteger">1</owl:qualifiedCardinality>
                <owl:onClass rdf:resource="vehicle"/>
            </owl:Restriction>
        </rdfs:subClassOf>
        <skos:historyNote>Introduced in ISO/TS 14812:2025</skos:historyNote>
    </owl:Class>
    <owl:Class rdf:about="vehicleEquipment">
        <clause>3.7.2.4</clause>
        <skos:prefLabel xml:lang="en">vehicle equipment</skos:prefLabel>
        <skos:definition>type of equipment in use or on board the vehicle</skos:definition>
        <rdfs:subClassOf>
            <owl:Restriction>
                <owl:onProperty rdf:resource="inUseOrOnBoard"/>
                <owl:qualifiedCardinality rdf:datatype="xsd:nonNegativeInteger">1</owl:qualifiedCardinality>
                <owl:onClass rdf:resource="vehicle"/>
            </owl:Restriction>
        </rdfs:subClassOf>
        <skos:historyNote>Introduced in ISO/TS 14812:2025</skos:historyNote>
    </owl:Class>
    <owl:Class rdf:about="vehicleFuelType">
        <clause>3.7.2.5</clause>
        <skos:prefLabel xml:lang="en">vehicle fuel type</skos:prefLabel>
        <skos:definition>type of fuel used by the vehicle</skos:definition>
        <rdfs:subClassOf>
            <owl:Restriction>
                <owl:onProperty rdf:resource="fuelUsedBy"/>
                <owl:qualifiedCardinality rdf:datatype="xsd:nonNegativeInteger">1</owl:qualifiedCardinality>
                <owl:onClass rdf:resource="vehicle"/>
            </owl:Restriction>
        </rdfs:subClassOf>
        <skos:historyNote>Introduced in ISO/TS 14812:2025</skos:historyNote>
    </owl:Class>
    <owl:Class rdf:about="vehicleIdentifier">
        <clause>3.7.2.6</clause>
        <skos:prefLabel xml:lang="en">vehicle identifier</skos:prefLabel>
        <skos:definition>series of 17 characters that is based on either ISO 3779 or ISO 3780 and
            uniquely identifies the individual vehicle and is normally securely attached to the
            vehicle chassis</skos:definition>
        <rdfs:subClassOf>
            <owl:Restriction>
                <owl:onProperty rdf:resource="globallyUniqueIdentifierFor"/>
                <owl:qualifiedCardinality rdf:datatype="xsd:nonNegativeInteger">1</owl:qualifiedCardinality>
                <owl:onClass rdf:resource="vehicle"/>
            </owl:Restriction>
        </rdfs:subClassOf>
        <skos:historyNote>Introduced in ISO/TS 14812:2025</skos:historyNote>
    </owl:Class>
    <owl:Class rdf:about="vehicleLoadType">
        <clause>3.7.2.7</clause>
        <skos:prefLabel xml:lang="en">vehicle load type</skos:prefLabel>
        <skos:definition>type of load carried by the vehicle</skos:definition>
        <rdfs:subClassOf>
            <owl:Restriction>
                <owl:onProperty rdf:resource="loadCarriedBy"/>
                <owl:qualifiedCardinality rdf:datatype="xsd:nonNegativeInteger">1</owl:qualifiedCardinality>
                <owl:onClass rdf:resource="vehicle"/>
            </owl:Restriction>
        </rdfs:subClassOf>
        <skos:historyNote>Introduced in ISO/TS 14812:2025</skos:historyNote>
    </owl:Class>
    <owl:Class rdf:about="vehicleRegistrationPlateIdentifier">
        <clause>3.7.2.8</clause>
        <skos:prefLabel xml:lang="en">vehicle registration plate identifier</skos:prefLabel>
        <skos:definition>numeric or alphanumeric identifier or code, displayed on a registration
            plate attached to the vehicle, and unique within the issuing authority's region
            therefore usable for official identification purposes</skos:definition>
        <rdfs:subClassOf>
            <owl:Restriction>
                <owl:onProperty rdf:resource="identifierUniqueWithinRegionFor"/>
                <owl:qualifiedCardinality rdf:datatype="xsd:nonNegativeInteger">1</owl:qualifiedCardinality>
                <owl:onClass rdf:resource="vehicle"/>
            </owl:Restriction>
        </rdfs:subClassOf>
        <skos:historyNote>Introduced in ISO/TS 14812:2025</skos:historyNote>
    </owl:Class>
    <owl:Class rdf:about="grossVehicleMass">
        <clause>3.7.2.9</clause>
        <skos:prefLabel xml:lang="en">gross vehicle mass</skos:prefLabel>
        <skos:altLabel xml:lang="en">gross vehicle weight</skos:altLabel>
        <skos:definition>operating mass (weight) of the vehicle according to legislation and/or
            regulations for the applicable region Note 1 to entry: Gross vehicle mass is often used
            to designate weight limits (e.g., on bridges).</skos:definition>
        <rdfs:subClassOf>
            <owl:Restriction>
                <owl:onProperty rdf:resource="operatingMassOf"/>
                <owl:qualifiedCardinality rdf:datatype="xsd:nonNegativeInteger">1</owl:qualifiedCardinality>
                <owl:onClass rdf:resource="vehicle"/>
            </owl:Restriction>
        </rdfs:subClassOf>
        <skos:historyNote>Introduced in ISO/TS 14812:2025</skos:historyNote>
    </owl:Class>
    <owl:Class rdf:about="grossVehicleMassRating">
        <clause>3.7.2.10</clause>
        <skos:prefLabel xml:lang="en">gross vehicle mass rating</skos:prefLabel>
        <skos:altLabel xml:lang="en">gross vehicle weight rating</skos:altLabel>
        <skos:definition>maximum operating mass (weight) of the vehicle, as determined by the
            vehicle manufacturer, at which the vehicle can be safely and reliably operated for its
            intended purpose</skos:definition>
        <rdfs:subClassOf>
            <owl:Restriction>
                <owl:onProperty rdf:resource="maxOperatingWeightFor"/>
                <owl:qualifiedCardinality rdf:datatype="xsd:nonNegativeInteger">1</owl:qualifiedCardinality>
                <owl:onClass rdf:resource="vehicle"/>
            </owl:Restriction>
        </rdfs:subClassOf>
        <skos:historyNote>Introduced in ISO/TS 14812:2025</skos:historyNote>
    </owl:Class>
    <owl:Class rdf:about="dynamicDrivingTask">
        <clause>3.7.3.1</clause>
        <skos:prefLabel xml:lang="en">dynamic driving task</skos:prefLabel>
        <altPrefLabel xml:lang="en">DDT</altPrefLabel>
        <skos:definition>all real-time operational and tactical functions required to operate a
            vehicle (3.7.1.1) in on-road traffic</skos:definition>
        <skos:note>The DDT includes lateral vehicle motion control, longitudinal
            vehicle motion control, monitoring the driving environment (3.1.3.11), object and event
            response execution, manoeuvre planning and enhancing conspicuity.</skos:note>
        <skos:note>The DDT excludes strategic functions such as trip scheduling and
            selection of destinations and waypoints.</skos:note>
        <rdfs:subClassOf>
            <owl:Restriction>
                <owl:onProperty rdf:resource="isRequiredToOperate"/>
                <owl:someValuesFrom rdf:resource="vehicle"/>
            </owl:Restriction>
        </rdfs:subClassOf>
        <skos:historyNote>Introduced in ISO/TS 14812:2022</skos:historyNote>
    </owl:Class>
    <owl:Class rdf:about="operationalDesignDomain">
        <clause>3.7.3.2</clause>
        <skos:prefLabel xml:lang="en">operational design domain</skos:prefLabel>
        <altPrefLabel xml:lang="en">ODD</altPrefLabel>
        <skos:definition>set of operating conditions under which a given driving automation system
            (3.7.3.6) or feature thereof is specifically designed to function</skos:definition>
        <skos:example>1 ADS (3.7.3.10) feature designed to operate a vehicle (3.7.1.1) only
            on fully access-controlled freeways in low-speed traffic, under fair weather conditions
            and optimal road (3.3.5.1) maintenance conditions (e.g. good lane markings and not under
            construction).</skos:example>
        <skos:example>2 ADS-dedicated vehicle designed to operate only within a
            geographically-defined area, and only during daylight at speeds not exceeding 25 mph.</skos:example>
        <skos:note>The conditions can include environmental, geographical,
            time-of-day, and/or other restrictions.</skos:note>
        <skos:note>The conditions can require the presence or absence of certain
            traffic or roadway (3.3.1.3) characteristics.</skos:note>
        <rdfs:subClassOf>
            <owl:Restriction>
                <owl:onProperty rdf:resource="forAGiven"/>
                <owl:someValuesFrom rdf:resource="drivingAutomationSystem"/>
            </owl:Restriction>
        </rdfs:subClassOf>
        <skos:historyNote>Introduced in ISO/TS 14812:2022</skos:historyNote>
    </owl:Class>
    <owl:Class rdf:about="fallback">
        <clause>3.7.3.3</clause>
        <skos:prefLabel xml:lang="en">fallback</skos:prefLabel>
        <altPrefLabel xml:lang="en">driving automation fallback</altPrefLabel>
        <skos:definition>&lt;driving automation&gt; response by a person (3.1.1.6) to perform the
            DDT (3.7.3.1) or by an ADS (3.7.3.10) to achieve a minimal risk condition when the
            response is triggered upon violation of the defined operational design domain (3.7.3.2)
            constraints or in response to a DDT performance-relevant driving automation system
            (3.7.3.6) failure</skos:definition>
        <skos:note>This term includes the response of a person to perform the DDT
            in a manner to quickly achieve a minimal risk condition.</skos:note>
        <rdfs:subClassOf>
            <owl:Restriction>
                <owl:onProperty rdf:resource="mayBeCausedBy"/>
                <owl:someValuesFrom rdf:resource="ddtPerformance-relevantSystemFailure"/>
            </owl:Restriction>
        </rdfs:subClassOf>
        <rdfs:subClassOf>
            <owl:Restriction>
                <owl:onProperty rdf:resource="mayBeCausedByAViolationOf"/>
                <owl:someValuesFrom rdf:resource="operationalDesignDomain"/>
            </owl:Restriction>
        </rdfs:subClassOf>
        <skos:historyNote>Introduced in ISO/TS 14812:2022</skos:historyNote>
    </owl:Class>
    <owl:Class rdf:about="fallback-readyUser">
        <clause>3.7.3.4</clause>
        <skos:prefLabel xml:lang="en">fallback-ready user</skos:prefLabel>
        <altPrefLabel xml:lang="en">DDT fallback-ready user</altPrefLabel>
        <skos:definition>&lt;driving automation&gt; person (3.1.1.6) who is able to operate the
            vehicle (3.7.1.1) if the Level 3 ADS (3.7.3.11) issues a request to intervene or if that
            person otherwise identifies a condition that requires intervention to perform the DDT
            (3.7.3.1)</skos:definition>
        <rdfs:subClassOf>
            <owl:Restriction>
                <owl:onProperty rdf:resource="readyToPerform"/>
                <owl:someValuesFrom rdf:resource="dynamicDrivingTask"/>
            </owl:Restriction>
        </rdfs:subClassOf>
        <skos:historyNote>Introduced in ISO/TS 14812:2022</skos:historyNote>
    </owl:Class>
    <owl:Class rdf:about="ddtPerformance-relevantSystemFailure">
        <clause>3.7.3.5</clause>
        <skos:prefLabel xml:lang="en">DDT performance-relevant system failure</skos:prefLabel>
        <skos:definition>malfunction in a vehicle system (3.2.1.5) that prevents the driving
            automation system (3.7.3.6) from reliably performing its portion of the DDT (3.7.3.1) on
            a sustained basis</skos:definition>
        <skos:note>The malfunction can be internal to the driving automation system
            or part of another vehicle system.</skos:note>
        <skos:historyNote>Introduced in ISO/TS 14812:2022</skos:historyNote>
    </owl:Class>
    <owl:Class rdf:about="drivingAutomationSystem">
        <clause>3.7.3.6</clause>
        <skos:prefLabel xml:lang="en">driving automation system</skos:prefLabel>
        <skos:definition>hardware and software system (3.1.2.1) that is able to perform part or all
            of the DDT (3.7.3.1) on a sustained basis</skos:definition>
        <skos:note>In contrast to this generic term for any level 1-5 system, the
            specific term for a level 3-5 system is "Automated Driving System (ADS)." Given the
            similarity between the generic term, "driving automation system," and the level
            3-5-specific term, "Automated Driving System," the latter term is intentionally
            capitalized when spelled out and reduced to its acronym, "ADS", as much as possible,
            while "driving automation system" should not be.</skos:note>
        <skos:note>A driving automation system includes any system capable of level
            1-5 driving automation.</skos:note>
        <skos:note>Driving automation levels are defined in ISO/SAE 22736, which is
            also known as SAE J3016.</skos:note>
        <skos:note>Driving automation levels include "level 1 driving automation"
            (3.7.3.8), "level 2 driving automation" (3.7.3.9), "level 3 ADS" (3.7.3.11), "level 4
            ADS" (3.7.3.12) and "level 5 ADS" (3.7.3.13).</skos:note>
        <rdfs:subClassOf>
            <owl:Restriction>
                <owl:onProperty rdf:resource="performsPartOrAllOf"/>
                <owl:someValuesFrom rdf:resource="dynamicDrivingTask"/>
            </owl:Restriction>
        </rdfs:subClassOf>
        <skos:historyNote>Introduced in ISO/TS 14812:2022</skos:historyNote>
    </owl:Class>
    <owl:Class rdf:about="driverSupportSystem">
        <clause>3.7.3.7</clause>
        <skos:prefLabel xml:lang="en">driver support system</skos:prefLabel>
        <skos:definition>driving automation system (3.7.3.6) that is only able to perform part of
            the DDT (3.7.3.1)</skos:definition>
        <skos:note>Driver support systems include level 1 (3.7.3.8) and level 2
            driving automation (3.7.3.9).</skos:note>
        <rdfs:subClassOf rdf:resource="drivingAutomationSystem"/>
        <rdfs:subClassOf>
            <owl:Restriction>
                <owl:onProperty rdf:resource="performsPartOf"/>
                <owl:someValuesFrom rdf:resource="dynamicDrivingTask"/>
            </owl:Restriction>
        </rdfs:subClassOf>
        <skos:historyNote>Introduced in ISO/TS 14812:2022</skos:historyNote>
    </owl:Class>
    <owl:Class rdf:about="level1DrivingAutomation">
        <clause>3.7.3.8</clause>
        <skos:prefLabel xml:lang="en">level 1 driving automation</skos:prefLabel>
        <altPrefLabel xml:lang="en">driver assistance</altPrefLabel>
        <skos:definition>driver support system (3.7.3.7) that provides either sustained lateral or
            sustained longitudinal vehicle (3.7.1.1) motion control within a specific operational
            design domain (3.7.3.2) with the expectation that a conventional driver (3.6.2.4)
            completes the DDT (3.7.3.1)</skos:definition>
        <skos:note>Other driving automation levels include "level 2 driving
            automation" (3.7.3.9), "level 3 ADS" (3.7.3.11), "level 4 ADS" (3.7.3.12), and "level 5
            ADS" (3.7.3.13).</skos:note>
        <rdfs:subClassOf rdf:resource="driverSupportSystem"/>
        <rdfs:subClassOf>
            <owl:Restriction>
                <owl:onProperty rdf:resource="operatesWithinA"/>
                <owl:someValuesFrom rdf:resource="operationalDesignDomain"/>
            </owl:Restriction>
        </rdfs:subClassOf>
        <skos:historyNote>Introduced in ISO/TS 14812:2022</skos:historyNote>
    </owl:Class>
    <owl:Class rdf:about="level2DrivingAutomation">
        <clause>3.7.3.9</clause>
        <skos:prefLabel xml:lang="en">level 2 driving automation</skos:prefLabel>
        <altPrefLabel xml:lang="en">partial driving automation</altPrefLabel>
        <skos:definition>driver support system (3.7.3.7) that provides sustained lateral and
            longitudinal vehicle (3.7.1.1) motion control within a specific operational design
            domain (3.7.3.2) with the expectation that a conventional driver (3.6.2.4) completes the
            object and event detection and response</skos:definition>
        <skos:note>Other driving automation levels include "level 1 driving
            automation" (3.7.3.8), "level 3 ADS" (3.7.3.11), "level 4 ADS" (3.7.3.12), and "level 5
            ADS" (3.7.3.13).</skos:note>
        <rdfs:subClassOf rdf:resource="driverSupportSystem"/>
        <rdfs:subClassOf>
            <owl:Restriction>
                <owl:onProperty rdf:resource="operatesWithinA"/>
                <owl:someValuesFrom rdf:resource="operationalDesignDomain"/>
            </owl:Restriction>
        </rdfs:subClassOf>
        <skos:historyNote>Introduced in ISO/TS 14812:2022</skos:historyNote>
    </owl:Class>
    <owl:Class rdf:about="ads">
        <clause>3.7.3.10</clause>
        <skos:prefLabel xml:lang="en">ADS</skos:prefLabel>
        <altPrefLabel xml:lang="en">Automated Driving System</altPrefLabel>
        <skos:definition>driving automation system (3.7.3.6) that is able to perform the entire DDT
            (3.7.3.1) on a sustained basis</skos:definition>
        <skos:note>The abbreviated form ("ADS") is the most preferred form and the
            alternative form ("Automated Driving System") uses initial capitals to avoid confusion
            with the more general "driving automation system".</skos:note>
        <rdfs:subClassOf rdf:resource="drivingAutomationSystem"/>
        <rdfs:subClassOf>
            <owl:Restriction>
                <owl:onProperty rdf:resource="performsAllOf"/>
                <owl:someValuesFrom rdf:resource="dynamicDrivingTask"/>
            </owl:Restriction>
        </rdfs:subClassOf>
        <rdfs:subClassOf>
            <owl:Restriction>
                <owl:onProperty rdf:resource="canControl"/>
                <owl:someValuesFrom rdf:resource="ads-equippedVehicle"/>
            </owl:Restriction>
        </rdfs:subClassOf>
        <skos:historyNote>Introduced in ISO/TS 14812:2022</skos:historyNote>
    </owl:Class>
    <owl:Class rdf:about="level3Ads">
        <clause>3.7.3.11</clause>
        <skos:prefLabel xml:lang="en">level 3 ADS</skos:prefLabel>
        <altPrefLabel xml:lang="en">conditional driving automation</altPrefLabel>
        <altPrefLabel xml:lang="en">level 3 Automated Driving System</altPrefLabel>
        <skos:definition>ADS (3.7.3.10) designed with the expectation that the fallback-ready user
            (3.7.3.4) is available to intervene</skos:definition>
        <skos:note>Level 3 ADSs are restricted to operating within a specific ODD
            (3.7.3.2).</skos:note>
        <skos:note>Other driving automation levels include "level 1 driving
            automation" (3.7.3.8), "level 2 driving automation" (3.7.3.9), "level 4 ADS" (3.7.3.12),
            and "level 5 ADS" (3.7.3.13).</skos:note>
        <skos:note>The user can intervene due to an ADS-issued request, a DDT
            (3.7.3.1) performance-relevant system failure, or other reasons.</skos:note>
        <rdfs:subClassOf rdf:resource="ads"/>
        <rdfs:subClassOf>
            <owl:Restriction>
                <owl:onProperty rdf:resource="operatesWithinA"/>
                <owl:someValuesFrom rdf:resource="operationalDesignDomain"/>
            </owl:Restriction>
        </rdfs:subClassOf>
        <rdfs:subClassOf>
            <owl:Restriction>
                <owl:onProperty rdf:resource="designedWithExpectationOf"/>
                <owl:someValuesFrom rdf:resource="fallback-readyUser"/>
            </owl:Restriction>
        </rdfs:subClassOf>
        <skos:historyNote>Introduced in ISO/TS 14812:2022</skos:historyNote>
    </owl:Class>
    <owl:Class rdf:about="level4Ads">
        <clause>3.7.3.12</clause>
        <skos:prefLabel xml:lang="en">level 4 ADS</skos:prefLabel>
        <altPrefLabel xml:lang="en">high driving automation</altPrefLabel>
        <altPrefLabel xml:lang="en">level 4 Automated Driving System</altPrefLabel>
        <skos:definition>ADS (3.7.3.10) that is capable of operating within a specific ODD (3.7.3.2)
            and providing its own fallback (3.7.3.3), without any expectation that a human driver
            (3.6.2.3) will respond to a request to intervene</skos:definition>
        <skos:note>Other driving automation levels include "level 1 driving
            automation" (3.7.3.8), "level 2 driving automation" (3.7.3.9), "level 3 ADS" (3.7.3.11),
            and "level 5 ADS" (3.7.3.13).</skos:note>
        <rdfs:subClassOf rdf:resource="ads"/>
        <rdfs:subClassOf>
            <owl:Restriction>
                <owl:onProperty rdf:resource="operatesWithinA"/>
                <owl:someValuesFrom rdf:resource="operationalDesignDomain"/>
            </owl:Restriction>
        </rdfs:subClassOf>
        <rdfs:subClassOf>
            <owl:Restriction>
                <owl:onProperty rdf:resource="providesItsOwn"/>
                <owl:someValuesFrom rdf:resource="fallback"/>
            </owl:Restriction>
        </rdfs:subClassOf>
        <skos:historyNote>Introduced in ISO/TS 14812:2022</skos:historyNote>
    </owl:Class>
    <owl:Class rdf:about="level5Ads">
        <clause>3.7.3.13</clause>
        <skos:prefLabel xml:lang="en">level 5 ADS</skos:prefLabel>
        <altPrefLabel xml:lang="en">full driving automation</altPrefLabel>
        <altPrefLabel xml:lang="en">level 5 Automated Driving System</altPrefLabel>
        <skos:definition>ADS (3.7.3.10) that is capable of unconditional (i.e. not ODD
            (3.7.3.2)-specific) operation and providing its own fallback (3.7.3.3), without any
            expectation that a human driver (3.6.2.3) will respond to a request to intervene</skos:definition>
        <skos:note>Other driving automation levels include "level 1 driving
            automation" (3.7.3.8), "level 2 driving automation" (3.7.3.9), "level 3 ADS" (3.7.3.11)
            and "level 4 ADS" (3.7.3.12).</skos:note>
        <rdfs:subClassOf rdf:resource="ads"/>
        <rdfs:subClassOf>
            <owl:Restriction>
                <owl:onProperty rdf:resource="operatesWithinA"/>
                <owl:someValuesFrom rdf:resource="operationalDesignDomain"/>
            </owl:Restriction>
        </rdfs:subClassOf>
        <rdfs:subClassOf>
            <owl:Restriction>
                <owl:onProperty rdf:resource="providesItsOwn"/>
                <owl:someValuesFrom rdf:resource="fallback"/>
            </owl:Restriction>
        </rdfs:subClassOf>
        <skos:historyNote>Introduced in ISO/TS 14812:2022</skos:historyNote>
    </owl:Class>
    <owl:Class rdf:about="conventionalVehicle">
        <clause>3.7.3.14</clause>
        <skos:prefLabel xml:lang="en">conventional vehicle</skos:prefLabel>
        <altPrefLabel xml:lang="en">automation-equipped conventional vehicle</altPrefLabel>
        <skos:definition>&lt;driving automation&gt; vehicle (3.7.1.1) designed to be operated by a
            person (3.1.1.6) during part or all of every trip.</skos:definition>
        <rdfs:subClassOf rdf:resource="vehicle"/>
        <skos:historyNote>Introduced in ISO/TS 14812:2022</skos:historyNote>
    </owl:Class>
    <owl:Class rdf:about="ads-equippedVehicle">
        <clause>3.7.3.15</clause>
        <skos:prefLabel xml:lang="en">ADS-equipped vehicle</skos:prefLabel>
        <skos:altLabel xml:lang="en">automated vehicle</skos:altLabel>
        <skos:altLabel xml:lang="en">AV</skos:altLabel>
        <skos:hiddenLabel xml:lang="en">autonomous vehicle</skos:hiddenLabel>
        <skos:definition>vehicle (3.7.1.1) integrated with an ADS (3.7.3.10)</skos:definition>
        <skos:note>The terms "automated vehicle" and "AV" are often used in a
            colloquial form. However, these terms can be used to mean either an "ADS-equipped
            vehicle" or a "vehicle with an engaged ADS". The term "ADS-equipped vehicle" is
            preferred since it is more precise and descriptive in its meaning.</skos:note>
        <skos:note>The term "autonomous vehicle" is also often used in a colloquial
            form and is even less well defined. The term is particularly problematic because the
            word "autonomous" has been used for a long time in the robotics and artificial
            intelligence research communities to signify systems (3.1.2.1) that have the ability and
            authority to make decisions independently and self-sufficiently. Due to its imprecise
            and overly broad meaning, use of the term "autonomous vehicle" is discouraged.</skos:note>
        <skos:note>This term can be, and when possible should be, refined by
            identifying the level of automation. For example, the terms "level 5 ADS-equipped
            vehicle" and "level 5 automated vehicle" should be interpreted as "ADS-equipped vehicle
            where the ADS is a level 5 ADS." (3.7.3.13).</skos:note>
        <skos:note>This term only describes the capabilities of the vehicle, not
            its operational state. In other words, the term applies as long as the ADS is connected
            (3.2.3.6) to the vehicle, whether the DDT (3.7.3.1) is actively engaged or not.</skos:note>
        <rdfs:subClassOf rdf:resource="vehicle"/>
        <rdfs:subClassOf>
            <owl:Restriction>
                <owl:onProperty rdf:resource="comprises"/>
                <owl:someValuesFrom rdf:resource="ads"/>
            </owl:Restriction>
        </rdfs:subClassOf>
        <skos:historyNote>Introduced in ISO/TS 14812:2022</skos:historyNote>
    </owl:Class>
    <owl:Class rdf:about="dual-modeVehicle">
        <clause>3.7.3.16</clause>
        <skos:prefLabel xml:lang="en">dual-mode vehicle</skos:prefLabel>
        <altPrefLabel xml:lang="en">driving automation dual-mode vehicle</altPrefLabel>
        <skos:definition>&lt;driving automation&gt; ADS-equipped vehicle (3.7.3.15) designed for
            both driverless operation and operation by a conventional driver (3.6.2.4) for complete
            trips</skos:definition>
        <rdfs:subClassOf rdf:resource="ads-equippedVehicle"/>
        <skos:historyNote>Introduced in ISO/TS 14812:2022</skos:historyNote>
    </owl:Class>
    <owl:Class rdf:about="ads-dedicatedVehicle">
        <clause>3.7.3.17</clause>
        <skos:prefLabel xml:lang="en">ADS-dedicated vehicle</skos:prefLabel>
        <skos:definition>ADS-equipped vehicle (3.7.3.15) designed for only driverless operation for
            complete trips</skos:definition>
        <rdfs:subClassOf rdf:resource="ads-equippedVehicle"/>
        <skos:historyNote>Introduced in ISO/TS 14812:2022</skos:historyNote>
    </owl:Class>
    <owl:Class rdf:about="off-grid">
        <clause>3.7.4.1</clause>
        <skos:prefLabel xml:lang="en">off-grid</skos:prefLabel>
        <altPrefLabel xml:lang="en">ITS off-grid</altPrefLabel>
        <skos:definition>characteristic of a material entity (3.1.1.3) that is currently unable to
            send data to or receive data from connected (3.2.3.6) entities</skos:definition>
        <rdfs:subClassOf>
            <owl:Restriction>
                <owl:onProperty rdf:resource="characteristicOf"/>
                <owl:someValuesFrom rdf:resource="materialEntity"/>
            </owl:Restriction>
        </rdfs:subClassOf>
        <skos:historyNote>Introduced in ISO/TS 14812:2022</skos:historyNote>
    </owl:Class>
    <owl:Class rdf:about="unconnected">
        <clause>3.7.4.2</clause>
        <skos:prefLabel xml:lang="en">unconnected</skos:prefLabel>
        <altPrefLabel xml:lang="en">ITS unconnected</altPrefLabel>
        <skos:definition>characteristic of a material entity (3.1.1.3) that is equipped with
            communications equipment that is not active or is otherwise unable to send data to or
            receive data from connected (3.2.3.6) entities</skos:definition>
        <rdfs:subClassOf rdf:resource="off-grid"/>
        <skos:historyNote>Introduced in ISO/TS 14812:2022</skos:historyNote>
    </owl:Class>
    <owl:Class rdf:about="disconnected">
        <clause>3.7.4.3</clause>
        <skos:prefLabel xml:lang="en">disconnected</skos:prefLabel>
        <altPrefLabel xml:lang="en">ITS disconnected</altPrefLabel>
        <skos:definition>characteristic of a material entity (3.1.1.3) that is or was equipped with
            communications equipment that is sufficiently physically disconnected such that the
            material entity is no longer able to send data to or receive data from connected
            (3.2.3.6) entities</skos:definition>
        <skos:note>The vehicle on-board equipment can still be present in the
            vehicle (3.7.1.1) and can even be partially connected, but not in any operational sense.</skos:note>
        <rdfs:subClassOf rdf:resource="off-grid"/>
        <skos:historyNote>Introduced in ISO/TS 14812:2022</skos:historyNote>
    </owl:Class>
    <owl:Class rdf:about="unequipped">
        <clause>3.7.4.4</clause>
        <skos:prefLabel xml:lang="en">unequipped</skos:prefLabel>
        <altPrefLabel xml:lang="en">ITS unequipped</altPrefLabel>
        <skos:definition>characteristic of a material entity (3.1.1.3) that is not and has never
            been equipped with communications equipment for sending data to or receiving data from
            connected (3.2.3.6) entities</skos:definition>
        <rdfs:subClassOf rdf:resource="off-grid"/>
        <skos:historyNote>Introduced in ISO/TS 14812:2022</skos:historyNote>
    </owl:Class>
    <owl:Class rdf:about="ultra-low-speedVehicle">
        <clause>3.7.5.1</clause>
        <skos:prefLabel xml:lang="en">ultra-low-speed vehicle</skos:prefLabel>
        <skos:altLabel xml:lang="en">pedestrian-speed vehicle</skos:altLabel>
        <skos:definition>vehicle (3.7.1.1) with a design speed (3.7.2.2) that does not exceed
            ultra-low vehicle speeds (3.7.5.7)</skos:definition>
        <skos:note>The term "pedestrian speed vehicle" is allowed but the preferred
            term follows a logical progression of levels.</skos:note>
        <rdfs:subClassOf rdf:resource="vehicle"/>
        <skos:historyNote>Introduced in ISO/TS 14812:2022</skos:historyNote>
    </owl:Class>
    <owl:Class rdf:about="low-speedVehicle">
        <clause>3.7.5.2</clause>
        <skos:prefLabel xml:lang="en">low-speed vehicle</skos:prefLabel>
        <skos:altLabel xml:lang="en">cycle-speed vehicle</skos:altLabel>
        <skos:definition>vehicle (3.7.1.1) with a design speed (3.7.2.2) in the range of low vehicle
            speeds (3.7.5.8)</skos:definition>
        <skos:example>Mountain bicycle.</skos:example>
        <skos:note>The term "cycle-speed vehicle" is allowed but the preferred term
            follows a logical progression of levels.</skos:note>
        <rdfs:subClassOf rdf:resource="vehicle"/>
        <skos:historyNote>Introduced in ISO/TS 14812:2022</skos:historyNote>
    </owl:Class>
    <owl:Class rdf:about="moderatelyLow-speedVehicle">
        <clause>3.7.5.3</clause>
        <skos:prefLabel xml:lang="en">moderately low-speed vehicle</skos:prefLabel>
        <skos:definition>vehicle (3.7.1.1) with a design speed (3.7.2.2) in the range of
            moderately-low vehicle speeds (3.7.5.9)</skos:definition>
        <skos:example>Typical moped.</skos:example>
        <rdfs:subClassOf rdf:resource="vehicle"/>
        <skos:historyNote>Introduced in ISO/TS 14812:2022</skos:historyNote>
    </owl:Class>
    <owl:Class rdf:about="moderate-speedVehicle">
        <clause>3.7.5.4</clause>
        <skos:prefLabel xml:lang="en">moderate-speed vehicle</skos:prefLabel>
        <skos:definition>vehicle (3.7.1.1) with a design speed (3.7.2.2) in the range of moderate
            vehicle speeds (3.7.5.10)</skos:definition>
        <skos:example>Typical side-by-side utility task vehicle (UTV).</skos:example>
        <rdfs:subClassOf rdf:resource="vehicle"/>
        <skos:historyNote>Introduced in ISO/TS 14812:2022</skos:historyNote>
    </owl:Class>
    <owl:Class rdf:about="moderatelyHigh-speedVehicle">
        <clause>3.7.5.5</clause>
        <skos:prefLabel xml:lang="en">moderately high-speed vehicle</skos:prefLabel>
        <skos:definition>vehicle (3.7.1.1) with a design speed (3.7.2.2) in the range of
            moderately-high vehicle speeds (3.7.5.11)</skos:definition>
        <skos:example>Typical passenger (3.6.2.1) car.</skos:example>
        <rdfs:subClassOf rdf:resource="vehicle"/>
        <skos:historyNote>Introduced in ISO/TS 14812:2022</skos:historyNote>
    </owl:Class>
    <owl:Class rdf:about="high-speedVehicle">
        <clause>3.7.5.6</clause>
        <skos:prefLabel xml:lang="en">high-speed vehicle</skos:prefLabel>
        <skos:definition>vehicle (3.7.1.1) with a design speed (3.7.2.2) in the range of high
            vehicle speeds (3.7.5.12)</skos:definition>
        <skos:example>1 Racing car.</skos:example>
        <skos:example>2 High-speed train</skos:example>
        <rdfs:subClassOf rdf:resource="vehicle"/>
        <skos:historyNote>Introduced in ISO/TS 14812:2022</skos:historyNote>
    </owl:Class>
    <owl:Class rdf:about="ultra-lowVehicleSpeed">
        <clause>3.7.5.7</clause>
        <skos:prefLabel xml:lang="en">ultra-low vehicle speed</skos:prefLabel>
        <skos:definition>speed (3.7.2.1) of a vehicle (3.7.1.1) that does not greatly exceed typical
            pedestrian (3.6.1.4) speeds</skos:definition>
        <skos:example>SAE J3194 associates this with a top speed of less than 13 km/h.</skos:example>
        <skos:note>Local regulations for the exact speed range vary.</skos:note>
        <rdfs:subClassOf rdf:resource="speed"/>
        <skos:historyNote>Introduced in ISO/TS 14812:2022</skos:historyNote>
    </owl:Class>
    <owl:Class rdf:about="lowVehicleSpeed">
        <clause>3.7.5.8</clause>
        <skos:prefLabel xml:lang="en">low vehicle speed</skos:prefLabel>
        <skos:definition>speed (3.7.2.1) of a vehicle (3.7.1.1) that exceeds pedestrian (3.6.1.4)
            speeds and is more typical of pedal cycles</skos:definition>
        <skos:example>SAE J3194 associates this with a top speed in the range between 13
            km/h and 32 km/h.</skos:example>
        <skos:note>Local regulations for the exact speed range vary.</skos:note>
        <rdfs:subClassOf rdf:resource="speed"/>
        <skos:historyNote>Introduced in ISO/TS 14812:2022</skos:historyNote>
    </owl:Class>
    <owl:Class rdf:about="moderately-lowVehicleSpeed">
        <clause>3.7.5.9</clause>
        <skos:prefLabel xml:lang="en">moderately-low vehicle speed</skos:prefLabel>
        <skos:definition>speed (3.7.2.1) of a vehicle (3.7.1.1) that exceeds speeds typical of pedal
            cycles but can be reached on performance pedal cycles in short bursts or by performance
            riders</skos:definition>
        <skos:example>SAE J3194 associates this with a top speed in the range of 32 km/h to
            48 km/h.</skos:example>
        <skos:note>Local regulations for the exact speed range vary.</skos:note>
        <rdfs:subClassOf rdf:resource="speed"/>
        <skos:historyNote>Introduced in ISO/TS 14812:2022</skos:historyNote>
    </owl:Class>
    <owl:Class rdf:about="moderateVehicleSpeed">
        <clause>3.7.5.10</clause>
        <skos:prefLabel xml:lang="en">moderate vehicle speed</skos:prefLabel>
        <skos:definition>speed (3.7.2.1) of a vehicle (3.7.1.1) that exceeds moderately-low vehicle
            speeds (3.7.5.9) but does not reach free-flow motorway speeds</skos:definition>
        <skos:example>A speed in the range of 48 km/h and 87 km/h.</skos:example>
        <skos:note>Local regulations for the exact speed range vary.</skos:note>
        <rdfs:subClassOf rdf:resource="speed"/>
        <skos:historyNote>Introduced in ISO/TS 14812:2022</skos:historyNote>
    </owl:Class>
    <owl:Class rdf:about="moderately-highVehicleSpeed">
        <clause>3.7.5.11</clause>
        <skos:prefLabel xml:lang="en">moderately-high vehicle speed</skos:prefLabel>
        <skos:definition>speed (3.7.2.1) of a vehicle (3.7.1.1) that is typical of free-flow
            motorway speeds to twice that speed</skos:definition>
        <skos:example>A speed in the range of 87 km/h and 198 km/h.</skos:example>
        <skos:note>Local regulations for the exact speed range vary.</skos:note>
        <rdfs:subClassOf rdf:resource="speed"/>
        <skos:historyNote>Introduced in ISO/TS 14812:2022</skos:historyNote>
    </owl:Class>
    <owl:Class rdf:about="highVehicleSpeed">
        <clause>3.7.5.12</clause>
        <skos:prefLabel xml:lang="en">high vehicle speed</skos:prefLabel>
        <skos:definition>speed (3.7.2.1) of a vehicle (3.7.1.1) that exceeds free flow motorway
            speeds by a factor of two or more</skos:definition>
        <skos:example>A speed in excess of 198 km/h.</skos:example>
        <skos:note>Local regulations for the exact speed range vary.</skos:note>
        <rdfs:subClassOf rdf:resource="speed"/>
        <skos:historyNote>Introduced in ISO/TS 14812:2022</skos:historyNote>
    </owl:Class>
    <owl:Class rdf:about="roadVehicle">
        <clause>3.7.6.1</clause>
        <skos:prefLabel xml:lang="en">road vehicle</skos:prefLabel>
        <skos:definition>vehicle (3.7.1.1) meeting the requirements to operate within the driving
            space (3.3.1.4) of a road (3.3.5.1)</skos:definition>
        <skos:note>Unless indicated otherwise, the term typically refers to
            vehicles that are allowed to operate in the same driving spaces as motorized passenger
            (3.6.2.1) cars, according to the legal requirements of the local jurisdictional entity
            (3.1.1.1). However, the term can be contextualized for other environments (3.1.3.11).
            For example, a bicycle is a "road vehicle" when the "road" is a cycleway (3.3.3.2).</skos:note>
        <rdfs:subClassOf rdf:resource="vehicle"/>
        <skos:historyNote>Introduced in ISO/TS 14812:2022</skos:historyNote>
    </owl:Class>
    <owl:Class rdf:about="motorizedVehicle">
        <clause>3.7.6.2</clause>
        <skos:prefLabel xml:lang="en">motorized vehicle</skos:prefLabel>
        <skos:definition>self-propelled vehicle (3.7.1.1)</skos:definition>
        <rdfs:subClassOf rdf:resource="vehicle"/>
        <skos:historyNote>Introduced in ISO/TS 14812:2022</skos:historyNote>
    </owl:Class>
    <owl:Class rdf:about="motorVehicle">
        <clause>3.7.6.3</clause>
        <skos:prefLabel xml:lang="en">motor vehicle</skos:prefLabel>
        <skos:definition>motorized (3.7.6.2) road vehicle (3.7.6.1) allowed to operate in the same
            driving spaces (3.3.1.4) as motorized passenger (3.6.2.1) cars</skos:definition>
        <rdfs:subClassOf rdf:resource="roadVehicle"/>
        <rdfs:subClassOf rdf:resource="motorizedVehicle"/>
        <skos:historyNote>Introduced in ISO/TS 14812:2022</skos:historyNote>
    </owl:Class>
    <owl:Class rdf:about="non-roadVehicle">
        <clause>3.7.6.4</clause>
        <skos:prefLabel xml:lang="en">non-road vehicle</skos:prefLabel>
        <skos:definition>vehicle (3.7.1.1) not meeting the legal requirements to be driven in
            traffic lanes (3.3.1.13) or cycle lanes (3.3.3.1) of a road network (3.3.5.2)</skos:definition>
        <rdfs:subClassOf rdf:resource="vehicle"/>
        <skos:historyNote>Introduced in ISO/TS 14812:2022</skos:historyNote>
    </owl:Class>
    <owl:Class rdf:about="roadCycle">
        <clause>3.7.6.5</clause>
        <skos:prefLabel xml:lang="en">road cycle</skos:prefLabel>
        <skos:definition>vehicle (3.7.1.1) meeting the legal requirements to operate in cycle lanes
            (3.3.3.1) and cycleways (3.3.3.2)</skos:definition>
        <skos:note>In some countries, other special lanes (3.3.1.12) could also be
            open to road cycles, such as bus lanes.</skos:note>
        <rdfs:subClassOf rdf:resource="vehicle"/>
        <skos:historyNote>Introduced in ISO/TS 14812:2022</skos:historyNote>
    </owl:Class>
    <owl:Class rdf:about="non-roadCycle">
        <clause>3.7.6.6</clause>
        <skos:prefLabel xml:lang="en">non-road cycle</skos:prefLabel>
        <skos:definition>human-powered vehicle (3.7.1.1) not meeting the legal requirements to be
            driven in cycle lanes (3.3.3.1)</skos:definition>
        <rdfs:subClassOf rdf:resource="vehicle"/>
        <skos:historyNote>Introduced in ISO/TS 14812:2022</skos:historyNote>
    </owl:Class>
    <owl:Class rdf:about="paymentMeans">
        <clause>3.8.1.1</clause>
        <skos:prefLabel xml:lang="en">payment means</skos:prefLabel>
        <skos:definition>financial instrument accepted by the service provider, that gives the user
            the right to use provided services</skos:definition>
        <skos:example>token, stored electronic account, fleet card, bank account, credit card, contract</skos:example>
        <rdfs:subClassOf>
            <owl:Restriction>
                <owl:onProperty rdf:resource="acceptedBy"/>
                <owl:someValuesFrom rdf:resource="serviceProvider"/>
            </owl:Restriction>
        </rdfs:subClassOf>
        <skos:historyNote>Introduced in ISO/TS 14812:2025</skos:historyNote>
    </owl:Class>
    <owl:Class rdf:about="paymentMode">
        <clause>3.8.1.2</clause>
        <skos:prefLabel xml:lang="en">payment mode</skos:prefLabel>
        <skos:altLabel xml:lang="en">payment method</skos:altLabel>
        <skos:definition>timing and location of remuneration for services including whether the
            payment is required prior to, at the time of or post access to the service or commodity</skos:definition>
        <skos:example>pre-payment</skos:example>
        <rdfs:subClassOf>
            <owl:Restriction>
                <owl:onProperty rdf:resource="timingAndLocationOfRemunerationTo"/>
                <owl:someValuesFrom rdf:resource="serviceProvider"/>
            </owl:Restriction>
        </rdfs:subClassOf>
        <skos:historyNote>Introduced in ISO/TS 14812:2025</skos:historyNote>
    </owl:Class>
</rdf:RDF>